a_ilen_read_uptoX_at proofs

proof/amd64/common/Keccak1600_subreadwrite.ec
@@ -2,13 +2,167 @@ require import AllCore IntDiv List StdOrder.
 
 require import BitEncoding.
 import BS2Int.
+import IntOrder.
 
 from Jasmin require import JModel_x86.
 from CryptoSpecs require import Keccak1600_Spec.
 from JazzEC require import Keccak1600_Jazz.
 
+require import Keccak_bindings.
+
 import SLH64.
 import IntOrder.
+
+(* MOVE TO SOMEWHERE ELSE? *)
+
+op bytes_at size cur at l=
+ take size (drop cur (nseq at W8.zero++l)++nseq size W8.zero).
+
+
+lemma size_bytes_at sz cur at l:
+ 0 <= sz =>
+ size (bytes_at sz cur at l) = sz.
+proof.
+move=> Hsz; rewrite size_take // size_cat size_nseq ler_maxr //.
+smt(size_ge0).
+qed.
+
+lemma size_bytes_at' sz cur at l:
+ size (bytes_at sz cur at l) = max 0 sz.
+proof.
+case: (0 <= sz) => ?.
+ by rewrite size_bytes_at // ler_maxr.
+by rewrite /bytes_at take_le0 /#.
+qed.
+
+lemma bytes_at_zeros n cur at:
+ 0 <= cur =>
+ bytes_at n cur at [W8.zero] = u8zeros n.
+proof.
+move=> *.
+apply (eq_from_nth W8.zero).
+ by rewrite size_bytes_at' size_nseq /#.
+move=> i; rewrite size_bytes_at' // => Hi.
+by rewrite nth_take 1..2:/# nth_cat ?size_drop 1:/# nth_drop 1..2:/# nth_cat !nth_u8zeros /#.
+qed.
+
+lemma get_u256bytes i w:
+ (u256bytes w).[i] = w \bits8 i.
+proof.
+case: (0 <= i < 32) => Hi.
+ by rewrite nth_to_list.
+rewrite bits8E nth_out ?size_to_list //.
+apply W8.ext_eq => k Hk.
+by rewrite zerowE initiE //= get_out /#.
+qed.
+
+lemma get_u128bytes i w:
+ (u128bytes w).[i] = w \bits8 i.
+proof.
+case: (0 <= i < 16) => Hi.
+ by rewrite nth_to_list.
+rewrite bits8E nth_out ?size_to_list //.
+apply W8.ext_eq => k Hk.
+by rewrite zerowE initiE //= get_out /#.
+qed.
+
+lemma get_u64bytes i w:
+ (u64bytes w).[i] = w \bits8 i.
+proof.
+case: (0 <= i < 8) => Hi.
+ by rewrite nth_to_list.
+rewrite bits8E nth_out ?size_to_list //.
+apply W8.ext_eq => k Hk.
+by rewrite zerowE initiE //= get_out /#.
+qed.
+
+lemma bits8_u64_shl8 (w: W64.t) k i:
+ 0 <= i < 8 =>
+ w `<<<` 8*k \bits8 i
+ = if i < k then W8.zero else w \bits8 (i-k).
+proof.
+move=> ?.
+apply W8.ext_eq => j Hj.
+rewrite bits8iE //=.
+rewrite (:0 <= i * 8 + j < 64) 1:/# /=.
+case: (i<k) => C.
+ by rewrite zerowE get_out /#.
+by rewrite bits8iE 1:/# /#.
+qed.
+
+lemma bits8_u128_shl8 (w: W128.t) k i:
+ 0 <= i < 16 =>
+ w `<<<` 8*k \bits8 i
+ = if i < k then W8.zero else w \bits8 (i-k).
+proof.
+move=> ?.
+apply W8.ext_eq => j Hj.
+rewrite bits8iE //=.
+rewrite (:0 <= i * 8 + j < 128) 1:/# /=.
+case: (i<k) => C.
+ by rewrite zerowE get_out /#.
+by rewrite bits8iE 1:/# /#.
+qed.
+
+lemma bits8_zeroextu64_32 (w: W32.t) i:
+ zeroextu64 w \bits8 i = if 0 <= i < 4 then w \bits8 i else W8.zero.
+proof.
+rewrite bits8E; apply W8.ext_eq => k Hk.
+case: (0 <= i < 8) => Hi.
+ rewrite initiE //= zeroextu64E pack2E initiE 1:/# /= initiE 1:/# /=.
+ case: (0 <= i < 4) => C.
+  by rewrite ifT 1:/# bits8E initiE /#.
+ by rewrite ifF 1:/# zerowE zerowE.
+by rewrite get_out 1:/# initiE //= get_out 1:/#.
+qed.
+
+lemma bits8_zeroextu64_16 (w: W16.t) i:
+ zeroextu64 w \bits8 i = if 0 <= i < 2 then w \bits8 i else W8.zero.
+proof.
+rewrite bits8E; apply W8.ext_eq => k Hk.
+case: (0 <= i < 8) => Hi.
+ rewrite initiE //= zeroextu64E pack4E initiE 1:/# /= initiE 1:/# /=.
+ case: (0 <= i < 2) => C.
+  by rewrite ifT 1:/# bits8E initiE /#.
+ by rewrite ifF 1:/# zerowE zerowE.
+by rewrite get_out 1:/# initiE //= get_out 1:/#.
+qed.
+
+lemma bits8_zeroextu64_8 (w: W8.t) i:
+ zeroextu64 w \bits8 i = if i=0 then w else W8.zero.
+proof.
+rewrite bits8E; apply W8.ext_eq => k Hk.
+case: (0 <= i < 8) => Hi.
+ rewrite initiE //= zeroextu64E pack8E initiE 1:/# /= initiE 1:/# /=.
+ case: (i=0) => C.
+  by rewrite ifT /#.
+ by rewrite ifF /#.
+by rewrite initiE //= ifF 1:/# get_out 1:/#.
+qed.
+
+lemma u64bytes_cat (w0 w1: W64.t):
+ u64bytes w0 ++ u64bytes w1
+ = u128bytes (VPINSR_2u64 (zeroextu128 w0) w1 W8.one).
+proof.
+by rewrite /VPINSR_2u64 to_uint1 /= /u64bytes /u128bytes /= zeroextu128E.
+qed.
+
+lemma u128bytes_cat (w0 w1: W128.t):
+ u128bytes w0 ++ u128bytes w1
+ = u256bytes (VINSERTI128 (zeroextu256 w0) w1 W8.one).
+proof.
+by rewrite /VINSERTI128 to_uint1 /= /u128bytes /u256bytes /= zeroextu256E.
+qed.
+
+lemma zeroextu128_zero:
+ zeroextu128 W64.zero = W128.zero
+by circuit.
+
+lemma zeroextu256_zero:
+ zeroextu256 W128.zero = W256.zero
+by circuit.
+
+(* *)
 
 lemma u64_shl0 (w: W64.t): w `<<<` 0 = w.
 proof. by apply W64.wordP => i Hi; rewrite shlwE Hi /=. qed.
@@ -137,80 +291,69 @@ module MM = {
                                lEN:int, tRAIL:int, cUR:int, aT:int) : 
   int * int * int * int * W64.t = {
     var w:W64.t;
-    var aT8:int;
     var t16:W64.t;
     var t8:W64.t;
     if ((((aT < cUR) \/ ((cUR + 8) <= aT)) \/ ((lEN = 0) /\ (tRAIL = 0)))) {
       w <- (W64.of_int 0);
     } else {
-      aT8 <- (aT - cUR);
       if ((8 <= lEN)) {
         w <-
         (get64_direct (WA.init8 (fun i => buf.[i])) (offset + dELTA));
-        w <@ M.__SHLQ (w, aT8);
-        dELTA <- (dELTA + (8 - aT8));
-        lEN <- (lEN - (8 - aT8));
-        aT8 <- 8;
+        w <@ M.__SHLQ (w, (aT - cUR));
+        dELTA <- (dELTA + ((cUR + 8) - aT));
+        lEN <- (lEN - ((cUR + 8) - aT));
+        aT <- (cUR + 8);
       } else {
         if ((4 <= lEN)) {
           w <-
           (zeroextu64
           (get32_direct (WA.init8 (fun i => buf.[i])) (offset + dELTA)
           ));
-          w <@ M.__SHLQ (w, aT8);
-          dELTA <- (dELTA + ((8 <= (4 + aT8)) ? (8 - aT8) : 4));
-          lEN <- (lEN - ((8 <= (4 + aT8)) ? (8 - aT8) : 4));
-          aT8 <- ((8 <= (4 + aT8)) ? 8 : (4 + aT8));
+          w <@ M.__SHLQ (w, (aT - cUR));
+          dELTA <-
+          (dELTA + (((cUR + 8) <= (aT + 4)) ? ((cUR + 8) - aT) : 4));
+          lEN <- (lEN - (((cUR + 8) <= (aT + 4)) ? ((cUR + 8) - aT) : 4));
+          aT <- (((cUR + 8) <= (aT + 4)) ? (cUR + 8) : (aT + 4));
         } else {
           w <- (W64.of_int 0);
         }
-        if (((aT8 < 8) /\ (2 <= lEN))) {
+        if (((aT < (cUR + 8)) /\ (2 <= lEN))) {
           t16 <-
           (zeroextu64
           (get16_direct (WA.init8 (fun i => buf.[i])) (offset + dELTA)
           ));
-          dELTA <- (dELTA + ((8 <= (2 + aT8)) ? (8 - aT8) : 2));
-          lEN <- (lEN - ((8 <= (2 + aT8)) ? (8 - aT8) : 2));
-          t16 <@ M.__SHLQ (t16, aT8);
+          dELTA <-
+          (dELTA + (((cUR + 8) <= (aT + 2)) ? ((cUR + 8) - aT) : 2));
+          lEN <- (lEN - (((cUR + 8) <= (aT + 2)) ? ((cUR + 8) - aT) : 2));
+          t16 <@ M.__SHLQ (t16, (aT - cUR));
           w <- (w `|` t16);
-          aT8 <- ((8 <= (2 + aT8)) ? 8 : (2 + aT8));
+          aT <- (((cUR + 8) <= (aT + 2)) ? (cUR + 8) : (aT + 2));
         } else {
           
         }
-        if ((aT8 < 8)) {
-          if ((1 <= lEN)) {
-            t8 <-
-            (zeroextu64
-            (get8_direct (WA.init8 (fun i => buf.[i]))
-            (offset + dELTA)));
-            t8 <- (t8 `|` (W64.of_int (256 * (tRAIL %% 256))));
-            dELTA <- (dELTA + 1);
-            lEN <- (lEN - 1);
-            t8 <@ M.__SHLQ (t8, aT8);
-            w <- (w `|` t8);
-            aT8 <- (aT8 + 1);
-            if (((aT8 < 8) /\ ((tRAIL %% 256) <> 0))) {
-              aT8 <- (aT8 + 1);
-              tRAIL <- 0;
-            } else {
-              
-            }
-          } else {
-            if (((tRAIL %% 256) <> 0)) {
-              t8 <- (W64.of_int (tRAIL %% 256));
-              t8 <@ M.__SHLQ (t8, aT8);
-              w <- (w `|` t8);
-              tRAIL <- 0;
-              aT8 <- (aT8 + 1);
-            } else {
-              
-            }
-          }
+        if (((aT < (cUR + 8)) /\ (1 <= lEN))) {
+          t8 <-
+          (zeroextu64
+          (get8_direct (WA.init8 (fun i => buf.[i])) (offset + dELTA))
+          );
+          dELTA <- (dELTA + 1);
+          lEN <- (lEN - 1);
+          t8 <@ M.__SHLQ (t8, (aT - cUR));
+          w <- (w `|` t8);
+          aT <- (aT + 1);
+        } else {
+          
+        }
+        if (((aT < (cUR + 8)) /\ (tRAIL <> 0))) {
+          t8 <- (W64.of_int (tRAIL %% 256));
+          t8 <- (t8 `<<` (W8.of_int (8 * (aT - cUR))));
+          w <- (w `|` t8);
+          aT <- (aT + 1);
+          tRAIL <- 0;
         } else {
           
         }
       }
-      aT <- (cUR + aT8);
     }
     return (dELTA, lEN, tRAIL, aT, w);
   }
@@ -218,36 +361,33 @@ module MM = {
                                 lEN:int, tRAIL:int, cUR:int, aT:int) : 
   int * int * int * int * W128.t = {
     var w:W128.t;
-    var aT16:int;
     var t64_0:W64.t;
     var t64_1:W64.t;
     if ((((aT < cUR) \/ ((cUR + 16) <= aT)) \/ ((lEN = 0) /\ (tRAIL = 0)))) {
       w <- (set0_128);
     } else {
-      aT16 <- (aT - cUR);
       if ((16 <= lEN)) {
         w <-
         (get128_direct (WA.init8 (fun i => buf.[i])) (offset + dELTA));
-        w <@ M.__SHLDQ (w, aT16);
-        dELTA <- (dELTA + (16 - aT16));
-        lEN <- (lEN - (16 - aT16));
-        aT16 <- 16;
+        w <@ M.__SHLDQ (w, (aT - cUR));
+        dELTA <- (dELTA + (16 - (aT - cUR)));
+        lEN <- (lEN - (16 - (aT - cUR)));
+        aT <- (cUR + 16);
       } else {
-        if ((8 <= aT16)) {
+        if (((cUR + 8) <= aT)) {
           w <- (set0_128);
-          (dELTA, lEN, tRAIL, aT16, t64_1) <@ __a_ilen_read_upto8_at (
-          buf, offset, dELTA, lEN, tRAIL, 8, aT16);
+          (dELTA, lEN, tRAIL, aT, t64_1) <@ __a_ilen_read_upto8_at (buf,
+          offset, dELTA, lEN, tRAIL, (cUR + 8), aT);
           w <- (VPINSR_2u64 w t64_1 (W8.of_int 1));
         } else {
-          (dELTA, lEN, tRAIL, aT16, t64_0) <@ __a_ilen_read_upto8_at (
-          buf, offset, dELTA, lEN, tRAIL, 0, aT16);
+          (dELTA, lEN, tRAIL, aT, t64_0) <@ __a_ilen_read_upto8_at (buf,
+          offset, dELTA, lEN, tRAIL, cUR, aT);
           w <- (zeroextu128 t64_0);
-          (dELTA, lEN, tRAIL, aT16, t64_1) <@ __a_ilen_read_upto8_at (
-          buf, offset, dELTA, lEN, tRAIL, 8, aT16);
+          (dELTA, lEN, tRAIL, aT, t64_1) <@ __a_ilen_read_upto8_at (buf,
+          offset, dELTA, lEN, tRAIL, (cUR + 8), aT);
           w <- (VPINSR_2u64 w t64_1 (W8.of_int 1));
         }
       }
-      aT <- (cUR + aT16);
     }
     return (dELTA, lEN, tRAIL, aT, w);
   }
@@ -255,37 +395,32 @@ module MM = {
                                 lEN:int, tRAIL:int, cUR:int, aT:int) : 
   int * int * int * int * W256.t = {
     var w:W256.t;
-    var aT32:int;
     var t128_0:W128.t;
     var t128_1:W128.t;
     if ((((aT < cUR) \/ ((cUR + 32) <= aT)) \/ ((lEN = 0) /\ (tRAIL = 0)))) {
       w <- (set0_256);
     } else {
-      aT32 <- (aT - cUR);
-      if (((aT32 = 0) /\ (32 <= lEN))) {
+      if (((aT = cUR) /\ (32 <= lEN))) {
         w <-
         (get256_direct (WA.init8 (fun i => buf.[i])) (offset + dELTA));
-        aT32 <- (aT32 + 32);
         dELTA <- (dELTA + 32);
         lEN <- (lEN - 32);
+        aT <- (aT + 32);
       } else {
-        if ((16 <= aT32)) {
+        if (((cUR + 16) <= aT)) {
           w <- (set0_256);
-          (dELTA, lEN, tRAIL, aT32, t128_1) <@ __a_ilen_read_upto16_at (
-          buf, offset, dELTA, lEN, tRAIL, 16, aT32);
+          (dELTA, lEN, tRAIL, aT, t128_1) <@ __a_ilen_read_upto16_at (
+          buf, offset, dELTA, lEN, tRAIL, (cUR + 16), aT);
           w <- (VINSERTI128 w t128_1 (W8.of_int 1));
         } else {
-          (dELTA, lEN, tRAIL, aT32, t128_0) <@ __a_ilen_read_upto16_at (
-          buf, offset, dELTA, lEN, tRAIL, 0, aT32);
-          (dELTA, lEN, tRAIL, aT32, t128_1) <@ __a_ilen_read_upto16_at (
-          buf, offset, dELTA, lEN, tRAIL, 16, aT32);
-          w <-
-          (W256.of_int
-          (((W128.to_uint t128_0) %% (2 ^ 128)) +
-          ((2 ^ 128) * (W128.to_uint t128_1))));
+          (dELTA, lEN, tRAIL, aT, t128_0) <@ __a_ilen_read_upto16_at (
+          buf, offset, dELTA, lEN, tRAIL, cUR, aT);
+          w <- (zeroextu256 t128_0);
+          (dELTA, lEN, tRAIL, aT, t128_1) <@ __a_ilen_read_upto16_at (
+          buf, offset, dELTA, lEN, tRAIL, (cUR + 16), aT);
+          w <- (VINSERTI128 w t128_1 (W8.of_int 1));
         }
       }
-      aT <- (cUR + aT32);
     }
     return (dELTA, lEN, tRAIL, aT, w);
   }
@@ -655,35 +790,28 @@ by islossless.
 
 
 
-op subread_pre cur at len tb =
- 0 <= cur && 0 <= at && 0 <= len && 0 <= tb < 256
- && at+len+b2i (tb<>0) <= 200
- && (cur<=at || len=0 && tb=0).
-
-op bytes_at size cur at l=
- take size (drop cur (nseq at W8.zero++l)++nseq size W8.zero).
-
-lemma size_bytes_at sz cur at l:
- 0 <= sz =>
- size (bytes_at sz cur at l) = sz.
-proof.
-move=> Hsz; rewrite size_take // size_cat size_nseq.
-smt(size_ge0).
-qed.
-
 lemma sub0 (buf: W8.t A.t) off:
  sub buf off 0 = [].
 proof. by rewrite -size_eq0 size_sub /#. qed.
 
-lemma nth_bytes_at sz cur at buf off len tb i:
+
+
+op subread_pre cur at off dlt len tb =
+ 0 <= cur /\ 0 <= at /\ 0 <= off /\ 0 <= dlt /\ 0 <= len /\ 0 <= tb < 256 /\
+ off + dlt + len <= _ASIZE /\
+ at + len + b2i (tb<>0) <= 200 /\
+ (cur <= at || len=0 /\ tb=0).
+
+
+lemma nth_bytes_at sz cur at buf off dlt len tb i:
  0 <= sz =>
- subread_pre cur at len tb =>
- nth W8.zero (bytes_at sz cur at (A.sub buf off len++[W8.of_int tb])) i
+ subread_pre cur at off dlt len tb =>
+ nth W8.zero (bytes_at sz cur at (A.sub buf (off+dlt) len++[W8.of_int tb])) i
  = if 0 <= at-cur <= i < sz
-   then nth W8.zero (sub buf off len++[W8.of_int tb]) (cur+i-at)
+   then nth W8.zero (sub buf (off+dlt) len++[W8.of_int tb]) (cur+i-at)
    else W8.zero.
 proof.
-move=> /> ???????[H|H].
+move=> /> ??????????[H|H].
 + case: (0 <= i < sz) => C; last first.
    by rewrite nth_out 1:size_bytes_at // ifF /#.
   case: (i < at-cur) => C1.
@@ -709,14 +837,16 @@ rewrite nth_out 1:size_nseq 1:/#.
 by rewrite nth_nseq /#.
 qed.
 
+
+
 op subread_spec
  (size: int)
  (buf: W8.t A.t) (off dlt len tb cur at: int)
  (dlt' len' tb' at': int) (w: W8.t list)
  : bool =
  0 <= size =>
- subread_pre cur at len tb =>
- subread_pre (cur+size) at' len' tb'
+ subread_pre cur at off dlt len tb =>
+ subread_pre (cur+size) at' off dlt' len' tb'
  /\ w = bytes_at size cur at (sub buf (off+dlt) len ++ [W8.of_int tb])
  /\ at+len+b2i(tb<>0)=at'+len'+b2i(tb'<>0)
  /\ (tb'=tb || len'=0 && tb'=0)
@@ -724,15 +854,14 @@ op subread_spec
  /\ at' = max at
               (min (cur+size)
                    (at+len+b2i (tb<>0)))
- /\ len' = max 0 (len - (max 0 (cur+size-at)))
- .
+ /\ len' = max 0 (len - (max 0 (cur+size-at))).
 
 lemma subread_specP N buf off dlt len trail cur at dlt' at' w':
  0 <= N =>
  cur <= at =>
- subread_pre cur at len trail =>
+ subread_pre cur at off dlt len trail =>
  subread_spec N buf off dlt len trail cur at dlt' 0 0 at' w' =>
- at' = at + len + b2i (trail%%256<>0)
+ at' = at + len + b2i (trail<>0)
  /\
  dlt' = dlt + len
  /\
@@ -740,7 +869,7 @@ lemma subread_specP N buf off dlt len trail cur at dlt' at' w':
  = bytes2state (nseq cur W8.zero++w').
 proof.
 move=> Hn Hcur Hpre Hspec.
-move: (Hpre) (Hspec Hn Hpre) => {Hspec} /> ???? H1 H2 H3 H4 H5.
+move: (Hpre) (Hspec Hn Hpre) => {Hspec} /> ?????????? H1 H2 H3 H4 H5.
 rewrite !b2i0 /= => H6 H7 H8.
 split; first smt().
 rewrite tP => i Hi.
@@ -767,6 +896,7 @@ case: (8 * i + k - at < len) => ? //.
 smt().
 qed.
 
+
 lemma subread_spec_ahead8 _buf _off _dlt _len _tb _cur _at:
  _cur + 8 <= _at =>
  subread_spec 8 _buf _off _dlt _len _tb _cur _at _dlt _len _tb _at (u64bytes W64.zero).
@@ -777,6 +907,18 @@ apply (eq_from_nth W8.zero); rewrite size_to_list.
  by rewrite size_bytes_at /#.
 move=> i Hi; rewrite nth_bytes_at // ifF 1:/#.
 by rewrite nth_to_list W8u8.get_zero.
+qed.
+
+lemma subread_spec_ahead16 _buf _off _dlt _len _tb _cur _at:
+ _cur + 16 <= _at =>
+ subread_spec 16 _buf _off _dlt _len _tb _cur _at _dlt _len _tb _at (u128bytes W128.zero).
+proof.
+move => H; rewrite /subread_spec => _ Hpre; split; first by smt().
+split; last smt().
+apply (eq_from_nth W8.zero); rewrite size_to_list.
+ by rewrite size_bytes_at /#.
+move=> i Hi; rewrite nth_bytes_at // ifF 1:/#.
+by rewrite nth_to_list W16u8.get_zero.
 qed.
 
 lemma subread_spec_ahead32 _buf _off _dlt _len _tb _cur _at:
@@ -800,8 +942,22 @@ have ->: _len=0 by smt().
 split; last smt().
 apply (eq_from_nth W8.zero).
  rewrite size_bytes_at /#.
-move=> i Hi; rewrite nth_bytes_at 1..2:/# !W8u8.get_zero /=.
+move=> i Hi; rewrite nth_bytes_at 1..2:/#.
 case: (0 <= _at - _cur <= i < 8) => C//.
+by rewrite nth_cat ?size_sub 1:/# sub0 /=.
+qed.
+
+lemma subread_spec_empty16 _buf _off _dlt _len _tb _cur _at:
+ _len <= 0 /\ _tb = 0 =>
+ subread_spec 16 _buf _off _dlt _len _tb _cur _at _dlt _len _tb _at (u128bytes W128.zero).
+proof.
+move => [Hlen ->]; rewrite /subread_spec /u128bytes /= !b2i0 /= => Hpre; split; first by smt().
+have ->: _len=0 by smt().
+split; last smt().
+apply (eq_from_nth W8.zero).
+ by rewrite size_bytes_at /#.
+move=> i Hi; rewrite nth_bytes_at 1..2:/# /=.
+case: (0 <= _at - _cur <= i < 16) => C//.
 by rewrite nth_cat ?size_sub 1:/# sub0 /=.
 qed.
 
@@ -814,16 +970,10 @@ have ->: _len=0 by smt().
 split; last smt().
 apply (eq_from_nth W8.zero).
  by rewrite size_bytes_at /#.
-move=> i Hi; rewrite nth_bytes_at 1..2:/# !W32u8.get_zero /=.
+move=> i Hi; rewrite nth_bytes_at 1..2:/# /=. 
 case: (0 <= _at - _cur <= i < 32) => C//.
 by rewrite nth_cat ?size_sub 1:/# sub0 /=.
 qed.
-
-(*
-lemma subread_spec_finished N buf off dlt cur at:
- at < cur =>
- subread_spec N buf 
-*)
 
 lemma bytes_at_absorb _buf _off _len _tb _at:
  0 <= _len => 0 <= _at =>
@@ -843,13 +993,13 @@ by rewrite nth_nseq 1:/#.
 qed.
 
 
-lemma subread_full buf off len tb at dlt' len' tb' at' wl:
- subread_pre 0 at len tb => 
- subread_spec 200 buf off 0 len tb 0 at dlt' len' tb' at' wl =>
+lemma subread_full buf off dlt len tb at dlt' len' tb' at' wl:
+ subread_pre 0 at off dlt len tb => 
+ subread_spec 200 buf off dlt len tb 0 at dlt' len' tb' at' wl =>
  at+len+b2i (tb<>0) <= 200 =>
  len' = 0 /\ tb' = 0
- /\ at'=at+len+b2i(tb<>0) /\ dlt'=len
- /\ bytes2state (u8zeros at ++ sub buf off len ++ [W8.of_int tb])
+ /\ at'=at+len+b2i(tb<>0) /\ dlt'=len+dlt
+ /\ bytes2state (u8zeros at ++ sub buf (off+dlt) len ++ [W8.of_int tb])
     = bytes2state wl.
 proof.
 move=> Hpre Hspec.
@@ -860,14 +1010,14 @@ by rewrite bytes_at_absorb 1..2:/#.
 qed.
 
 
-lemma subread_finished size buf off len tb at dlt' len' tb' at' wl:
+lemma subread_finished size buf off dlt len tb at dlt' len' tb' at' wl:
  0 <= size =>
- subread_pre 0 at len tb => 
- subread_spec size buf off 0 len tb 0 at dlt' len' tb' at' wl =>
+ subread_pre 0 at off dlt len tb => 
+ subread_spec size buf off dlt len tb 0 at dlt' len' tb' at' wl =>
  len' = 0 =>
  tb' = 0 =>
- at'= max at (at+len+b2i(tb<>0)) /\ dlt'=len
- /\ bytes2state (u8zeros at ++ sub buf off len ++ [W8.of_int tb])
+ at'= max at (at+len+b2i(tb<>0)) /\ dlt'=len+dlt
+ /\ bytes2state (u8zeros at ++ sub buf (off+dlt) len ++ [W8.of_int tb])
     = bytes2state wl.
 proof.
 move=> Hsize Hpre Hspec Hlen' Htb'.
@@ -891,26 +1041,6 @@ case: (tb=0) => Ctb.
  by rewrite Ctb /#.
 by rewrite ifF /#.
 qed.
-
-(*
-lemma subread_finish R size buf off dlt len tb cur at dlt' len' tb' at' wl:
- 0 <= size =>
- subread_pre cur at len tb => 
- subread_spec size buf off dlt len tb cur at dlt' len' tb' at' wl =>
- at+len+b2i (tb<>0) <= R =>
- R <= cur+size =>
- len' = 0 /\ tb' = 0
- /\ at'=at+len+b2i(tb<>0) /\ dlt'=dlt+len.
-proof.
-move=> Hsize Hpre Hspec.
-move: (Hspec Hsize Hpre).
-move: {Hspec} Hpre => /> ??? Hinv Hend _ _ ?? Hat HH.
-by move=> H1 H2 /#.
-qed.
-*)
-
-require import StdOrder.
-import IntOrder.
 
 lemma subread_spec_cat N1 N2 buf off dlt dlt' dlt'' len len' len'' tb tb' tb'' cur at at' at'' w' w'':
  0 <= N1 => 0 <= N2 =>
@@ -960,2003 +1090,538 @@ case: (at<=cur+N1) => Cat.
 smt().
 qed.
 
-lemma bytes_at8_zero cur at:
- 0 <= cur =>
- bytes_at 8 cur at [W8.zero] = u64bytes W64.zero.
+
+lemma get128_bytes (buf: W8.t A.t) off k:
+ 0 <= off =>
+ off + 16 <= _ASIZE =>
+ get128_direct (WA.init8 ("_.[_]" buf)) off \bits8 k
+ = (sub buf off 16).[k].
 proof.
-move=> *.
-rewrite /bytes_at; apply (eq_from_nth W8.zero).
- by rewrite size_to_list size_take 1:/# !size_cat size_drop 1:/# size_cat !size_nseq /= /#.
-rewrite size_take 1:/# !size_cat size_drop 1:/# size_cat !size_nseq /=.
-move=> i Hi.
-rewrite nth_take 1..2:/# nth_cat ?size_drop 1:/# u64bytes0 nth_drop 1..2:/# nth_cat !nth_u8zeros /#.
+move=> Ho1 Ho2; rewrite get128E.
+have->: W16u8.Pack.init (fun j => (WA.init8 ("_.[_]" buf)).[off+j])
+        = W16u8.Pack.of_list (sub buf off 16).
+ apply W16u8.Pack.ext_eq => i Hi.
+ by rewrite initiE 1:/# /= initiE 1:/# get_of_list // nth_sub.
+by rewrite get_pack16 1:size_sub // !nth_sub.
 qed.
 
-lemma buf8_expand buf base:
-  0 <= base =>
-  base + 8 < _ASIZE =>
-  (map (fun (j : int) => (WA.init8 (ReadWriteArray.A."_.[_]" buf)).[base + j]) (iota_ 0 8)) =
-  [buf.[base]; buf.[base + 1]; buf.[base + 2]; buf.[base + 3]; buf.[base + 4];
-   buf.[base + 5]; buf.[base + 6]; buf.[base + 7]].
+lemma get64_bytes (buf: W8.t A.t) off k:
+ 0 <= off =>
+ off + 8 <= _ASIZE =>
+ get64_direct (WA.init8 ("_.[_]" buf)) off \bits8 k
+ = (sub buf off 8).[k].
 proof.
-  move => H0 H1.
-  rewrite (eq_from_nth W8.zero _ ([buf.[base]; buf.[base + 1]; buf.[base + 2];
-                                   buf.[base + 3]; buf.[base + 4]; buf.[base + 5];
-                                   buf.[base + 6]; buf.[base + 7]])).
-     + rewrite size_map size_iota /#.
-     + rewrite size_map size_iota lez_maxr 1:/# => i0 i0_bnd.
-       rewrite (nth_map 0 W8.zero); first by smt(size_iota).
-       rewrite nth_iota 1:/# add0r /WA.init8 /=.
-       rewrite initE ifT. by rewrite (ltr_trans (base + 8)) /#.  
-  smt(). smt().
+move=> Ho1 Ho2; rewrite get64E.
+have->: W8u8.Pack.init (fun j => (WA.init8 ("_.[_]" buf)).[off+j])
+        = W8u8.Pack.of_list (sub buf off 8).
+ apply W8u8.Pack.ext_eq => i Hi.
+ by rewrite initiE 1:/# /= initiE 1:/# get_of_list // nth_sub.
+by rewrite get_pack8 1:size_sub // !nth_sub.
 qed.
 
-lemma buf4_expand buf base:
-  0 <= base =>
-  base + 8 < _ASIZE =>
-  (map (fun (j : int) => (WA.init8 (ReadWriteArray.A."_.[_]" buf)).[base + j]) (iota_ 0 4)) =
-  [buf.[base]; buf.[base + 1]; buf.[base + 2]; buf.[base + 3]].
+lemma get32_bytes (buf: W8.t A.t) off k:
+ 0 <= off =>
+ off + 4 <= _ASIZE =>
+ get32_direct (WA.init8 ("_.[_]" buf)) off \bits8 k
+ = (sub buf off 4).[k].
 proof.
-  move => H0 H1.
-  rewrite (eq_from_nth W8.zero _ ([buf.[base]; buf.[base + 1];
-                                   buf.[base + 2]; buf.[base + 3]])).
-     + rewrite size_map size_iota /#.
-     + rewrite size_map size_iota lez_maxr 1:/# => i0 i0_bnd.
-       rewrite (nth_map 0 W8.zero); first by smt(size_iota).
-       rewrite nth_iota 1:/# add0r /WA.init8 /=.
-       rewrite initE ifT. by rewrite (ltr_trans (base + 8)) /#.  
-  smt(). smt().
+move=> Ho1 Ho2; rewrite get32E.
+have->: W4u8.Pack.init (fun j => (WA.init8 ("_.[_]" buf)).[off+j])
+        = W4u8.Pack.of_list (sub buf off 4).
+ apply W4u8.Pack.ext_eq => i Hi.
+ by rewrite initiE 1:/# /= initiE 1:/# get_of_list // nth_sub.
+by rewrite get_pack4 1:size_sub // !nth_sub.
 qed.
 
-lemma expunge_W8u8 buf:
-  size buf = 8 =>
-  W64.init (fun i0 => (W8u8.Pack.init (fun i1 => buf.[i1])).[i0 %/ 8].[i0 %% 8]) =
-  W64.init (fun (i0 : int) => buf.[i0 %/ 8].[i0 %% 8]).
+lemma get16_bytes (buf: W8.t A.t) off k:
+ 0 <= off =>
+ off + 2 <= _ASIZE =>
+ get16_direct (WA.init8 ("_.[_]" buf)) off \bits8 k
+ = (sub buf off 2).[k].
 proof.
-  rewrite (W64.init_ext _ (fun (i0 : int) => buf.[i0 %/ 8].[i0 %% 8])).
-  by move => x x_bnd /=; rewrite W8u8.Pack.initE ifT /#. smt().
+move=> Ho1 Ho2; rewrite get16E.
+have->: W2u8.Pack.init (fun j => (WA.init8 ("_.[_]" buf)).[off+j])
+        = W2u8.Pack.of_list (sub buf off 2).
+ apply W2u8.Pack.ext_eq => i Hi.
+ by rewrite initiE 1:/# /= initiE 1:/# get_of_list // nth_sub.
+by rewrite get_pack2 1:size_sub // !nth_sub.
 qed.
 
-lemma W64_merge_inits (buf: W8.t list) x:
-  0<= size buf <= 8 =>
-  W64.init (fun (j : int) => (W64.init (fun (i0 : int) => buf.[i0 %/ 8].[i0 %% 8])).[x])
-   = W64.init (fun (j : int) => buf.[x%/8].[x%%8]).
+lemma get8_bytes (buf: W8.t A.t) off:
+ 0 <= off < _ASIZE =>
+ get8_direct (WA.init8 ("_.[_]" buf)) off
+ = buf.[off].
+proof. by move=> Hoff; rewrite /get8 initiE. qed.
+
+
+lemma bits8_shl_get64 buf off k i:
+ 0 <= off =>
+ 0 <= k < 8 =>
+ 0 <= i < 8 =>
+ off + 8 <= _ASIZE =>
+ get64_direct (WA.init8 (A."_.[_]" buf)) off `<<<` 8 * k \bits8 i
+ = if i < k then W8.zero else buf.[off+i-k].
 proof.
-  move => H.
-  rewrite (W64.init_ext (fun j => (W64.init (fun i0 => buf.[i0 %/ 8].[i0 %% 8])).[x])
-                        (fun j => buf.[x%/8].[x%%8])). move => x0 x0_bnd.
-  rewrite /= W64.initE.
-  case(0 <= x < 64) => x_in; first by smt().
-  + rewrite nth_out /#.
+move=> ????; rewrite bits8_u64_shl8 1:// get64_bytes 1..2:/#.
+case: (i<k) => // C.
+by rewrite nth_sub /#.
+qed.
+
+lemma subread_u128 _buf _off _dlt _len _trail _cur _at:
+ 16 <= _len =>
+ 0 <= _at-_cur < 16 =>
+ subread_spec 16 _buf _off _dlt _len _trail _cur _at
+  (_dlt + (16 - (_at - _cur))) (_len - (16 - (_at - _cur))) _trail (_cur + 16)
+  (u128bytes
+     (get128_direct (WA.init8 ("_.[_]" _buf)) (_off + _dlt) `<<<`
+      8 * (_at - _cur))).
+proof.
+move=> Hen Hcur _ Hpre; split; first smt().
+split; last smt().
+apply (eq_from_nth W8.zero).
+ rewrite size_to_list size_take // size_cat size_nseq ler_maxr //=.
+ by rewrite size_drop 1:/# !size_cat size_sub 1:/# size_nseq /= /#.
+move=> i; rewrite size_to_list => Hi.
+rewrite nth_bytes_at //.
+rewrite get_u128bytes bits8_u128_shl8 //.
+case: (_at-_cur <= i) => C.
+ by rewrite ifF 1:/# ifT 1:/# nth_cat size_sub 1:/# ifT 1:/# nth_sub 1:/# get128_bytes 1..2:/# nth_sub /#.
+by rewrite ifT 1:/# ifF 1:/#.
+qed.
+
+lemma subread_u64 _buf _off _dlt _len _trail _cur _at:
+ 8 <= _len =>
+ 0 <= _at-_cur < 8 =>
+ subread_spec 8 _buf _off _dlt _len _trail _cur _at (_dlt + (_cur + 8 - _at))
+  (_len - (_cur + 8 - _at)) _trail (_cur + 8)
+  (u64bytes
+     (get64_direct (WA.init8 ("_.[_]" _buf)) (_off + _dlt) `<<<`
+      8 * (_at - _cur))).
+proof.
+move=> Hen Hcur _ Hpre; split; first smt().
+split; last smt().
+apply (eq_from_nth W8.zero).
+ rewrite size_to_list size_take // size_cat size_nseq ler_maxr //=.
+ by rewrite size_drop 1:/# !size_cat size_sub 1:/# size_nseq /= /#.
+move=> i; rewrite size_to_list => Hi.
+rewrite nth_bytes_at //.
+rewrite get_u64bytes bits8_u64_shl8 //.
+case: (_at-_cur <= i) => C.
+ by rewrite ifF 1:/# ifT 1:/# nth_cat size_sub 1:/# ifT 1:/# nth_sub 1:/# get64_bytes 1..2:/# nth_sub /#.
+by rewrite ifT 1:/# ifF 1:/#.
+qed.
+
+lemma subread_u32 n _buf _off _dlt _cur _at :
+ 0 <= _at-_cur < 8 =>
+ n = min (_cur + 8 - _at) 4 =>
+ subread_spec 8 _buf _off _dlt 4 0 _cur
+   _at (_dlt+n) (4-n) 0 (_at+n)
+   (u64bytes (zeroextu64 (get32_direct (WA.init8 ("_.[_]" _buf)) (_off + _dlt)) `<<<`
+      8 * (_at - _cur))).
+proof.
+move=> Hen Hcur _ Hpre; split; first smt().
+split; last smt().
+apply (eq_from_nth W8.zero).
+ rewrite size_to_list size_take // size_cat size_nseq ler_maxr //=.
+ by rewrite size_drop 1:/# !size_cat size_sub 1:/# size_nseq /= /#.
+move=> i; rewrite size_to_list => Hi.
+rewrite nth_bytes_at //.
+rewrite get_u64bytes bits8_u64_shl8 //.
+case: (_at-_cur <= i) => C //=.
+ rewrite ifF 1:/# ifT 1:/# nth_cat size_sub 1:/# bits8_zeroextu64_32.
+ rewrite (:i - (_at - _cur)=_cur + i - _at) 1:/#; case: (0<= _cur + i - _at < 4) => ? //.
+  by rewrite get32_bytes /#.
+ case: (_cur + i - _at < 4) => // ?.
+ by rewrite nth_sub /#.
+by rewrite ifT 1:/#.
+qed.
+
+lemma u64bits8_subread i buf off cur dlt len tb at dlt1 len1 tb1 at1 (w:W64.t):
+ subread_pre cur at off dlt len tb =>
+ subread_spec 8 buf off dlt len tb cur at dlt1 len1 tb1 at1 (u64bytes w) =>
+ w \bits8 i
+ = (bytes_at 8 cur at (sub buf (off + dlt) len++[of_int tb])).[i].
+proof.
+move=> Hpre H; move: (H _ Hpre) => // |> ?E???.
+by rewrite -get_u64bytes E.
+qed.
+
+lemma subread_w4_u16 n1 buf off cur dlt len at dlt1 len1 at1 w:
+ 0 <= len < 8 =>
+ 2 <= len%%4 =>
+ 0 <= at-cur < 8 =>
+ at+n1 = min (cur+8) (at+len%/4*4+2) =>
+ subread_spec 8 buf off dlt (len%/4*4) 0 cur at
+   dlt1 len1 0 at1 (u64bytes w) =>
+ subread_spec 8 buf off dlt (len%/2*2) 0 cur at
+   (dlt+n1) (len%/2*2-n1) 0 (at+n1)
+   (u64bytes
+     (w `|`
+      (zeroextu64
+         (get16_direct (WA.init8 ("_.[_]" buf)) (off + dlt1)) `<<<` 8*(at1-cur)))).
+proof.
+move=> Hlen Hlen2 Hcur Hat H _ Hpre; split; first smt().
+have Hpre': subread_pre cur at off dlt (len %/ 4 * 4) 0 by smt().
+split.
+ apply (eq_from_nth W8.zero).
+  rewrite size_to_list size_take // size_cat size_nseq ler_maxr //=.
+  by rewrite size_drop 1:/# !size_cat size_sub 1:/# size_nseq /= /#.
+ move=> i; rewrite size_to_list => Hi.
+ rewrite get_u64bytes orb8E bits8_u64_shl8 //.
+ rewrite (u64bits8_subread _ _ _ _ _ _ _ _ _ _ _ _ _ Hpre' H).
+ rewrite bits8_zeroextu64_16 !nth_bytes_at // get16_bytes 1..2:/#.
+ case: (0 <= at - cur <= i < 8) => ?.
+  case: (i < at1 - cur) => ?.
+   by rewrite orw0 !nth_cat !size_sub 1..2:/# /= !ifT 1..2:/# !nth_sub /#.
+  case: (0 <= i - (at1 - cur) < 2) => ?.
+   rewrite nth_sub 1:/# !nth_cat !size_sub 1..2:/# ifF 1:/# ifT 1:/# /=.
+   by rewrite nth_sub /#.
+  by rewrite orw0 !nth_cat !size_sub 1..2:/# ifF 1:/# ifF 1:/#.
+ rewrite or0w; case: (i < at1-cur) => ? //.
+ case: (0 <= i - (at1 - cur) < 2) => ? //.
+ by rewrite nth_sub /#.
+smt().
+qed.
+
+lemma subread_w4_ahead buf off cur dlt len at dlt1 len1 at1 w:
+ 0 <= len < 8 =>
+ 0 <= at-cur < 8 =>
+ at1 = cur+8 =>
+ subread_spec 8 buf off dlt (len%/4*4) 0 cur at
+   dlt1 len1 0 at1 (u64bytes w) =>
+ subread_spec 8 buf off dlt (len%/2*2) 0 cur at
+   dlt1 (len%/2*2-(cur+8-at)) 0 at1 (u64bytes w).
+proof.
+move=> Hlen Hcur Hat H _ Hpre; split; first smt().
+split.
+ move: (H _ _); 1..2:smt().
+ move => |> _ -> ??.
+ apply (eq_from_nth W8.zero); rewrite !size_bytes_at // => k Hk.
+ rewrite !nth_bytes_at //; first smt().
+ case: (0 <= at - cur <= k < 8) => ?//.
+ rewrite !nth_cat !size_sub 1..2:/#.
+ case: (cur + k - at < len %/ 4 * 4) => ?.
+  by rewrite ifT 1:/# !nth_sub /#.
+ by rewrite ifF 1:/#.
+smt().
+qed.
+
+lemma subread_w2_u8 n2 buf off cur dlt len at dlt1 len1 at1 w:
+ 0 <= len < 8 =>
+ 1 <= len%%2 =>
+ 0 <= at1-cur < 8 =>
+ at+n2 = at+len =>
+ subread_spec 8 buf off dlt (len%/2*2) 0 cur at
+   dlt1 len1 0 at1 (u64bytes w) =>
+ subread_spec 8 buf off dlt len 0 cur at
+   (dlt+n2) (len-n2) 0 (at+n2)
+   (u64bytes
+     (w `|`
+      (zeroextu64
+         (get8_direct (WA.init8 ("_.[_]" buf)) (off + dlt1)) `<<<` 8*(at1-cur)))).
+proof.
+move=> Hlen Hlen2 Hcur Hat H _ Hpre; split; first smt().
+have Hpre': subread_pre cur at off dlt (len %/ 2 * 2) 0 by smt().
+split.
+ apply (eq_from_nth W8.zero).
+  rewrite size_to_list size_take // size_cat size_nseq ler_maxr //=.
+  by rewrite size_drop 1:/# !size_cat size_sub 1:/# size_nseq /= /#.
+ move=> i; rewrite size_to_list => Hi.
+ rewrite get_u64bytes orb8E bits8_u64_shl8 //.
+ rewrite (u64bits8_subread _ _ _ _ _ _ _ _ _ _ _ _ _ Hpre' H).
+ rewrite bits8_zeroextu64_8 !nth_bytes_at // get8_bytes 1:/#.
+ case: (0 <= at - cur <= i < 8) => ?.
+  case: (i < at1 - cur) => ?.
+   by rewrite orw0 !nth_cat !size_sub 1..2:/# /= !ifT 1..2:/# !nth_sub /#.
+  case: (i = (at1 - cur)) => ?.
+   rewrite !nth_cat !size_sub 1..2:/# ifF 1:/# ifT 1:/# /=.
+   by rewrite nth_sub /#.
+  by rewrite ifF 1:/# orw0 !nth_cat !size_sub 1..2:/# ifF 1:/# ifF 1:/#.
+ rewrite or0w; case: (i < at1-cur) => ? //.
+ by rewrite ifF 1:/#.
+smt().
+qed.
+
+lemma subread_w2_ahead buf off cur dlt len at dlt1 len1 at1 w:
+ 0 <= len < 8 =>
+ 0 <= at-cur < 8 =>
+ at1 = cur+8 =>
+ subread_spec 8 buf off dlt (len%/2*2) 0 cur at
+   dlt1 len1 0 at1 (u64bytes w) =>
+ subread_spec 8 buf off dlt len 0 cur at
+   dlt1 (len-(cur+8-at)) 0 at1 (u64bytes w).
+proof.
+move=> Hlen Hcur Hat H _ Hpre; split; first smt().
+split.
+ move: (H _ _); 1..2:smt().
+ move => |> _ -> ??.
+ apply (eq_from_nth W8.zero); rewrite !size_bytes_at // => k Hk.
+ rewrite !nth_bytes_at //; first smt().
+ case: (0 <= at - cur <= k < 8) => ?//.
+ rewrite !nth_cat !size_sub 1..2:/#.
+ case: (cur + k - at < len %/ 2 * 2) => ?.
+  by rewrite ifT 1:/# !nth_sub /#.
+ by rewrite ifF 1:/#.
+smt().
+qed.
+
+lemma subread_w8_trail buf off cur dlt len trail at dlt1 len1 at1 w:
+ trail <> 0 =>
+ 0 <= len < 8 =>
+ 0 <= at-cur < 8 =>
+ at1 < cur+8 =>
+ subread_spec 8 buf off dlt len 0 cur at dlt1 len1 0 at1 (u64bytes w) =>
+ subread_spec 8 buf off dlt len trail cur at dlt1 len1 0 (at1+1)
+   (u64bytes
+     (w `|` (W64.of_int (trail %% 256) `<<` W8.of_int (8 * (at1 - cur))))).
+proof.
+move=> Htb Hlen Hlen2 Hat H _ Hpre.
+have Hpre': subread_pre cur at off dlt len 0 by smt().
+move: (H _ Hpre') => // /> ????????E??.
+split; first smt().
+split.
+ apply (eq_from_nth W8.zero); rewrite size_to_list ?size_bytes_at // => k Hk.
+ rewrite b2i0 /=.
+ rewrite get_u64bytes orb8E -get_u64bytes E !nth_bytes_at //.
+ case: (0 <= at - cur <= k < 8) => ?; last first.
+  rewrite or0w bits8E; apply W8.ext_eq => j Hj /=.
+  rewrite initiE //= /(`<<`) of_uintK (modz_small _ W8.modulus) 1:/# /=.
+  by rewrite (:0 <= k * 8 + j < 64) 1:/# /= of_intwE /#.
+ rewrite !nth_cat size_sub 1:/#.
+ case: (cur + k - at < len) => C.
+  rewrite bits8E /=; pose W:= W8.init _.
+  have ->: W = W8.zero.
+   apply W8.ext_eq => j Hj; rewrite zerowE /W initiE /(`<<`) //=.
+   by rewrite of_intwE /#.
+  by rewrite orw0.
+ rewrite or0w.
+ rewrite /(`<<`) bits8E; apply W8.ext_eq => j Hj /=.
+ rewrite initiE //=.
+ have ->: forall n, (W64.of_int (trail %% 256)).[n] = (W8.of_int trail).[n].
+  move=> n; case: (0 <= n < 8) => ?.
+   by rewrite !of_intwE (:trail%%256=trail) 1:/# /W64.int_bit /W8.int_bit /#.
+  case: (0 <= n < 64) => ?.
+   rewrite W8.get_out 1:/# of_intwE /W64.int_bit.
+   rewrite (:trail %% 256 %% W64.modulus = trail) 1:/#.
+   have ?: 8 <= n < 64 by smt().
+   rewrite divz_small; split; first smt().
+   move=> _. apply (ltr_le_trans W8.modulus); first smt().
+   rewrite ger0_norm; first smt(expr_ge0).
+   by apply ler_weexpn2l => /#.
+  by rewrite !get_out /#.
+ case: (cur + k - at - len = 0) => ?.
   smt().
+ by rewrite zerowE get_out /#.
+smt().
 qed.
 
-
-lemma preu64_0s x i _buf pos:
-  0 <= x =>
-  64 + x <= i < 8 =>
-  (get64_direct (WA.init8 (ReadWriteArray.A."_.[_]" _buf)) pos) `<<<` 8 * x
-  \bits8 nth witness (iota_ 0 8) i = W8.zero.
+lemma subread_w8_trail_ahead buf off cur dlt len trail at dlt1 len1 at1 w:
+ 0 <= len < 8 =>
+ 0 <= at-cur < 8 =>
+ at1 = cur+8 =>
+ subread_spec 8 buf off dlt len 0 cur at dlt1 len1 0 at1 (u64bytes w) =>
+ subread_spec 8 buf off dlt len trail cur at dlt1 len1 trail at1 (u64bytes w).
 proof.
-  move => H0 H1.
-  rewrite /(\bits8) (W8.ext_eq _ W8.zero). move => x0 x0_bnd.
-  rewrite initE ifT 1:/# /=.
-  rewrite (nth_change_dfl 0 witness) 1:size_iota 1:/#.
-  have->: 0 <= nth 0 (iota_ 0 8) i * 8 + x0 < 64 by smt(nth_iota).
-  rewrite andaE andTb.
-  have aux: 32 <= nth 0 (iota_ 0 8) i * 8 + x0 - 8 * x < 64. smt(nth_iota).
-  rewrite nth_iota /#. smt().
-qed.
-
-lemma posu64_0s x i _buf pos:
-  0 <= x =>
-  0 <= i < min 8 x =>
-  (get64_direct (WA.init8 (ReadWriteArray.A."_.[_]" _buf)) pos) `<<<` 8 * x
-  \bits8 nth witness (iota_ 0 8) i = W8.zero.
-proof.
-  move => H0 H1.
-  rewrite /(\bits8) (W8.ext_eq _ W8.zero). move => x0 x0_bnd.
-  rewrite initE ifT 1:/# /=.
-  case(8 < x) => x_max.
-  rewrite (nth_change_dfl 0 witness) 1:size_iota 1:/#.
-  have->: 0 <= nth 0 (iota_ 0 8) i * 8 + x0 < 64 by smt(nth_iota).
-  rewrite andaE andTb get_out; smt(nth_iota).
-  have->: 0 <= nth witness (iota_ 0 8) i * 8 + x0 < 64 by smt(nth_iota).
-  rewrite andaE andTb get_out; smt(nth_iota). smt().
+move=> Hlen Hcur Hat H _ Hpre; split; first smt().
+split.
+ move: (H _ _); 1..2:smt().
+ move => |> _ -> ??.
+ apply (eq_from_nth W8.zero); rewrite !size_bytes_at // => k Hk.
+ rewrite !nth_bytes_at //; first smt().
+ case: (0 <= at - cur <= k < 8) => ?//.
+ by rewrite !nth_cat !size_sub /#.
+smt().
 qed.
 
 
-lemma preu32_0s x i _buf pos:
-  0 <= x =>
-  4 + x <= i < 8 =>
-  zeroextu64 (get32_direct (WA.init8 (ReadWriteArray.A."_.[_]" _buf)) pos) `<<<` 8 * x
-  \bits8 nth witness (iota_ 0 8) i = W8.zero.
-proof.
-  move => H0 H1.
-  pose a:= (get32_direct (WA.init8 ("_.[_]" _buf)) pos).
-  rewrite /zeroextu64 {1}/W64.of_int /to_uint pmod_small. 
-  + split. smt(bs2int_ge0). move =>*.
-  + rewrite (ltr_trans (2^size (W32.w2bits a))). rewrite bs2int_le2Xs. smt().
-  rewrite (int2bs_cat 32) 1:/# pdiv_small.
-  + split. smt(bs2int_ge0). move =>*. 
-  + rewrite (ltr_le_trans (2^size (W32.w2bits a))). rewrite bs2int_le2Xs. smt().
-  rewrite int2bs0 W64_bits2w_cat_nseq0. 
-  have->: 32 = size (w2bits a) by rewrite size_w2bits.
-  rewrite bs2intK /(\bits8) (W8.ext_eq _ W8.zero). move => x0 x0_bnd.
-  rewrite initE ifT 1:/# /=.
-  rewrite (nth_change_dfl 0 witness) 1:size_iota 1:/#.
-  have->: 0 <= nth 0 (iota_ 0 8) i * 8 + x0 < 64 by smt(nth_iota).
-  rewrite andaE andTb.
-  have aux: 32 <= nth 0 (iota_ 0 8) i * 8 + x0 - 8 * x < 64. smt(nth_iota).
-  rewrite get_bits2w 1:/# get_w2bits get_out /#. smt().
-qed.
 
-
-lemma posu32_0s x i _buf pos:
-  0 <= x =>
-  0 <= i < min 8 x =>
-  zeroextu64 (get32_direct (WA.init8 (ReadWriteArray.A."_.[_]" _buf)) pos) `<<<` 8 * x
-  \bits8 nth witness (iota_ 0 8) i = W8.zero.
-proof.
-  move => H0 H1.
-  pose a:= (get32_direct (WA.init8 ("_.[_]" _buf)) pos).
-  rewrite /zeroextu64 {1}/W64.of_int /to_uint pmod_small. 
-  + split. smt(bs2int_ge0). move =>*.
-  + rewrite (ltr_trans (2^size (W32.w2bits a))). rewrite bs2int_le2Xs. smt().
-  rewrite (int2bs_cat 32) 1:/# pdiv_small.
-  + split. smt(bs2int_ge0). move =>*. 
-  + rewrite (ltr_le_trans (2^size (W32.w2bits a))). rewrite bs2int_le2Xs. smt().
-  rewrite int2bs0 W64_bits2w_cat_nseq0. 
-  have->: 32 = size (w2bits a) by rewrite size_w2bits.
-  rewrite bs2intK /(\bits8) (W8.ext_eq _ W8.zero). move => x0 x0_bnd.
-  rewrite initE ifT 1:/# /=.
-  case(8 < x) => x_max.
-  rewrite (nth_change_dfl 0 witness) 1:size_iota 1:/#.
-  have->: 0 <= nth 0 (iota_ 0 8) i * 8 + x0 < 64 by smt(nth_iota).
-  rewrite andaE andTb get_out; smt(nth_iota).
-  have->: 0 <= nth witness (iota_ 0 8) i * 8 + x0 < 64 by smt(nth_iota).
-  rewrite andaE andTb get_out; smt(nth_iota). smt().
-qed.
-
-
-lemma u32_word x i _buf pos:
-  0 <= x =>
-  min 8 x <= i < min 8 (4 + x) =>
-  zeroextu64 (get32_direct (WA.init8 (ReadWriteArray.A."_.[_]" _buf)) pos) `<<<` 8 * x
-  \bits8 nth witness (iota_ 0 8) i =
-  (get32_direct (WA.init8 (ReadWriteArray.A."_.[_]" _buf)) pos)
-  \bits8 nth 0 (iota_ 0 (min 4 (8-x))) (i-x).
-proof.
-  move => H0 H1.
-  pose a:= (get32_direct (WA.init8 ("_.[_]" _buf)) pos).
-  rewrite /zeroextu64 {1}/W64.of_int /to_uint pmod_small. 
-  + split. smt(bs2int_ge0). move =>*.
-  + rewrite (ltr_trans (2^size (W32.w2bits a))). rewrite bs2int_le2Xs. smt().
-  rewrite (int2bs_cat 32) 1:/# pdiv_small.
-  + split. smt(bs2int_ge0). move =>*. 
-  + rewrite (ltr_le_trans (2^size (W32.w2bits a))). rewrite bs2int_le2Xs. smt().
-  rewrite int2bs0 W64_bits2w_cat_nseq0. 
-  have->: 32 = size (w2bits a) by rewrite size_w2bits.
-  rewrite bs2intK /(\bits8) (W8.ext_eq _ (a \bits8 nth 0 (iota_ 0 (min 4 (8-x))) (i-x))).
-  move => x0 x0_bnd.
-  rewrite initE ifT 1:/# /=.
-  case(8 <= x) => x_max.
-  rewrite (nth_change_dfl 0 witness) 1:size_iota 1:/#.
-  have->: 0 <= nth 0 (iota_ 0 8) i * 8 + x0 < 64 by smt(nth_iota).
-  rewrite andaE andTb get_out; smt(nth_iota).
-  rewrite (nth_change_dfl 0 witness) 1:size_iota 1:/# get_bits2w. smt(nth_iota).  
-  have->: 0 <= nth 0 (iota_ 0 8) i * 8 + x0 < 64 by smt(nth_iota).
-  rewrite andaE andTb get_w2bits /(\bits8) initE ifT 1:/# /=.
-  smt(nth_iota). 
-  rewrite /(\bits8) /#.
-qed.
-
-lemma preu16_0s x y i _buf pos:
-  0 <= y =>
-  0 <= x =>
-  y + 2 + x <= i < 8 =>
-  zeroextu64 (get16_direct (WA.init8 (ReadWriteArray.A."_.[_]" _buf)) (pos+y))
-   `<<<` 8 * (y + x) \bits8 nth witness (iota_ 0 8) i = W8.zero.
-proof.
-  move => H0 H1 H2.
-  pose a:= (get16_direct (WA.init8 ("_.[_]" _buf)) (pos+y)).
-  rewrite /zeroextu64 {1}/W64.of_int /to_uint pmod_small. 
-  + split. smt(bs2int_ge0). move =>*.
-  + rewrite (ltr_trans (2^size (W16.w2bits a))). rewrite bs2int_le2Xs. smt().
-  rewrite (int2bs_cat 16) 1:/# pdiv_small.
-  + split. smt(bs2int_ge0). move =>*. 
-  + rewrite (ltr_le_trans (2^size (W16.w2bits a))). rewrite bs2int_le2Xs. smt().
-  rewrite int2bs0 W64_bits2w_cat_nseq0. 
-  have->: 16 = size (w2bits a) by rewrite size_w2bits.
-  rewrite bs2intK /(\bits8) (W8.ext_eq _ W8.zero). move => x0 x0_bnd.
-  rewrite initE ifT 1:/# /=.
-  rewrite (nth_change_dfl 0 witness) 1:size_iota 1:/#.
-  have->: 0 <= nth 0 (iota_ 0 8) i * 8 + x0 < 64 by smt(nth_iota).
-  rewrite andaE andTb.
-  have aux: 16 <= nth 0 (iota_ 0 8) i * 8 + x0 - 8 * (y + x) < 64. smt(nth_iota).
-  rewrite get_bits2w 1:/# get_w2bits get_out /#.
-  smt().
-qed.
-
-lemma posu16_0s x y i _buf pos:
-  0 <= y =>
-  0 <= x =>
-  0 <= i < min 8 (y + x) =>
-  zeroextu64 (get16_direct (WA.init8 (ReadWriteArray.A."_.[_]" _buf)) (pos + y))
-    `<<<` 8 * (y + x) \bits8 nth witness (iota_ 0 8) i = W8.zero.
-proof.
-  move => H0 H1 H2.
-  pose a:= (get16_direct (WA.init8 ("_.[_]" _buf)) (pos + y)).
-  rewrite /zeroextu64 {1}/W64.of_int /to_uint pmod_small. 
-  + split. smt(bs2int_ge0). move =>*.
-  + rewrite (ltr_trans (2^size (W16.w2bits a))). rewrite bs2int_le2Xs. smt().
-  rewrite (int2bs_cat 16) 1:/# pdiv_small.
-  + split. smt(bs2int_ge0). move =>*. 
-  + rewrite (ltr_le_trans (2^size (W16.w2bits a))). rewrite bs2int_le2Xs. smt().
-  rewrite int2bs0 W64_bits2w_cat_nseq0. 
-  have->: 16 = size (w2bits a) by rewrite size_w2bits.
-  rewrite bs2intK /(\bits8) (W8.ext_eq _ W8.zero). move => x0 x0_bnd.
-  rewrite initE ifT 1:/# /=.
-  rewrite (nth_change_dfl 0 witness) 1:size_iota 1:/#.
-  have->: 0 <= nth 0 (iota_ 0 8) i * 8 + x0 < 64 by smt(nth_iota).
-  rewrite andaE andTb get_out; smt(nth_iota).
-  smt().
-qed.
-
-lemma u16_word x y i _buf pos:
-  0 <= y =>
-  0 <= x =>
-  min 8 (y+x) <= i < min 8 (y + 2 + x) =>
-  zeroextu64 (get16_direct (WA.init8 (ReadWriteArray.A."_.[_]" _buf)) (pos + y))
-    `<<<` 8 * (y + x) \bits8 nth witness (iota_ 0 8) i =
-  (get16_direct (WA.init8 (ReadWriteArray.A."_.[_]" _buf)) (pos + y))
-  \bits8 nth 0 (iota_ 0 2) (i-y-x).
-proof.
-  move => H0 H1 H2.
-  pose a:= (get16_direct (WA.init8 ("_.[_]" _buf)) (pos + y)).
-  rewrite /zeroextu64 {1}/W64.of_int /to_uint pmod_small. 
-  + split. smt(bs2int_ge0). move =>*.
-  + rewrite (ltr_trans (2^size (W16.w2bits a))). rewrite bs2int_le2Xs. smt().
-  rewrite (int2bs_cat 16) 1:/# pdiv_small.
-  + split. smt(bs2int_ge0). move =>*. 
-  + rewrite (ltr_le_trans (2^size (W16.w2bits a))). rewrite bs2int_le2Xs. smt().
-  rewrite int2bs0 W64_bits2w_cat_nseq0. 
-  have->: 16 = size (w2bits a) by rewrite size_w2bits.
-  rewrite bs2intK /(\bits8) (W8.ext_eq _ (a \bits8 nth 0 (iota_ 0 2) (i-y-x))).
-  move => x0 x0_bnd.
-  rewrite initE ifT 1:/# /=.
-  rewrite (nth_change_dfl 0 witness) 1:size_iota 1:/#.
-  have->: 0 <= nth 0 (iota_ 0 8) i * 8 + x0 < 64 by smt(nth_iota).
-  rewrite andaE andTb.
-  case(8 <= y + x) => *.
-  + rewrite !get_out /#.
-  + rewrite /(\bits8)initE ifT 1:/# /= get_bits2w. smt(nth_iota).
-    rewrite get_w2bits !nth_iota /#. smt().
-qed.
-
-lemma preu8_0s x y i _buf pos:
-  0 <= y =>
-  0 <= x =>
-  y + 1 + x <= i < 8 =>
-  zeroextu64 (get8_direct (WA.init8 (ReadWriteArray.A."_.[_]" _buf)) (pos+y))
-   `<<<` 8 * (y + x) \bits8 nth witness (iota_ 0 8) i = W8.zero.
-proof.
-  move => H0 H1 H2.
-  pose a:= (get8_direct (WA.init8 ("_.[_]" _buf)) (pos+y)).
-  rewrite /zeroextu64 {1}/W64.of_int /to_uint pmod_small. 
-  + split. smt(bs2int_ge0). move =>*.
-  + rewrite (ltr_trans (2^size (W8.w2bits a))). rewrite bs2int_le2Xs. smt().
-  rewrite (int2bs_cat 8) 1:/# pdiv_small.
-  + split. smt(bs2int_ge0). move =>*. 
-  + rewrite (ltr_le_trans (2^size (W8.w2bits a))). rewrite bs2int_le2Xs. smt().
-  rewrite int2bs0 W64_bits2w_cat_nseq0. 
-  have->: 8 = size (w2bits a) by rewrite size_w2bits.
-  rewrite bs2intK /(\bits8) (W8.ext_eq _ W8.zero). move => x0 x0_bnd.
-  rewrite initE ifT 1:/# /=.
-  rewrite (nth_change_dfl 0 witness) 1:size_iota 1:/#.
-  have->: 0 <= nth 0 (iota_ 0 8) i * 8 + x0 < 64 by smt(nth_iota).
-  rewrite andaE andTb.
-  have aux: 8 <= nth 0 (iota_ 0 8) i * 8 + x0 - 8 * (y + x) < 64. smt(nth_iota).
-  rewrite get_bits2w 1:/# get_w2bits get_out /#.
-  smt().
-qed.
-
-lemma posu8_0s x y i _buf pos:
-  0 <= y =>
-  0 <= x =>
-  0 <= i < min 8 (y + x) =>
-  zeroextu64 (get8_direct (WA.init8 (ReadWriteArray.A."_.[_]" _buf)) (pos + y))
-    `<<<` 8 * (y + x) \bits8 nth witness (iota_ 0 8) i = W8.zero.
-proof.
-  move => H0 H1 H2.
-  pose a:= (get8_direct (WA.init8 ("_.[_]" _buf)) (pos + y)).
-  rewrite /zeroextu64 {1}/W64.of_int /to_uint pmod_small. 
-  + split. smt(bs2int_ge0). move =>*.
-  + rewrite (ltr_trans (2^size (W8.w2bits a))). rewrite bs2int_le2Xs. smt().
-  rewrite (int2bs_cat 8) 1:/# pdiv_small.
-  + split. smt(bs2int_ge0). move =>*. 
-  + rewrite (ltr_le_trans (2^size (W8.w2bits a))). rewrite bs2int_le2Xs. smt().
-  rewrite int2bs0 W64_bits2w_cat_nseq0. 
-  have->: 8 = size (w2bits a) by rewrite size_w2bits.
-  rewrite bs2intK /(\bits8) (W8.ext_eq _ W8.zero). move => x0 x0_bnd.
-  rewrite initE ifT 1:/# /=.
-  case(8 < x) => x_max.
-  rewrite (nth_change_dfl 0 witness) 1:size_iota 1:/#.
-  have->: 0 <= nth 0 (iota_ 0 8) i * 8 + x0 < 64 by smt(nth_iota).
-  rewrite andaE andTb get_out; smt(nth_iota).
-  have->: 0 <= nth witness (iota_ 0 8) i * 8 + x0 < 64 by smt(nth_iota).
-  rewrite andaE andTb get_out; smt(nth_iota). smt().
-qed.
-
-lemma u8_word x y i _buf pos:
-  0 <= y =>
-  0 <= x =>
-  min 8 (y + x) <= i < min 8 (y + 1 + x) =>
-  zeroextu64 (get8_direct (WA.init8 (ReadWriteArray.A."_.[_]" _buf)) (pos + y))
-    `<<<` 8 * (y + x) \bits8 nth witness (iota_ 0 8) i =
-  [get8 (WA.init8 ("_.[_]" _buf)) (pos + y)].[i - y - x].
-proof.
-  move => H0 H1 H2.
-  pose a:= (get8_direct (WA.init8 ("_.[_]" _buf)) (pos + y)).
-  rewrite /zeroextu64 {1}/W64.of_int /to_uint pmod_small. 
-  + split. smt(bs2int_ge0). move =>*.
-  + rewrite (ltr_trans (2^size (W8.w2bits a))). rewrite bs2int_le2Xs. smt().
-  rewrite (int2bs_cat 8) 1:/# pdiv_small.
-  + split. smt(bs2int_ge0). move =>*. 
-  + rewrite (ltr_le_trans (2^size (W8.w2bits a))). rewrite bs2int_le2Xs. smt().
-  rewrite int2bs0 W64_bits2w_cat_nseq0. 
-  have->: 8 = size (w2bits a) by rewrite size_w2bits.
-  rewrite /(\bits8) bs2intK.
-  rewrite (W8.ext_eq _ ([get8 (WA.init8 ("_.[_]" _buf)) (pos+y)].[i-y-x])).
-  move => x0 x0_bnd.
-  rewrite initE ifT 1:/# /=.
-  rewrite (nth_change_dfl 0 witness) 1:size_iota 1:/#.
-  have->: 0 <= nth 0 (iota_ 0 8) i * 8 + x0 < 64 by smt(nth_iota).
-  rewrite andaE andTb nth_iota 1:/# /=.
-  case(i - y - x = 0) => u8_eq.
-  + rewrite get_bits2w 1:/# get_w2bits /#.
-  + smt().
-  smt().
-qed.
-
-lemma preTrail_0s x off i _trail:
-  0 <= x =>
-  0 <= off =>
-  0 <= _trail =>
-  _trail < 256 =>
-  off + 1 + x <= i < 8 =>
-  W64.of_int _trail `<<<` 8 * (off + x) \bits8 nth witness (iota_ 0 8) i =
-  W8.zero.
-proof.
-  move => H0 H1 H2 H3 H4.
-  rewrite nth_iota 1:/# /(\bits8) /= (W8.ext_eq _ W8.zero). move => x0 x0_bnd.
-    rewrite initE ifT 1:/# /= andaE. have->: 0 <= i * 8 + x0 < 64 by smt().
-    rewrite andTb /of_int get_bits2w 1:/# pmod_small 1:/#.
-    rewrite (int2bs_cat 8) 1:/# pdiv_small 1:/# nth_cat size_int2bs ifF 1:/# int2bs0.
-    rewrite nth_nseq /#. smt().
-qed.
-
-lemma posTrail_0s x i off _trail:
-  0 <= x =>
-  0 <= off =>
-  0 <= i < min 8 (off + x) =>
-  0 <= _trail =>
-  _trail < 256 =>
-  W64.of_int _trail `<<<` 8 * (off + x) \bits8 nth witness (iota_ 0 8) i = W8.zero.
-proof.
-  move => H0 H1 H2 H3 H4.
-  rewrite /zeroextu64 {1}/W64.of_int /to_uint pmod_small 1:/#.
-  rewrite nth_iota 1:/# /(\bits8) /= (W8.ext_eq _ W8.zero). move => x0 x0_bnd.
-    rewrite initE ifT 1:/# /=. have->: 0 <= i * 8 + x0 < 64 by smt().
-    rewrite andaE andTb get_out; smt(nth_iota).
-  smt().
-qed.
-
-lemma trail_word x i off _trail:
-  0 <= x =>
-  0 <= off =>
-  0 <= _trail =>
-  _trail < 256 =>
-  min 8 (off+x) <= i < min 8 (off + 1 + x) =>
-  W64.of_int _trail `<<<` 8 * (off + x) \bits8 nth witness (iota_ 0 8) i =
-  W8.of_int _trail.
-proof.
-  move => H0 H1 H2 H3 H4.
-  rewrite /W64.of_int !pmod_small 1:/#.
-  rewrite nth_iota 1:/# /(\bits8) /= (W8.ext_eq _ (W8.of_int _trail)). move => x0 x0_bnd.
-    rewrite initE ifT 1:/# /=. have->: 0 <= i * 8 + x0 < 64 by smt().
-    rewrite andaE andTb /W8.of_int pmod_small 1:/# !get_bits2w ..2:/#.
-    rewrite (int2bs_cat 8) 1:/# pdiv_small 1:/# nth_cat size_int2bs ifT /#.
-  smt().
-qed.
-
-lemma trail_simplify y x a:
-    0 <= x =>
-    0 <= a =>
-    W64.of_int (256 * y) `<<<` 8 * (a + x) = W64.of_int y `<<<` 8 * (a + 1 + x).
-proof.
-  move => H0 H1. have->: 256 = 2^8 by smt(). rewrite mulrC -shlMP 1:/# shlw_add /#.
-qed.
-
-
-lemma compose2u8 _buf pos x _cur _at _len _trail:
-  8 <= _len + x =>
-  0 <= _cur =>
-  0 <= _at =>
-  _cur <= _at =>
-  _at - _cur = x =>
-  x < 8 =>
-  6 <= x =>
-  0 <= pos =>
-  pos + 8 < _ASIZE =>
-u64bytes
-  (zeroextu64 (get16_direct (WA.init8 (ReadWriteArray.A."_.[_]" _buf)) pos) `<<<` 8 * x)
- = bytes_at 8 _cur _at (sub _buf pos _len ++ [W8.of_int _trail]).
-proof.
-  move => H0 H1 H2 H3 H4 H5 H6 H7 H8.
-  pose w0:= zeroextu64 (get16_direct (WA.init8 ("_.[_]" _buf)) pos) `<<<` 8 * x.
-  pose l1:= u64bytes w0.
-  pose l2:= bytes_at 8 _cur _at (sub _buf pos _len ++ [W8.of_int _trail]).
-    rewrite (eq_from_nth W8.zero l1 l2).
-    + rewrite size_to_list size_take 1:/# size_cat size_drop 1:/# size_nseq /#.
-    + rewrite size_to_list /l1 => i i_bnd.
-      rewrite /l2 /bytes_at nth_take..2:/# drop_cat_le nth_cat size_nseq lez_maxr 1:/#.
-      case(2 + x <= i) => i_max.
-      + rewrite /u64bytes (nth_map witness W8.zero) /iotared 1:size_iota 1:/# H3 /=.
-        rewrite (preu16_0s x 0 _ _ pos) ..3:/# !size_cat size_drop 1:/# size_mkseq.
-        rewrite size_nseq !lez_maxr ..4:/# ifT 1:/# nth_cat size_drop 1:/# size_nseq.
-        rewrite ifT 1:/# nth_drop ..2:/# nth_nseq /#.
-      case(i < x) => i_min.
-      + rewrite /u64bytes (nth_map witness W8.zero) /iotared 1:size_iota 1:/# H3 /=.
-        rewrite (posu16_0s x 0 _ _ pos) ..3:/# !size_cat size_drop 1:/# size_nseq.
-        rewrite size_mkseq ifT 1:/# nth_cat size_drop 1:/# size_nseq ifT 1:/#.
-        rewrite nth_drop ..2:/# nth_nseq /#.
-      + move: i_max i_min. rewrite -lezNgt lezNgt /= => i_max i_min.
-      + rewrite /u64bytes (nth_map witness W8.zero) /iotared 1:size_iota 1:/# H3 /=.
-        rewrite (u16_word x 0 _ _ pos) ..3:/# !size_cat size_drop 1:/# size_nseq.
-        rewrite size_mkseq ifT 1:/# nth_cat size_drop 1:/# size_nseq ifF 1:/#.
-        rewrite nth_cat nth_mkseq 1:/# size_mkseq ifT 1:/# !lez_maxr ..3:/# /(\bits8) /=.
-        rewrite (W8.ext_eq _ (_buf.[pos + (i - x)])). move => x0 x0_bnd.
-          rewrite initE ifT 1:/# /WA.init8 /get16_direct /pack2_t /=.
-          rewrite initE ifT 1:nth_iota ..2:/# /= initE ifT 1:nth_iota ..2:/# /=.
-          rewrite !nth_iota 1:/# initE ifT /#. smt().
-      smt().
-qed.
-
-
-lemma compose4u8 _buf _off _dlt _at _cur _len _trail:
-  4 <= _len =>
-  0 <= _cur =>
-  0 <= _at =>
-  _cur <= _at =>
-  _at - _cur < 8 =>
-  4 <= _at - _cur =>
-  0 <= _off + _dlt =>
-  _off + _dlt + 8 < _ASIZE =>
-u64bytes (zeroextu64 (get32_direct (WA.init8 (ReadWriteArray.A."_.[_]" _buf)) (_off + _dlt)) `<<<` 8 * (_at - _cur)) =
-bytes_at 8 _cur _at (sub _buf (_off + _dlt) _len ++ [W8.of_int _trail]).
-proof.
-  move => H0 H1 H2 H3 H4 H5 H6 H7.
-  pose l1:= u64bytes (zeroextu64 (get32_direct (WA.init8 ("_.[_]" _buf)) (_off + _dlt)) `<<<` 8 * (_at - _cur)).
-  pose l2:= bytes_at 8 _cur _at (sub _buf (_off + _dlt) _len ++ [W8.of_int _trail]).
-  rewrite (eq_from_nth W8.zero l1 l2).
-  + rewrite size_to_list size_take 1:/# size_cat size_drop 1:/# !size_cat size_mkseq /=.
-    rewrite !size_nseq !lez_maxr /#.
-  + rewrite size_to_list => i i_bnd.
-    rewrite nth_to_list_in 1:/# get32E /WA.init8 W4u8.Pack.init_of_list. 
-    rewrite (buf4_expand) ..2:/# W64.wlslE /(\bits8).
-    pose b:= (W4u8.Pack.of_list ([_buf.[_off + _dlt]; _buf.[_off + _dlt + 1]; _buf.[_off + _dlt + 2]; _buf.[_off + _dlt + 3]])).
-    rewrite /zeroextu64 /W64.of_int /W32.to_uint pmod_small.
-    rewrite bs2int_ge0 andaE andTb.
-    rewrite (ltr_trans (2^(size (JWord.W32.w2bits(pack4_t b))))).
-    + by rewrite bs2int_le2Xs.
-    + by rewrite size_w2bits.
-    rewrite (int2bs_cat 32 64) 1:/# divz_small.
-    rewrite bs2int_ge0 andaE andTb.
-    rewrite (ltr_le_trans (2^(size (w2bits (pack4_t b))))).
-    + by rewrite bs2int_le2Xs.
-    + by rewrite size_w2bits.
-    have{1}->: 32 = size (w2bits (pack4_t b)); first by rewrite size_w2bits.
-    rewrite bs2intK /W64.bits2w /=.
-    rewrite (W8.init_ext (fun j => (W64.init (fun j0 => (W64.init (nth false (w2bits (pack4_t b) ++ int2bs 32 0))).[j0-8*(_at-_cur)])).[i*8+j]) (fun j => (W64.init (nth false (w2bits (pack4_t b) ++ int2bs 32 0))).[i * 8 + j - 8 * (_at - _cur)])).
-    + move => x x_bnd /=.
-      rewrite W64.initE /= (W64.initE (nth false (w2bits (pack4_t b) ++ int2bs 32 0))) /#.
-    rewrite /l2 /bytes_at /sub nth_take ..2:/# drop_cat_le size_nseq ifT 1:/#.
-    rewrite !nth_cat !size_cat size_drop 1:/# size_nseq size_mkseq /=.
-    case(i < _at - _cur) => i_min.
-    + rewrite !ifT ..2:/# nth_drop ..2:/# nth_nseq 1:/#.
-      rewrite (W8.ext_eq _ W8.zero). move => x x_bnd.
-      rewrite W8.initE ifT 1:/# /= W64.initE /#. smt().
-    + rewrite ifT 1:/# ifF 1:/# ifT 1:/# nth_mkseq 1:/# !lez_maxr ..3:/# /=.
-      rewrite (W8.ext_eq _ (_buf.[_off + _dlt + (i - (_at - _cur))])). move => x x_bnd.
-      rewrite W8.initE ifT 1:/# /= W64.initE ifT 1:/# nth_cat size_w2bits ifT 1:/#.
-      rewrite get_w2bits /b /pack4_t W32.initE ifT 1:/# /= W4u8.Pack.get_of_list /#.
-      smt().
-    smt().
-qed.
-
-lemma compose6u8 _buf pos x _cur _at _len _trail:
-  6 <= _len =>
-  0 <= _cur =>
-  0 <= _at =>
-  _cur <= _at =>
-  _at - _cur = x =>
-  x < 4 =>
-  2 <= x =>
-  0 <= pos =>
-  pos + 8 < _ASIZE =>
-u64bytes
-  ((zeroextu64 (get32_direct (WA.init8 (ReadWriteArray.A."_.[_]" _buf)) pos) `<<<` 8*x) `|`
-   (zeroextu64 (get16_direct (WA.init8 (ReadWriteArray.A."_.[_]" _buf)) (pos + 4))
-    `<<<` 8 * (4 + x))) = bytes_at 8 _cur _at (sub _buf pos _len ++ [W8.of_int _trail]).
-proof.
-  move => H0 H1 H2 H3 H4 H5 H6 H7 H8.
-  pose w0:= zeroextu64 (get32_direct (WA.init8 ("_.[_]" _buf)) pos) `<<<` 8*x.
-  pose w1:= zeroextu64 (get16_direct (WA.init8 ("_.[_]" _buf)) (pos + 4)) `<<<` 8*(4+x).
-  pose l1:= u64bytes (w0 `|` w1).
-  pose l2:= bytes_at 8 _cur _at (sub _buf pos _len ++ [W8.of_int _trail]).
-    rewrite (eq_from_nth W8.zero l1 l2).
-    + rewrite size_to_list size_take 1:/# size_cat size_drop 1:/# size_nseq /#.
-    + rewrite size_to_list /l1 => i i_bnd.
-      rewrite /l2 /bytes_at nth_take ..2:/# drop_cat_le nth_cat size_nseq lez_maxr 1:/#.
-      case(6 + x <= i) => i_max.
-        rewrite /u64bytes (nth_map witness W8.zero) /iotared 1:size_iota 1:/# /=.
-        rewrite preu32_0s ..2:/# preu16_0s ..4:/#.
-      case(i < x) => i_min.
-      + rewrite /u64bytes (nth_map witness W8.zero) /iotared 1:size_iota 1:/# /=.
-        rewrite posu32_0s ..2:/# posu16_0s ..3:/# ifT ifT 1:/# 1:size_cat 1:size_drop 1:/#.
-        rewrite !size_cat size_nseq /sub size_mkseq /#. smt().
-        rewrite nth_cat size_drop 1:/# size_nseq ifT 1:/# nth_drop ..2:/# nth_nseq /#.
-      + move: i_max i_min. rewrite -lezNgt lezNgt /= => i_max i_min.
-      case(i < 4 + x) => u32.
-      + rewrite /u64bytes (nth_map witness W8.zero) /iotared 1:size_iota 1:/# /=.
-        rewrite u32_word ..2:/# posu16_0s ..3:/# ifT ifT 1:/# 1:size_cat.
-        rewrite !size_cat size_drop 1:/# /sub size_mkseq /#. smt().
-        rewrite !nth_cat size_drop 1:/# size_nseq ifF 1:/# size_mkseq ifT 1:/#.
-        rewrite nth_mkseq 1:/# orw0 /= !lez_maxr ..3:/# /(\bits8).
-        rewrite (W8.ext_eq _ (_buf.[pos + (i - x)])). move => x0 x0_bnd.
-          rewrite initE ifT 1:/# /WA.init8 /get32_direct /pack4_t /=.
-          rewrite initE ifT 1:nth_iota ..2:/# /= initE ifT 1:nth_iota ..2:/# /=.
-          rewrite !nth_iota 1:/# initE ifT /#. smt().
-      move: u32. rewrite -lezNgt => u16. 
-      + rewrite /u64bytes (nth_map witness W8.zero) /iotared 1:size_iota 1:/# /=.
-        rewrite preu32_0s ..2:/# u16_word ..3:/# ifT ifT 1:/# 1:size_cat.
-        rewrite !size_cat size_drop 1:/# /sub size_mkseq size_nseq /#. smt().
-        rewrite !nth_cat size_drop 1:/# size_nseq ifF 1:/# size_mkseq ifT 1:/#.
-        rewrite nth_mkseq 1:/# or0w /= !lez_maxr ..3:/# /(\bits8).
-        rewrite (W8.ext_eq _ (_buf.[pos + (i - x)])). move => x0 x0_bnd.
-          rewrite initE ifT 1:/# /WA.init8 /get16_direct /pack2_t /=.
-          rewrite initE ifT 1:nth_iota ..2:/# /= initE ifT 1:nth_iota ..2:/# /=.
-          rewrite !nth_iota 1:/# initE ifT /#. smt().
-      smt().
-qed.
-
-lemma compose8u8 _buf _off _dlt _at _cur _len _trail:
-  8 <= _len =>
-  0 <= _cur =>
-  0 <= _at =>
-  _cur <= _at =>
-  _at - _cur < 8 =>
-  0 <= _at - _cur =>
-  0 <= _off + _dlt =>
-  _off + _dlt + 8 < _ASIZE =>
-  u64bytes (get64_direct (WA.init8 (ReadWriteArray.A."_.[_]" _buf))
-                         (_off + _dlt) `<<<` 8 * (_at - _cur)) =
-bytes_at 8 _cur _at (sub _buf (_off + _dlt) _len ++ [W8.of_int _trail]).
-proof.
-  move => H0 H1 H2 H3 H4 H5 H6 H7.
-  pose l1:= u64bytes (get64_direct (WA.init8 ("_.[_]" _buf)) (_off + _dlt)
-            `<<<` 8*(_at - _cur)).
-  pose l2:= bytes_at 8 _cur _at (sub _buf (_off + _dlt) _len ++ [W8.of_int _trail]).
-    rewrite (eq_from_nth W8.zero l1 l2).
-    + rewrite size_to_list size_take 1:/# size_cat size_drop 1:/# size_nseq /#.
-    + rewrite size_to_list /l1 => i i_bnd.
-      rewrite /l2 /bytes_at nth_take ..2:/# drop_cat_le nth_cat size_nseq lez_maxr 1:/#.
-      case(i < _at - _cur) => i_min.
-        rewrite /u64bytes (nth_map witness W8.zero) /iotared 1:size_iota 1:/# /=.
-        rewrite posu64_0s ..2:/# ifT ifT 1:/#. rewrite !size_cat size_drop 1:/# size_mkseq.
-        rewrite size_nseq /#. smt().
-        rewrite nth_cat size_drop 1:/# size_nseq ifT 1:/# nth_drop ..2:/# nth_nseq /#.
-      + rewrite ifT ifT 1:/#. rewrite !size_cat size_drop 1:/# size_mkseq size_nseq /#.
-        smt(). rewrite nth_to_list /get64_direct /pack8_t nth_cat size_drop 1:/# size_nseq.
-        rewrite ifF 1:/# !nth_cat size_mkseq ifT 1:/# nth_mkseq 1:/# /=.
-        rewrite (W8.ext_eq _ (_buf.[_off + _dlt + (i - max 0 (max 0 _at - _cur))])).
-        move => x x_bnd. rewrite /(\bits8) initE ifT 1:/# /=.
-        have->: 0 <= i * 8 + x < 64 by smt(). rewrite andaE andTb initE ifT 1:/# /=.
-        rewrite initE ifT 1:/# /= initE ifT /#. smt().
-      smt().
-qed.
-
-lemma compose_trail (_buf: W8.t A.t) pos _cur _at _trail:
-  0 <= _cur =>
-  0 <= _at =>
-  0 <= _trail =>
-  _trail < 256 =>
-  _cur <= _at =>
-  _at - _cur < 8 =>
-  0 <= _at - _cur =>
-  0 <= pos =>
-  pos + 8 < _ASIZE =>
- u64bytes (W64.of_int _trail `<<<` 8 * (_at - _cur)) =
- bytes_at 8 _cur _at (sub _buf pos 0 ++ [W8.of_int _trail]).
-proof.
-  move => H0 H1 H2 H3 H4 H5 H6 H7 H8.
-  pose w0:= W64.of_int _trail `<<<` 8 * (_at - _cur).
-  pose l1:= u64bytes w0.
-  pose l2:= bytes_at 8 _cur _at (sub _buf pos 0 ++ [W8.of_int _trail]).
-    rewrite (eq_from_nth W8.zero l1 l2).
-    + rewrite size_to_list size_take 1:/# size_cat size_drop 1:/# size_nseq /#.
-    + rewrite size_to_list /l1 => i i_bnd.
-      rewrite /l2 /bytes_at nth_take ..2:/# drop_cat_le nth_cat size_nseq lez_maxr 1:/#.
-      case(1 + (_at - _cur) <= i) => i_max.
-      + rewrite /u64bytes (nth_map witness W8.zero) /iotared 1:size_iota 1:/# /=.
-        rewrite (preTrail_0s (_at-_cur) 0 i) ..5:/# ifF ifT 1:/#.
-        rewrite !size_cat size_drop 1:/# size_mkseq size_nseq /#.
-        smt(). rewrite !size_cat size_drop 1:/# size_nseq size_mkseq /= nth_nseq /#.
-      case(i < (_at-_cur)) => i_min.
-      + rewrite /u64bytes (nth_map witness W8.zero) /iotared 1:size_iota 1:/# /=.
-        rewrite (posTrail_0s (_at-_cur) i 0)..5:/# ifT ifT 1:/# 1:size_cat ?size_drop 1:/#.
-        rewrite !size_cat size_nseq size_mkseq /#. smt().
-        rewrite nth_cat size_drop 1:/# size_nseq ifT 1:/# nth_drop ..2:/# nth_nseq /#.
-      + move: i_max i_min. rewrite -lezNgt lezNgt /= => i_max i_min.
-      + rewrite /u64bytes (nth_map witness W8.zero) /iotared 1:size_iota 1:/# /=.
-        rewrite (trail_word (_at-_cur) i 0) ..5:/# !ifT 1:/#.
-        rewrite !size_cat size_drop 1:/# size_mkseq size_nseq /#. smt().
-        rewrite !nth_cat size_drop 1:/# size_nseq ifF 1:/# size_mkseq ifF 1:/# /#.
-      smt().
-qed.
-
-lemma compose1u8_trail _buf pos x _cur _at _trail:
-  0 <= _cur =>
-  0 <= _at =>
-  0 <= _trail =>
-  _trail < 256 =>
-  _cur <= _at =>
-  _at - _cur = x =>
-  x < 8 =>
-  0 <= x =>
-  0 <= pos =>
-  pos + 8 < _ASIZE =>
-u64bytes
-  (zeroextu64 (get8 (WA.init8 (ReadWriteArray.A."_.[_]" _buf)) pos)
-    `|` W64.of_int (256 * _trail) `<<<` 8 * x)
- = bytes_at 8 _cur _at (sub _buf pos 1 ++ [W8.of_int _trail]).
-proof.
-  move => H0 H1 H2 H3 H4 H5 H6 H7 H8 H9. rewrite -shlw_or (trail_simplify _ x 0) ..2:/# /=.
-  pose w0:= zeroextu64 (get8 (WA.init8 ("_.[_]" _buf)) pos) `<<<` 8 * x.
-  pose w1:= W64.of_int (_trail) `<<<` 8 * (1 + x).
-  pose l1:= u64bytes (w0 `|` w1).
-  pose l2:= bytes_at 8 _cur _at (sub _buf pos 1 ++ [W8.of_int _trail]).
-    rewrite (eq_from_nth W8.zero l1 l2).
-    + rewrite size_to_list size_take 1:/# size_cat size_drop 1:/# size_nseq /#.
-    + rewrite size_to_list /l1 => i i_bnd.
-      rewrite /l2 /bytes_at nth_take ..2:/# drop_cat_le nth_cat size_nseq lez_maxr 1:/#.
-      case(2 + x <= i) => i_max.
-      + rewrite /u64bytes (nth_map witness W8.zero) /iotared 1:size_iota 1:/# /=.
-        rewrite (preu8_0s x 0 _ _ pos) ..3:/# preTrail_0s ..5:/#.
-        rewrite ifF ifT 1:/#. rewrite !size_cat size_drop 1:/# size_mkseq size_nseq /#.
-        smt(). rewrite !size_cat size_drop 1:/# size_nseq size_mkseq /= nth_nseq /#.
-      case(i < x) => i_min.
-      + rewrite /u64bytes (nth_map witness W8.zero) /iotared 1:size_iota 1:/# /=.
-        rewrite (posu8_0s x 0 _ _ pos) ..3:/# posTrail_0s ..5:/#.
-        rewrite ifT ifT 1:/# 1:size_cat 1:size_drop 1:/#.
-        rewrite !size_cat size_nseq size_mkseq /#. smt().
-        rewrite nth_cat size_drop 1:/# size_nseq ifT 1:/# nth_drop ..2:/# nth_nseq /#.
-      + move: i_max i_min. rewrite -lezNgt lezNgt /= => i_max i_min.
-      case(i < 1 + x) => u8.
-      + rewrite /u64bytes (nth_map witness W8.zero) /iotared 1:size_iota 1:/# /=.
-        rewrite (u8_word x 0 _ _ pos) ..3:/# posTrail_0s ..5:/#.
-        rewrite !ifT 1:/#. rewrite !size_cat size_drop 1:/# /sub size_mkseq size_nseq /#.
-        smt(). rewrite !nth_cat size_drop 1:/# size_nseq ifF 1:/# size_mkseq ifT 1:/#.
-        rewrite nth_mkseq 1:/# orw0 /= !lez_maxr ..3:/# /(\bits8) ifT 1:/# /get8 initE /#.
-      move: u8. rewrite -lezNgt => over_u8.
-      + rewrite /u64bytes (nth_map witness W8.zero) /iotared 1:size_iota 1:/# /=.
-        rewrite (preu8_0s x 0 _ _ pos) ..3:/# trail_word ..5:/#.
-        rewrite !ifT 1:/#. rewrite !size_cat size_drop 1:/# size_mkseq size_nseq /#. smt().
-        rewrite !nth_cat size_drop 1:/# size_nseq ifF 1:/# size_mkseq ifF 1:/# !or0w /#.
-      smt().
-qed.
-
-lemma compose2u8_trail _buf pos x _cur _at _trail:
-  0 <= _cur =>
-  0 <= _at =>
-  0 <= _trail =>
-  _trail < 256 =>
-  _cur <= _at =>
-  _at - _cur = x =>
-  x < 8 =>
-  0 <= x =>
-  0 <= pos =>
-  pos + 8 < _ASIZE =>
-u64bytes
-  ((zeroextu64 (get16_direct (WA.init8 (ReadWriteArray.A."_.[_]" _buf)) pos)
-    `<<<` 8 * x) `|` (W64.of_int (_trail) `<<<` 8 * (2 + x)))
- = bytes_at 8 _cur _at (sub _buf pos 2 ++ [W8.of_int _trail]).
-proof.
-  move => H0 H1 H2 H3 H4 H5 H6 H7 H8 H9.
-  pose w0:= zeroextu64 (get16_direct (WA.init8 ("_.[_]" _buf)) pos) `<<<` 8 * x.
-  pose w1:= W64.of_int (_trail) `<<<` 8 * (2 + x).
-  pose l1:= u64bytes (w0 `|` w1).
-  pose l2:= bytes_at 8 _cur _at (sub _buf pos 2 ++ [W8.of_int _trail]).
-    rewrite (eq_from_nth W8.zero l1 l2).
-    + rewrite size_to_list size_take 1:/# size_cat size_drop 1:/# size_nseq /#.
-    + rewrite size_to_list /l1 => i i_bnd.
-      rewrite /l2 /bytes_at nth_take ..2:/# drop_cat_le nth_cat size_nseq lez_maxr 1:/#.
-      case(3 + x <= i) => i_max.
-      + rewrite /u64bytes (nth_map witness W8.zero) /iotared 1:size_iota 1:/# /=.
-        rewrite (preu16_0s x 0 _ _ pos) ..3:/# preTrail_0s ..5:/#.
-        rewrite ifF ifT 1:/#. rewrite !size_cat size_drop 1:/# size_mkseq size_nseq /#.
-        smt(). rewrite !size_cat size_drop 1:/# size_nseq size_mkseq /= nth_nseq /#.
-      case(i < x) => i_min.
-      + rewrite /u64bytes (nth_map witness W8.zero) /iotared 1:size_iota 1:/# /=.
-        rewrite (posu16_0s x 0 _ _ pos) ..3:/# posTrail_0s ..5:/#.
-        rewrite ifT ifT 1:/# 1:size_cat 1:size_drop 1:/#.
-        rewrite !size_cat size_nseq size_mkseq /#. smt().
-        rewrite nth_cat size_drop 1:/# size_nseq ifT 1:/# nth_drop ..2:/# nth_nseq /#.
-      + move: i_max i_min. rewrite -lezNgt lezNgt /= => i_max i_min.
-      case(i < 2 + x) => u16.
-      + rewrite /u64bytes (nth_map witness W8.zero) /iotared 1:size_iota 1:/# /=.
-        rewrite (u16_word x 0 _ _ pos) ..3:/# posTrail_0s ..5:/#.
-        rewrite !ifT 1:/#. rewrite !size_cat size_drop 1:/# /sub size_mkseq size_nseq /#.
-        smt(). rewrite !nth_cat size_drop 1:/# size_nseq ifF 1:/# size_mkseq ifT 1:/#.
-        rewrite nth_mkseq 1:/# orw0 /= !lez_maxr ..3:/# /(\bits8).
-        rewrite (W8.ext_eq _ (_buf.[pos + (i - x)])). move => x0 x0_bnd.
-          rewrite initE ifT 1:/# /WA.init8 /get16_direct /pack2_t /=.
-          rewrite initE ifT 1:nth_iota ..2:/# /= initE ifT 1:nth_iota ..2:/# /=.
-          rewrite !nth_iota 1:/# initE ifT /#. smt().
-      move: u16. rewrite -lezNgt => over_u16.
-      + rewrite /u64bytes (nth_map witness W8.zero) /iotared 1:size_iota 1:/# /=.
-        rewrite (preu16_0s x 0 _ _ pos) ..3:/# trail_word ..5:/#.
-        rewrite !ifT 1:/#. rewrite !size_cat size_drop 1:/# size_mkseq size_nseq /#. smt().
-        rewrite !nth_cat size_drop 1:/# size_nseq ifF 1:/# size_mkseq ifF 1:/# !or0w /#.
-      smt().
-qed.
-
-lemma compose3u8_trail _buf pos x _cur _at _trail:
-  0 <= _cur =>
-  0 <= _at =>
-  0 <= _trail =>
-  _trail < 256 =>
-  _cur <= _at =>
-  _at - _cur = x =>
-  x <= 5 =>
-  0 <= x =>
-  0 <= pos =>
-  pos + 8 < _ASIZE =>
-u64bytes
-  ((zeroextu64 (get16_direct (WA.init8 (ReadWriteArray.A."_.[_]" _buf)) pos)
-    `<<<` 8 * x) `|`
-   (zeroextu64 (get8 (WA.init8 (ReadWriteArray.A."_.[_]" _buf)) (pos + 2)) `|`
-   W64.of_int (256 * _trail) `<<<` 8 * (2 + x)))
- = bytes_at 8 _cur _at (sub _buf pos 3 ++ [W8.of_int _trail]).
-proof.
-  move => H0 H1 H2 H3 H4 H5 H6 H7 H8 H9. rewrite -shlw_or trail_simplify ..2:/# /=.
-  pose w0:= zeroextu64 (get16_direct (WA.init8 ("_.[_]" _buf)) pos) `<<<` 8 * x.
-  pose w1:= zeroextu64 (get8 (WA.init8 ("_.[_]" _buf)) (pos + 2)) `<<<` 8 * (2 + x).
-  pose w2:= W64.of_int (_trail) `<<<` 8 * (3 + x).
-  pose l1:= u64bytes (w0 `|` (w1 `|` w2)).
-  pose l2:= bytes_at 8 _cur _at (sub _buf pos 3 ++ [W8.of_int _trail]).
-    rewrite (eq_from_nth W8.zero l1 l2).
-    + rewrite size_to_list size_take 1:/# size_cat size_drop 1:/# size_nseq /#.
-    + rewrite size_to_list /l1 => i i_bnd.
-      rewrite /l2 /bytes_at nth_take ..2:/# drop_cat_le nth_cat size_nseq lez_maxr 1:/#.
-      case(4 + x <= i) => i_max.
-      + rewrite /u64bytes (nth_map witness W8.zero) /iotared 1:size_iota 1:/# /=.
-        rewrite (preu16_0s x 0 _ _ pos) ..3:/# preu8_0s ..3:/# preTrail_0s ..5:/#.
-        rewrite ifF ifT 1:/#. rewrite !size_cat size_drop 1:/# size_mkseq size_nseq /#.
-        smt(). rewrite !size_cat size_drop 1:/# size_nseq size_mkseq /= nth_nseq /#.
-      case(i < x) => i_min.
-      + rewrite /u64bytes (nth_map witness W8.zero) /iotared 1:size_iota 1:/# /=.
-        rewrite (posu16_0s x 0 _ _ pos) ..3:/# posu8_0s ..3:/# posTrail_0s ..5:/#.
-        rewrite ifT ifT 1:/# 1:size_cat 1:size_drop 1:/#.
-        rewrite !size_cat size_nseq size_mkseq /#. smt().
-        rewrite nth_cat size_drop 1:/# size_nseq ifT 1:/# nth_drop ..2:/# nth_nseq /#.
-      + move: i_max i_min. rewrite -lezNgt lezNgt /= => i_max i_min.
-      case(i < 2 + x) => u16.
-      + rewrite /u64bytes (nth_map witness W8.zero) /iotared 1:size_iota 1:/# /=.
-        rewrite (u16_word x 0 _ _ pos) ..3:/# posu8_0s ..3:/# posTrail_0s ..5:/#.
-        rewrite !ifT 1:/#. rewrite !size_cat size_drop 1:/# /sub size_mkseq size_nseq /#.
-        smt(). rewrite !nth_cat size_drop 1:/# size_nseq ifF 1:/# size_mkseq ifT 1:/#.
-        rewrite nth_mkseq 1:/# orw0 /= !lez_maxr ..3:/# /(\bits8).
-        rewrite (W8.ext_eq _ (_buf.[pos + (i - x)])). move => x0 x0_bnd.
-          rewrite initE ifT 1:/# /WA.init8 /get16_direct /pack2_t /=.
-          rewrite initE ifT 1:nth_iota ..2:/# /= initE ifT 1:nth_iota ..2:/# /=.
-          rewrite !nth_iota 1:/# initE ifT /#. smt().
-      move: u16. rewrite -lezNgt => over_u16.
-      case(i < 3 + (_at - _cur)) => u8.
-      + rewrite /u64bytes (nth_map witness W8.zero) /iotared 1:size_iota 1:/# /=.
-        rewrite (preu16_0s x 0 _ _ pos) ..3:/# u8_word ..3:/# posTrail_0s ..5:/#.
-        rewrite !ifT 1:/#. rewrite !size_cat size_drop 1:/# size_mkseq size_nseq /#. smt().
-        rewrite !nth_cat size_drop 1:/# size_nseq ifF 1:/# size_mkseq ifT 1:/#.
-        rewrite nth_mkseq 1:/# or0w /= !lez_maxr ..3:/# /(\bits8) ifT 1:/#.
-        rewrite (W8.ext_eq _ (_buf.[pos + (i - x)])). move => x0 x0_bnd.
-          rewrite /get8 initE ifT /#. smt().
-      + rewrite /u64bytes (nth_map witness W8.zero) /iotared 1:size_iota 1:/# /=.
-        rewrite (preu16_0s x 0 _ _ pos) ..3:/# preu8_0s ..3:/# trail_word ..5:/#.
-        rewrite !ifT 1:/#. rewrite !size_cat size_drop 1:/# size_mkseq size_nseq /#. smt().
-        rewrite !nth_cat size_drop 1:/# size_nseq ifF 1:/# size_mkseq ifF 1:/# !or0w /#.
-      smt().
-qed.
-
-lemma compose4u8_trail _buf pos x _cur _at _trail:
-  0 <= _cur =>
-  0 <= _at =>
-  0 <= _trail =>
-  _trail < 256 =>
-  _cur <= _at =>
-  _at - _cur = x =>
-  x < 4 =>
-  0 <= x =>
-  0 <= pos =>
-  pos + 8 < _ASIZE =>
-  u64bytes
-    ((zeroextu64 (get32_direct (WA.init8 (ReadWriteArray.A."_.[_]" _buf)) pos) `<<<` 8 * x)
-    `|`
-   (W64.of_int _trail `<<<` 8 * (4 + x))) =
-bytes_at 8 _cur _at (sub _buf pos 4 ++ [W8.of_int _trail]).
-proof.
-  move => H0 H1 H2 H3 H4 H5 H6 H7 H8 H9.
-  pose w0:= zeroextu64 (get32_direct (WA.init8 ("_.[_]" _buf)) pos) `<<<` 8 * x.
-  pose w1:= W64.of_int _trail `<<<` 8 * (4 + x).
-  pose l1:= u64bytes (w0 `|` w1).
-  pose l2:= bytes_at 8 _cur _at (sub _buf pos 4 ++ [W8.of_int _trail]).
-    rewrite (eq_from_nth W8.zero l1 l2).
-    + rewrite size_to_list size_take 1:/# size_cat size_drop 1:/# size_nseq /#.
-    + rewrite size_to_list /l1 => i i_bnd.
-      rewrite /l2 /bytes_at nth_take ..2:/# drop_cat_le nth_cat size_nseq lez_maxr 1:/#.
-      case(5 + x <= i) => i_max.
-      + rewrite /u64bytes (nth_map witness W8.zero) /iotared 1:size_iota 1:/# /=.
-        rewrite preu32_0s ..2:/# preTrail_0s ..5:/#.
-        rewrite ifF ifT 1:/#. rewrite !size_cat size_drop 1:/# size_mkseq size_nseq /#.
-        smt(). rewrite nth_nseq. rewrite !size_cat size_drop 1:/# size_nseq size_mkseq /#.
-        smt().
-      case(i < x) => i_min.
-      + rewrite /u64bytes (nth_map witness W8.zero) /iotared 1:size_iota 1:/# /=.
-        rewrite posu32_0s..2:/# posTrail_0s..5:/# ifT ifT 1:/# 1:size_cat 1:size_drop 1:/#.
-        rewrite !size_cat size_nseq size_mkseq /#. smt().
-        rewrite nth_cat size_drop 1:/# size_nseq ifT 1:/# nth_drop ..2:/# nth_nseq /#.
-      + move: i_max i_min. rewrite -lezNgt lezNgt /= => i_max i_min.
-      case(i < 4 + x) => u32.
-      + rewrite /u64bytes (nth_map witness W8.zero) /iotared 1:size_iota 1:/# /=.
-        rewrite u32_word ..2:/# posTrail_0s ..5:/# !ifT 1:/#.
-        rewrite !size_cat size_drop 1:/# /sub size_mkseq size_nseq /#.
-        smt().
-        rewrite !nth_cat size_drop 1:/# size_nseq ifF 1:/# size_mkseq ifT 1:/#.
-        rewrite nth_mkseq 1:/# orw0 /= !lez_maxr ..3:/# /(\bits8).
-        rewrite (W8.ext_eq _ (_buf.[pos + (i - x)])). move => x0 x0_bnd.
-          rewrite initE ifT 1:/# /WA.init8 /get32_direct /pack4_t /=. 
-          rewrite initE ifT 1:nth_iota ..2:/# /= initE ifT 1:nth_iota ..2:/# /=.
-          rewrite !nth_iota 1:/# initE ifT /#. smt().
-      move: u32. rewrite -lezNgt => over_u32.
-      case(i < 5 + x) => trail.
-      + rewrite /u64bytes (nth_map witness W8.zero) /iotared 1:size_iota 1:/# /=.
-        rewrite preu32_0s ..2:/# trail_word ..5:/# !ifT 1:/#.
-        rewrite !size_cat size_drop 1:/# size_mkseq size_nseq /#. smt().
-        rewrite !nth_cat size_drop 1:/# size_nseq size_mkseq !ifF /#. smt().
-      smt().
-qed.
-
-
-lemma compose5u8_trail _buf pos x _cur _at _trail:
-  0 <= _cur =>
-  0 <= _at =>
-  0 <= _trail =>
-  _trail < 256 =>
-  _cur <= _at =>
-  _at - _cur = x =>
-  x < 4 =>
-  0 <= x =>
-  0 <= pos =>
-  pos + 8 < _ASIZE =>
-  u64bytes
-    ((zeroextu64 (get32_direct (WA.init8 (ReadWriteArray.A."_.[_]" _buf)) pos)
-      `<<<` 8 * x) `|`
-     ((zeroextu64 (get8 (WA.init8 (ReadWriteArray.A."_.[_]" _buf)) (pos + 4))
-       `<<<` 8 * (4+x)) `|` (W64.of_int _trail `<<<` 8 * (5 + x)))) =
-  bytes_at 8 _cur _at (sub _buf pos 5 ++ [W8.of_int _trail]).
-proof.
-  move => H0 H1 H2 H3 H4 H5 H6 H7 H8 H9.
-  pose w0:= zeroextu64 (get32_direct (WA.init8 ("_.[_]" _buf)) pos) `<<<` 8 * x.
-  pose w1:= zeroextu64 (get8_direct (WA.init8 ("_.[_]" _buf)) (pos + 4)) `<<<` 8 * (4 + x).
-  pose w2:= W64.of_int _trail `<<<` 8 * (5 + x).
-  pose l1:= u64bytes (w0 `|` (w1 `|` w2)).
-  pose l2:= bytes_at 8 _cur _at (sub _buf pos 5 ++ [W8.of_int _trail]).
-    rewrite (eq_from_nth W8.zero l1 l2).
-    + rewrite size_to_list size_take 1:/# size_cat size_drop 1:/# size_nseq /#.
-    + rewrite size_to_list /l1 => i i_bnd.
-      rewrite /l2 /bytes_at nth_take ..2:/# drop_cat_le nth_cat size_nseq lez_maxr 1:/#.
-      case(6 + x <= i) => i_max.
-      + rewrite /u64bytes (nth_map witness W8.zero) /iotared 1:size_iota 1:/# /=.
-        rewrite preu32_0s ..2:/# preu8_0s ..3:/# preTrail_0s ..5:/#.
-        rewrite ifF ifT 1:/#. rewrite !size_cat size_drop 1:/# size_mkseq size_nseq /#.
-        smt(). rewrite nth_nseq. rewrite !size_cat size_drop 1:/# size_nseq size_mkseq /#.
-        smt().
-      case(i < x) => i_min.
-      + rewrite /u64bytes (nth_map witness W8.zero) /iotared 1:size_iota 1:/# /=.
-        rewrite posu32_0s ..2:/# posu8_0s ..3:/# posTrail_0s ..5:/#.
-        rewrite ifT ifT 1:/# 1:size_cat 1:size_drop 1:/#.
-        rewrite !size_cat size_nseq size_mkseq /#. smt().
-        rewrite nth_cat size_drop 1:/# size_nseq ifT 1:/# nth_drop ..2:/# nth_nseq /#.
-      + move: i_max i_min. rewrite -lezNgt lezNgt /= => i_max i_min.
-      case(i < 4 + (_at - _cur)) => u32.
-      + rewrite /u64bytes (nth_map witness W8.zero) /iotared 1:size_iota 1:/# /=.
-        rewrite u32_word ..2:/# posu8_0s ..3:/# posTrail_0s ..5:/#.
-        rewrite !ifT 1:/#. rewrite !size_cat size_drop 1:/# /sub size_mkseq size_nseq /#.
-        smt().
-        rewrite !nth_cat size_drop 1:/# size_nseq ifF 1:/# size_mkseq ifT 1:/#.
-        rewrite nth_mkseq 1:/# orw0 /= !lez_maxr ..3:/# /(\bits8).
-        rewrite (W8.ext_eq _ (_buf.[pos + (i - x)])). move => x0 x0_bnd.
-          rewrite initE ifT 1:/# /WA.init8 /get32_direct /pack4_t /=. 
-          rewrite initE ifT 1:nth_iota ..2:/# /= initE ifT 1:nth_iota ..2:/# /=.
-          rewrite !nth_iota 1:/# initE ifT /#. smt().
-      move: u32. rewrite -lezNgt => over_u32.
-      case(i < 5 + (_at - _cur)) => u8.
-      + rewrite /u64bytes (nth_map witness W8.zero) /iotared 1:size_iota 1:/# /=.
-        rewrite preu32_0s ..2:/# u8_word ..3:/# posTrail_0s ..5:/#.
-        rewrite !ifT 1:/#. rewrite !size_cat size_drop 1:/# size_mkseq size_nseq /#. smt().
-        rewrite !nth_cat size_drop 1:/# size_nseq ifF 1:/# size_mkseq ifT 1:/#.
-        rewrite nth_mkseq 1:/# or0w /= !lez_maxr ..3:/# /(\bits8) ifT 1:/#.
-        rewrite (W8.ext_eq _ (_buf.[pos + (i - x)])). move => x0 x0_bnd.
-          rewrite /get8 initE ifT 1:/# /WA.init8 /get16_direct /pack2_t /#. smt().
-      + rewrite /u64bytes (nth_map witness W8.zero) /iotared 1:size_iota 1:/# /=.
-        rewrite preu32_0s ..2:/# preu8_0s ..3:/# trail_word ..5:/#.
-        rewrite !ifT 1:/#. rewrite !size_cat size_drop 1:/# size_mkseq size_nseq /#. smt().
-        rewrite !nth_cat size_drop 1:/# size_nseq size_mkseq !ifF /#.
-      smt().
-qed.
-
-
-lemma compose6u8_trail _buf pos x _cur _at _trail:
-  0 <= _cur =>
-  0 <= _at =>
-  0 <= _trail =>
-  _trail < 256 =>
-  _cur <= _at =>
-  _at - _cur = x =>
-  0 <= x =>
-  x < 2 =>
-  0 <= pos =>
-  pos + 8 < _ASIZE =>
-u64bytes
-  ((zeroextu64 (get32_direct (WA.init8 (ReadWriteArray.A."_.[_]" _buf)) pos) `<<<` 8*x) `|`
-   (zeroextu64 (get16_direct (WA.init8 (ReadWriteArray.A."_.[_]" _buf)) (pos + 4))
-    `<<<` 8 * (4 + x)) `|`
-   (W64.of_int (_trail) `<<<` 8 * (6 + x)))
- = bytes_at 8 _cur _at (sub _buf pos 6 ++ [W8.of_int _trail]).
-proof.
-  move => H0 H1 H3 H4 H5 H6 H7 H8 H9 H10.
-  pose w0:= zeroextu64 (get32_direct (WA.init8 ("_.[_]" _buf)) pos) `<<<` 8 * x.
-  pose w1:= zeroextu64 (get16_direct (WA.init8 ("_.[_]" _buf)) (pos+ 4)) `<<<` 8 * (4 + x).
-  pose w2:= W64.of_int _trail `<<<` 8 * (6 + x).
-  pose l1:= u64bytes (w0 `|` w1 `|` w2).
-  pose l2:= bytes_at 8 _cur _at (sub _buf pos 6 ++ [W8.of_int _trail]).
-    rewrite (eq_from_nth W8.zero l1 l2).
-    + rewrite size_to_list size_take 1:/# size_cat size_drop 1:/# size_nseq /#.
-    + rewrite size_to_list /l1 => i i_bnd.
-      rewrite /l2 /bytes_at nth_take ..2:/# drop_cat_le nth_cat size_nseq lez_maxr 1:/#.
-      case(7 + x <= i) => i_max.
-      + rewrite /u64bytes (nth_map witness W8.zero) /iotared 1:size_iota 1:/# /=.
-        rewrite preu32_0s ..2:/# preu16_0s ..3:/# preTrail_0s ..5:/#.
-        rewrite ifF ifT 1:/#. rewrite !size_cat size_drop 1:/# size_mkseq size_nseq /#.
-        smt(). rewrite nth_nseq. rewrite !size_cat size_drop 1:/# size_nseq size_mkseq /#.
-        smt().
-      case(i < x) => i_min.
-      + rewrite /u64bytes (nth_map witness W8.zero) /iotared 1:size_iota 1:/# /=.
-        rewrite posu32_0s ..2:/# posu16_0s ..3:/# posTrail_0s ..5:/#.
-        rewrite ifT ifT 1:/# 1:size_cat 1:size_drop 1:/#.
-        rewrite !size_cat size_nseq size_mkseq /#. smt().
-        rewrite nth_cat size_drop 1:/# size_nseq ifT 1:/# nth_drop ..2:/# nth_nseq /#.
-      + move: i_max i_min. rewrite -lezNgt lezNgt /= => i_max i_min.
-      case(i < 4 + x) => u32.
-      + rewrite /u64bytes (nth_map witness W8.zero) /iotared 1:size_iota 1:/# /=.
-        rewrite u32_word ..2:/# posu16_0s ..3:/# posTrail_0s ..5:/#.
-        rewrite !ifT 1:/#. rewrite !size_cat size_drop 1:/# /sub size_mkseq /#. smt().
-        rewrite !nth_cat size_drop 1:/# size_nseq ifF 1:/# size_mkseq ifT 1:/#.
-        rewrite nth_mkseq 1:/# orw0 /= !lez_maxr ..3:/# /(\bits8).
-        rewrite (W8.ext_eq _ (_buf.[pos + (i - x)])). move => x0 x0_bnd.
-          rewrite initE ifT 1:/# /WA.init8 /get32_direct /pack4_t /=.
-          rewrite initE ifT 1:nth_iota ..2:/# /= initE ifT 1:nth_iota ..2:/# /=.
-          rewrite !nth_iota 1:/# initE ifT /#. smt().
-      move: u32. rewrite -lezNgt => over_u32.
-      case(i < 6 + x) => u16.
-      + rewrite /u64bytes (nth_map witness W8.zero) /iotared 1:size_iota 1:/# /=.
-        rewrite preu32_0s ..2:/# u16_word ..3:/#  posTrail_0s ..5:/#.
-        rewrite !ifT 1:/#. rewrite !size_cat size_drop 1:/# size_mkseq size_nseq /#. smt().
-        rewrite !nth_cat size_drop 1:/# size_nseq ifF 1:/# size_mkseq ifT 1:/#.
-        rewrite nth_mkseq 1:/# or0w /= !lez_maxr ..3:/# /(\bits8).
-        rewrite (W8.ext_eq _ (_buf.[pos + (i - x)])). move => x0 x0_bnd.
-          rewrite initE ifT 1:/# /WA.init8 /get16_direct /pack2_t /=.
-          rewrite initE ifT 1:nth_iota ..2:/# /= initE ifT 1:nth_iota ..2:/# /=.
-          rewrite !nth_iota 1:/# initE ifT /#. smt().
-      + rewrite /u64bytes (nth_map witness W8.zero) /iotared 1:size_iota 1:/# /=.
-        rewrite preu32_0s ..2:/# preu16_0s ..3:/# trail_word ..5:/#.
-        rewrite !ifT 1:/#. rewrite !size_cat size_drop 1:/# size_mkseq size_nseq /#. smt().
-        rewrite !nth_cat size_drop 1:/# size_nseq size_mkseq ifF 1:/# !or0w /#.
-      smt().
-qed.
-
-lemma compose7u8_trail _buf pos x _cur _at _trail:
-  0 <= _cur =>
-  0 <= _at =>
-  0 <= _trail =>
-  _trail < 256 =>
-  _cur <= _at =>
-  _at - _cur = x =>
-  x < 4 =>
-  0 <= x =>
-  0 <= pos =>
-  pos + 8 < _ASIZE =>
-u64bytes
-  ((zeroextu64 (get32_direct (WA.init8 (ReadWriteArray.A."_.[_]" _buf)) pos) `<<<` 8*x) `|`
-   (zeroextu64 (get16_direct (WA.init8 (ReadWriteArray.A."_.[_]" _buf)) (pos + 4))
-    `<<<` 8 * (4 + x)) `|`
-   (zeroextu64 (get8 (WA.init8 (ReadWriteArray.A."_.[_]" _buf)) (pos + 6)) `|`
-   W64.of_int (256 * _trail) `<<<` 8 * (6 + x)))
- = bytes_at 8 _cur _at (sub _buf pos 7 ++ [W8.of_int _trail]).
-proof.
-  move => H0 H1 H2 H3 H4 H5 H6 H7 H8 H9. rewrite -shlw_or trail_simplify ..2:/# /=.
-  pose w0:= zeroextu64 (get32_direct (WA.init8 ("_.[_]" _buf)) pos) `<<<` 8 * x.
-  pose w1:= zeroextu64 (get16_direct (WA.init8 ("_.[_]" _buf)) (pos+ 4)) `<<<` 8 * (4 + x).
-  pose w2:= zeroextu64 (get8 (WA.init8 ("_.[_]" _buf)) (pos + 6)) `<<<` 8 * (6 + x).
-  pose w3:= W64.of_int (_trail) `<<<` 8 * (7 + x).
-  pose l1:= u64bytes (w0 `|` w1 `|` (w2 `|` w3)).
-  pose l2:= bytes_at 8 _cur _at (sub _buf pos 7 ++ [W8.of_int _trail]).
-    rewrite (eq_from_nth W8.zero l1 l2).
-    + rewrite size_to_list size_take 1:/# size_cat size_drop 1:/# size_nseq /#.
-    + rewrite size_to_list /l1 => i i_bnd.
-      rewrite /l2 /bytes_at nth_take ..2:/# drop_cat_le nth_cat size_nseq lez_maxr 1:/#.
-      case(7 + x <= i) => i_max.
-      + rewrite /u64bytes (nth_map witness W8.zero) /iotared 1:size_iota 1:/# /=.
-        rewrite preu32_0s ..2:/# preu16_0s ..3:/# preu8_0s ..3:/# trail_word ..5:/#.
-        rewrite !ifT 1:/#. rewrite !size_cat size_drop 1:/# size_mkseq /#. smt().
-        rewrite nth_cat nth_drop ..2:/# nth_cat size_mkseq size_drop 1:/# size_nseq.
-        rewrite !ifF /#.
-      case(i < x) => i_min.
-      + rewrite /u64bytes (nth_map witness W8.zero) /iotared 1:size_iota 1:/# /=.
-        rewrite posu32_0s ..2:/# posu16_0s ..3:/# posu8_0s ..3:/# posTrail_0s ..5:/#.
-        rewrite ifT ifT 1:/# 1:size_cat 1:size_drop 1:/#.
-        rewrite !size_cat size_nseq size_mkseq /#. smt().
-        rewrite nth_cat size_drop 1:/# size_nseq ifT 1:/# nth_drop ..2:/# nth_nseq /#.
-      + move: i_max i_min. rewrite -lezNgt lezNgt /= => i_max i_min.
-      case(i < 4 + (_at - _cur)) => u32.
-      + rewrite /u64bytes (nth_map witness W8.zero) /iotared 1:size_iota 1:/# /=.
-        rewrite u32_word ..2:/# posu16_0s ..3:/# posu8_0s ..3:/# posTrail_0s ..5:/#.
-        rewrite !ifT 1:/#. rewrite !size_cat size_drop 1:/# /sub size_mkseq /#. smt().
-        rewrite !nth_cat size_drop 1:/# size_nseq ifF 1:/# size_mkseq ifT 1:/#.
-        rewrite nth_mkseq 1:/# orw0 /= !lez_maxr ..3:/# /(\bits8).
-        rewrite (W8.ext_eq _ (_buf.[pos + (i - x)])). move => x0 x0_bnd.
-          rewrite initE ifT 1:/# /WA.init8 /get32_direct /pack4_t /=.
-          rewrite initE ifT 1:nth_iota ..2:/# /= initE ifT 1:nth_iota ..2:/# /=.
-          rewrite !nth_iota 1:/# initE ifT /#. smt().
-      move: u32. rewrite -lezNgt => over_u32.
-      case(i < 6 + (_at - _cur)) => u16.
-      + rewrite /u64bytes (nth_map witness W8.zero) /iotared 1:size_iota 1:/# /=.
-        rewrite preu32_0s ..2:/# u16_word ..3:/# posu8_0s ..3:/# posTrail_0s ..5:/#.
-        rewrite !ifT 1:/#. rewrite !size_cat size_drop 1:/# size_mkseq size_nseq /#. smt().
-        rewrite !nth_cat size_drop 1:/# size_nseq ifF 1:/# size_mkseq ifT 1:/#.
-        rewrite nth_mkseq 1:/# or0w /= !lez_maxr ..3:/# /(\bits8).
-        rewrite (W8.ext_eq _ (_buf.[pos + (i - x)])). move => x0 x0_bnd.
-          rewrite initE ifT 1:/# /WA.init8 /get16_direct /pack2_t /=.
-          rewrite initE ifT 1:nth_iota ..2:/# /= initE ifT 1:nth_iota ..2:/# /=.
-          rewrite !nth_iota 1:/# initE ifT /#. smt().
-      + rewrite /u64bytes (nth_map witness W8.zero) /iotared 1:size_iota 1:/# /=.
-        rewrite preu32_0s ..2:/# preu16_0s ..3:/# u8_word ..3:/# posTrail_0s ..5:/#.
-        rewrite !ifT 1:/#. rewrite !size_cat size_drop 1:/# size_mkseq size_nseq /#. smt().
-        rewrite !nth_cat size_drop 1:/# size_nseq ifF 1:/# size_mkseq ifT 1:/#.
-        rewrite nth_mkseq 1:/# or0w /= !lez_maxr ..3:/# /(\bits8).
-        rewrite (W8.ext_eq _ (_buf.[pos + (i - x)])). move => x0 x0_bnd.
-          rewrite ifT 1:/# /get8 initE ifT /#. smt().
-      smt().
-qed.
-
-lemma compose2u8_trail0 _buf pos x _cur _at:
-  0 <= _cur =>
-  0 <= _at =>
-  _cur <= _at =>
-  _at - _cur = x =>
-  x < 8 =>
-  0 <= x =>
-  0 <= pos =>
-  pos + 8 < _ASIZE =>
-u64bytes
-  (zeroextu64 (get16_direct (WA.init8 (ReadWriteArray.A."_.[_]" _buf)) pos) `<<<` 8 * x)
- = bytes_at 8 _cur _at (sub _buf pos 2 ++ [W8.zero]).
-proof.
-  move => H0 H1 H2 H3 H4 H5 H6 H7.
-  pose w0:= zeroextu64 (get16_direct (WA.init8 ("_.[_]" _buf)) pos) `<<<` 8 * x.
-  pose l1:= u64bytes w0.
-  pose l2:= bytes_at 8 _cur _at (sub _buf pos 2 ++ [W8.zero]).
-    rewrite (eq_from_nth W8.zero l1 l2).
-    + rewrite size_to_list size_take 1:/# size_cat size_drop 1:/# size_nseq /#.
-    + rewrite size_to_list /l1 => i i_bnd.
-      rewrite /l2 /bytes_at nth_take..2:/# drop_cat_le nth_cat size_nseq lez_maxr 1:/#H2/=.
-      case(2 + x <= i) => i_max.
-      + rewrite /u64bytes (nth_map witness W8.zero) /iotared 1:size_iota 1:/# /=.
-        rewrite (preu16_0s x 0 _ _ pos) ..3:/# !size_cat size_drop 1:/# size_mkseq.
-        rewrite size_nseq !lez_maxr ..4:/# /=.
-        case(i < _at - _cur + 3) =>*.
-        rewrite !nth_cat size_drop 1:/# size_nseq ifF 1:/# size_mkseq ifF /#.
-        rewrite nth_nseq /#.
-      case(i < x) => i_min.
-      + rewrite /u64bytes (nth_map witness W8.zero) /iotared 1:size_iota 1:/# /=.
-        rewrite (posu16_0s x 0 _ _ pos) ..3:/# !size_cat size_drop 1:/# size_nseq.
-        rewrite size_mkseq ifT 1:/# nth_cat size_drop 1:/# size_nseq ifT 1:/#.
-        rewrite nth_drop ..2:/# nth_nseq /#.
-      + move: i_max i_min. rewrite -lezNgt lezNgt /= => i_max i_min.
-      + rewrite /u64bytes (nth_map witness W8.zero) /iotared 1:size_iota 1:/# /=.
-        rewrite (u16_word x 0 _ _ pos) ..3:/# !size_cat size_drop 1:/# size_nseq.
-        rewrite size_mkseq ifT 1:/# nth_cat size_drop 1:/# size_nseq ifF 1:/#.
-        rewrite nth_cat nth_mkseq 1:/# size_mkseq ifT 1:/# !lez_maxr ..3:/# /(\bits8) /=.
-        rewrite (W8.ext_eq _ (_buf.[pos + (i - x)])). move => x0 x0_bnd.
-          rewrite initE ifT 1:/# /WA.init8 /get16_direct /pack2_t /=.
-          rewrite initE ifT 1:nth_iota ..2:/# /= initE ifT 1:nth_iota ..2:/# /=.
-          rewrite !nth_iota 1:/# initE ifT /#. smt().
-      smt().
-qed.
-
-lemma compose4u8_trail0 _buf pos x _cur _at:
-  0 <= _cur =>
-  0 <= _at =>
-  _cur <= _at =>
-  _at - _cur = x =>
-  x < 4 =>
-  0 <= x =>
-  0 <= pos =>
-  pos + 8 < _ASIZE =>
-  u64bytes (zeroextu64 (get32_direct (WA.init8 (ReadWriteArray.A."_.[_]" _buf)) pos)
-            `<<<` 8*x) = bytes_at 8 _cur _at (sub _buf pos 4 ++ [W8.zero]).
-proof.
-  move => H0 H1 H2 H3 H4 H5 H6 H7.
-  pose w0:= zeroextu64 (get32_direct (WA.init8 ("_.[_]" _buf)) pos) `<<<` 8*x.
-  pose l1:= u64bytes w0.
-  pose l2:= bytes_at 8 _cur _at (sub _buf pos 4 ++ [W8.zero]).
-    rewrite (eq_from_nth W8.zero l1 l2).
-    + rewrite size_to_list size_take 1:/# size_cat size_drop 1:/# size_nseq /#.
-    + rewrite size_to_list /l1 => i i_bnd.
-      rewrite /l2 /bytes_at nth_take ..2:/# drop_cat_le nth_cat size_nseq lez_maxr 1:/#.
-      case(4 + x <= i) => i_max.
-        rewrite /u64bytes (nth_map witness W8.zero) /iotared 1:size_iota 1:/# /=.
-        rewrite preu32_0s ..2:/# drop_cat_le size_mkseq H2 /=.
-        rewrite !size_cat !nth_cat size_drop 1:/# size_mkseq size_nseq !lez_maxr ..4:/# /=.
-        case(i < _at - _cur + 5) =>*; rewrite ?nth_nseq /#.
-      case(i < x) => i_min.
-      + rewrite /u64bytes (nth_map witness W8.zero) /iotared 1:size_iota 1:/# /=.
-        rewrite posu32_0s ..2:/# ifT ifT 1:/# 1:size_cat 1:size_drop 1:/#.
-        rewrite !size_cat size_nseq /sub size_mkseq /#. smt().
-        rewrite nth_cat size_drop 1:/# size_nseq ifT 1:/# nth_drop ..2:/# nth_nseq /#.
-      + move: i_max i_min. rewrite -lezNgt lezNgt /= => i_max i_min.
-      + rewrite /u64bytes (nth_map witness W8.zero) /iotared 1:size_iota 1:/# /=.
-        rewrite u32_word ..2:/# ifT ifT 1:/# 1:size_cat.
-        rewrite !size_cat size_drop 1:/# /sub size_mkseq size_nseq /#. smt().
-        rewrite !nth_cat size_drop 1:/# size_nseq ifF 1:/# size_mkseq ifT 1:/#.
-        rewrite nth_mkseq 1:/# /= !lez_maxr ..3:/# /(\bits8).
-        rewrite (W8.ext_eq _ (_buf.[pos + (i - x)])). move => x0 x0_bnd.
-          rewrite initE ifT 1:/# /WA.init8 /get32_direct /pack4_t /=.
-          rewrite initE ifT 1:nth_iota ..2:/# /= initE ifT 1:nth_iota ..2:/# /=.
-          rewrite !nth_iota 1:/# initE ifT /#. smt().
-      smt().
-qed.
-
-
-lemma compose6u8_trail0 _buf pos x _cur _at:
-  0 <= _cur =>
-  0 <= _at =>
-  _cur <= _at =>
-  _at - _cur = x =>
-  x < 2 =>
-  0 <= x =>
-  0 <= pos =>
-  pos + 8 < _ASIZE =>
-u64bytes
-  ((zeroextu64 (get32_direct (WA.init8 (ReadWriteArray.A."_.[_]" _buf)) pos) `<<<` 8*x) `|`
-   (zeroextu64 (get16_direct (WA.init8 (ReadWriteArray.A."_.[_]" _buf)) (pos + 4))
-    `<<<` 8 * (4 + x))) = bytes_at 8 _cur _at (sub _buf pos 6 ++ [W8.zero]).
-proof.
-  move => H0 H1 H2 H3 H4 H5 H6 H7.
-  pose w0:= zeroextu64 (get32_direct (WA.init8 ("_.[_]" _buf)) pos) `<<<` 8*x.
-  pose w1:= zeroextu64 (get16_direct (WA.init8 ("_.[_]" _buf)) (pos + 4)) `<<<` 8*(4+x).
-  pose l1:= u64bytes (w0 `|` w1).
-  pose l2:= bytes_at 8 _cur _at (sub _buf pos 6 ++ [W8.zero]).
-    rewrite (eq_from_nth W8.zero l1 l2).
-    + rewrite size_to_list size_take 1:/# size_cat size_drop 1:/# size_nseq /#.
-    + rewrite size_to_list /l1 => i i_bnd.
-      rewrite /l2 /bytes_at nth_take ..2:/# drop_cat_le nth_cat size_nseq lez_maxr 1:/#.
-      case(6 + x <= i) => i_max.
-        rewrite /u64bytes (nth_map witness W8.zero) /iotared 1:size_iota 1:/# /=.
-        rewrite preu32_0s ..2:/# preu16_0s ..3:/# drop_cat_le size_mkseq H2 /=.
-        rewrite !size_cat !nth_cat size_drop 1:/# size_mkseq size_nseq !lez_maxr ..4:/# /=.
-        case(i < _at - _cur + 7) =>*; rewrite ?nth_nseq /#.
-      case(i < x) => i_min.
-      + rewrite /u64bytes (nth_map witness W8.zero) /iotared 1:size_iota 1:/# /=.
-        rewrite posu32_0s ..2:/# posu16_0s ..3:/# ifT ifT 1:/# 1:size_cat 1:size_drop 1:/#.
-        rewrite !size_cat size_nseq /sub size_mkseq /#. smt().
-        rewrite nth_cat size_drop 1:/# size_nseq ifT 1:/# nth_drop ..2:/# nth_nseq /#.
-      + move: i_max i_min. rewrite -lezNgt lezNgt /= => i_max i_min.
-      case(i < 4 + (_at - _cur)) => u32.
-      + rewrite /u64bytes (nth_map witness W8.zero) /iotared 1:size_iota 1:/# /=.
-        rewrite u32_word ..2:/# posu16_0s ..3:/# ifT ifT 1:/# 1:size_cat.
-        rewrite !size_cat size_drop 1:/# /sub size_mkseq /#. smt().
-        rewrite !nth_cat size_drop 1:/# size_nseq ifF 1:/# size_mkseq ifT 1:/#.
-        rewrite nth_mkseq 1:/# orw0 /= !lez_maxr ..3:/# /(\bits8).
-        rewrite (W8.ext_eq _ (_buf.[pos + (i - x)])). move => x0 x0_bnd.
-          rewrite initE ifT 1:/# /WA.init8 /get32_direct /pack4_t /=.
-          rewrite initE ifT 1:nth_iota ..2:/# /= initE ifT 1:nth_iota ..2:/# /=.
-          rewrite !nth_iota 1:/# initE ifT /#. smt().
-      move: u32. rewrite -lezNgt => u16. 
-      + rewrite /u64bytes (nth_map witness W8.zero) /iotared 1:size_iota 1:/# /=.
-        rewrite preu32_0s ..2:/# u16_word ..3:/# ifT ifT 1:/# 1:size_cat.
-        rewrite !size_cat size_drop 1:/# /sub size_mkseq size_nseq /#. smt().
-        rewrite !nth_cat size_drop 1:/# size_nseq ifF 1:/# size_mkseq ifT 1:/#.
-        rewrite nth_mkseq 1:/# or0w /= !lez_maxr ..3:/# /(\bits8).
-        rewrite (W8.ext_eq _ (_buf.[pos + (i - x)])). move => x0 x0_bnd.
-          rewrite initE ifT 1:/# /WA.init8 /get16_direct /pack2_t /=.
-          rewrite initE ifT 1:nth_iota ..2:/# /= initE ifT 1:nth_iota ..2:/# /=.
-          rewrite !nth_iota 1:/# initE ifT /#. smt().
-      smt().
-qed.
-
-hoare a_ilen_read_upto8_at_h _buf _off _dlt _len _trail _cur _at:
+lemma a_ilen_read_upto8_at_h _buf _off _dlt _len _trail _cur _at:
+ (* 0 <= _len => *)
+ hoare [
  MM.__a_ilen_read_upto8_at
  : buf=_buf /\ offset=_off /\ dELTA=_dlt /\ lEN=_len /\ tRAIL=_trail /\ cUR=_cur /\ aT=_at
- ==> subread_spec 8 _buf _off _dlt _len _trail _cur _at res.`1 res.`2 res.`3 res.`4 (u64bytes res.`5).
+ ==> subread_spec 8 _buf _off _dlt _len _trail _cur _at res.`1 res.`2 res.`3 res.`4 (u64bytes res.`5) ].
 proof.
+case: (_len < 0) => Hlen.
+ conseq (:_ ==> true) => //.
+ by move => /> /#.
 proc; simplify.
+
 if => //.
- auto => /> [[H|H]|H].
- + move=> _; rewrite /subread_pre => /> ??????.
+ auto => |> [[H|H]|H]. 
+ + move=> _; rewrite /subread_pre => /> ?????????.
    rewrite (:!_cur<=_at) 1:/# /= => [[Elen Etb]].
    rewrite !Elen !Etb; split; first smt().
    split.
-    rewrite sub0 bytes_at8_zero /#. 
+    by rewrite sub0 bytes_at_zeros 1:/# /u64bytes /= !get_zero -mkseq_nseq /mkseq -iotaredE. 
    smt().
-  + apply subread_spec_ahead8; smt().
-  apply subread_spec_empty8; smt().
+  + by apply subread_spec_ahead8; smt().
+  by apply subread_spec_empty8; smt().
+
 sp; if => //.
  (* 8 <= lEN *)
- wp; ecall (SHLQ_h w aT8); auto => />.
- rewrite !negb_or negb_and -!lezNgt andb_orr. move =>*.
+ wp; ecall (SHLQ_h w (aT-cUR)); auto => |> *.
  split; first smt().
-  move => ???. rewrite /subread_pre oraE andaE => [#] *.
- do split; 1..2: smt(); 2..5: smt().
-   have->: to_uint (W64.of_int (_off + _dlt)) = _off + _dlt. admit.
-   have min_pos: 0 <= _off + _dlt. admit.
-   have max_pos: _off + _dlt + 8 < _ASIZE. admit.
-   apply compose8u8; smt().
- (* 4 <= lEN < 8 *)
+ move=> ??.
+ by apply subread_u64.
+
+conseq (: _cur <= _at < _cur+8 /\ _len < 8 /\ (_len<>0 \/ _trail<>0) 
+         /\ buf=_buf /\ offset=_off /\ cUR=_cur /\ tRAIL=_trail
+         /\ dELTA=_dlt /\ lEN=_len /\ aT=_at==> _).
+ by move => /> /#.
+
+pose n0 := min (_cur + 8 - _at) (_len %/ 4 * 4).
+seq 1: ( #[:7]pre
+       /\ subread_spec 8 _buf _off _dlt (_len %/ 4 * 4) 0 _cur _at dELTA (_len %/ 4 * 4-n0) 0 aT (u64bytes w)
+       /\ dELTA = _dlt+n0 /\ lEN = _len - n0 /\ aT=_at+n0).
+ if => //.
+  (* 4 <= lEN  *)
+  wp; ecall (SHLQ_h w (aT-cUR)); auto => /> *.
+  split; first smt().
+  move=> ??.
+  rewrite /n0.
+  have ->: _len %/ 4 * 4 = 4 by smt().
+  have ->: (_dlt + if _cur + 8 <= _at + 4 then _cur + 8 - _at else 4)
+          = _dlt + min (_cur+8-_at) 4 by smt().
+  have ->: (if _cur + 8 <= _at + 4 then _cur + 8 else _at + 4)
+          = _at + min (_cur+8-_at) 4 by smt().
+  split.
+   by apply (subread_u32 (min (_cur+8-_at) 4) _buf _off _dlt _cur _at _ _); smt().
+  smt().
+ auto => /> ?????.
+ rewrite /n0.
+ have ->: _len%/4*4 = 0 by smt().
+ rewrite ler_minr 1:/# /=.
+ by apply subread_spec_empty8.
+
+pose n1 := min (_cur+8-_at) (_len %/ 2 * 2).
+exlim aT => at1; exlim lEN => len1; exlim dELTA => dlt1.
+conseq (: _cur <= _at < _cur+8 /\ _len < 8 /\ (_len<>0 \/ _trail<>0) 
+         /\ buf=_buf /\ offset=_off /\ cUR=_cur
+         /\ tRAIL=_trail /\ dELTA=dlt1 /\ lEN=len1 /\ aT=at1
+         /\ subread_spec 8 _buf _off _dlt (_len%/4*4) 0 _cur
+             _at dlt1 (_len %/ 4 * 4 - n0) 0 at1 (u64bytes w)
+         /\ dlt1=_dlt+n0 /\ len1=_len-n0 /\ at1=_at+n0
+         ==> _).
+ by move => />. 
+
+seq 1: ( #[/:8]pre
+/\ subread_spec 8 _buf _off _dlt (_len %/ 2 * 2) 0 _cur
+    _at dELTA (_len%/2*2-n1) 0 aT (u64bytes w) 
+/\ dELTA=_dlt+n1 /\ lEN=_len-n1 /\ aT=_at+n1).
+ if => //.
+  (* 2 <= lEN *)
+  wp; ecall (SHLQ_h t16 (aT-cUR)); auto => /> ????? H1??.
+  split; first smt(). 
+  move=> ??; split.
+   rewrite -!addzA.
+   have ->: (n0 + if _cur + 8 <= _at + (n0 + 2) then _cur + (8 - (_at + n0)) else 2)=n1 by smt().
+   have ->: (if _cur + 8 <= _at + (n0 + 2) then _cur + 8 else _at + (n0 + 2))=_at+n1 by smt().
+   rewrite (addzA _at).
+   by apply (subread_w4_u16 n1 _buf _off _ _ _ _ _ _ _ _ _ _ _ _ H1); smt().
+  smt().
+ auto => /> &m ????H.
+ rewrite negb_and; move => [?|?].
+  have En0: n0 = _cur+8-_at by smt().
+  have En1: n1 = n0 by smt().
+  split.
+   rewrite En1 {2}En0.
+   by apply (subread_w4_ahead _buf _off _ _ _ _ _ _ _ _ _ _ _ H); smt().
+  smt().
+ have ->: (_len %/ 2 * 2) = (_len %/ 4 * 4) by smt().
+ have ->: n1 = n0 by smt().
+ split; first smt().
+ smt(). 
+
+pose n2 := min (_cur+8-_at) _len.
+exlim aT => at2; exlim lEN => len2; exlim dELTA => dlt2.
+conseq (: _cur <= _at < _cur+8 /\ _len < 8 /\ (_len<>0 \/ _trail<>0) 
+         /\ buf=_buf /\ offset=_off /\ cUR=_cur
+         /\ tRAIL=_trail /\ dELTA=dlt2 /\ lEN=len2 /\ aT=at2
+         /\ subread_spec 8 _buf _off _dlt (_len%/2*2) 0 _cur
+             _at dlt2 (_len %/ 2 * 2 - n1) 0 at2 (u64bytes w)
+         /\ dlt2=_dlt+n1 /\ len2=_len-n1 /\ at2=_at+n1
+         ==> _).
+ by move => />. 
+
+seq 1: ( #[/:8]pre
+       /\ subread_spec 8 _buf _off _dlt _len 0 _cur
+                         _at dELTA (_len-n2) 0 aT (u64bytes w) 
+       /\ dELTA=_dlt+n2 /\ lEN=_len-n2 /\ aT=_at+n2).
+ if => //.
+  (* 1 <= lEN *)
+  wp; ecall (SHLQ_h t8 (aT-cUR)); auto => /> ????? H1??.
+  split; first smt(). 
+  move=> ??; split.
+   rewrite -!addzA.
+   have ->: n1+1=n2 by smt().
+   rewrite (addzA _at).
+   by apply (subread_w2_u8 n2 _buf _off _ _ _ _ _ _ _ _ _ _ _ _ H1); smt().
+  smt().
+ auto => /> &m ????H.
+ rewrite negb_and; move => [?|?].
+  have En1: n1 = _cur+8-_at by smt().
+  have En2: n2 = n1 by smt().
+  split.
+   rewrite En2 {2}En1.
+   by apply (subread_w2_ahead _buf _off _ _ _ _ _ _ _ _ _ _ _ H); smt().
+  smt().
+ have ->: _len = _len %/ 2 * 2 by smt().
+ have ->: n2 = n1 by smt().
+ split; first smt().
+ smt(). 
+
 if => //.
- case(4 <= aT8).
-   rcondf 6. wp; ecall (SHLQ_h w aT8); auto => /#.
-   rcondf 6. wp; ecall (SHLQ_h w aT8); auto => /#.
-   wp; ecall (SHLQ_h w aT8); auto => />.
-   rewrite !negb_or negb_and -!lezNgt andb_orr. move => [#] *.
-   split; first smt().
-   move=> ???. rewrite /subread_pre oraE andaE => [#] *.
-   do split; 1..2: smt(); 2..5: smt().
-   + (* Need info regarding _off and _dlt bounds *)
-     have->: to_uint (W64.of_int (_off + _dlt)) = _off + _dlt. admit.
-     have min_pos: 0 <= _off + _dlt. admit.
-     have max_pos: _off + _dlt + 8 < _ASIZE. admit.
-     apply compose4u8; smt().
-     case(6 <= lEN).
-     + rcondt 6. wp; ecall (SHLQ_h w aT8); auto => /#.
-       case(2 <= aT8). 
-       + rcondf 12. wp; ecall (SHLQ_h t16 aT8); wp; ecall (SHLQ_h w aT8); auto => /#.
-         wp; ecall (SHLQ_h t16 aT8); wp; ecall (SHLQ_h w aT8); auto => />.
-         rewrite !negb_or negb_and -!lezNgt andb_orr. move => [#] H H1 H2 H3 H4 H5.
-         split; first smt(). move => [#] H6 H7.
-         split; first smt().
-        rewrite ifF 1:/# ifF 1:/# !ifT ..2:/#=> H8 H9 H10. rewrite /subread_pre oraE andaE.
-        move => [#] H11 H12 H13 H14 H15 H16 H17.
-        do split; 1..2: smt(); 2..5: smt().
-        + (* Need info regarding _off and _dlt bounds *)
-          have aux: _ASIZE < W64.modulus. admit.
-          have min_pos: 0 <= _off + _dlt. admit.
-          have max_pos: _off + _dlt + 8 < _ASIZE. admit.
-          rewrite !of_uintK !pmod_small.
-            split; 1: by smt(). move=> _. rewrite (ltr_trans _ASIZE); 1:smt(). rewrite aux.
-            split; 1: by smt(). move=> _. rewrite (ltr_trans _ASIZE); 1:smt(). rewrite aux.
-        rewrite -(compose6u8 _ _ (_at - _cur)) /#.
-   + rcondt 12. wp; ecall (SHLQ_h t16 aT8); wp; ecall (SHLQ_h w aT8); auto => /#.
-     case(lEN = 7).
-     + rcondt 12. wp; ecall (SHLQ_h t16 aT8); wp; ecall (SHLQ_h w aT8); auto => /#.
-        wp; ecall (SHLQ_h t8 aT8); wp; ecall (SHLQ_h t16 aT8); wp; ecall (SHLQ_h w aT8).
-        auto => />.
-        rewrite !negb_or negb_and -!lezNgt. move => [#] H0 H1 H2 H3 H4.
-        split; first smt(). move => [#] H6 H7.
-        split; first smt().
-        rewrite !ifF ..4:/# => H8 H9.
-        split; first smt(). move => H10 H11.
-        (* Need info regarding _off and _dlt bounds *)
-        have aux: _ASIZE < W64.modulus. admit.
-        have min_pos: 0 <= _off + _dlt. admit.
-        have max_pos: _off + _dlt + 8 < _ASIZE. admit.
-        split. move =>  ???. rewrite /subread_pre !andaE oraE. move => [#] *.
-        do split; 1..3: smt(); 2..4: smt().
-        + rewrite !of_uintK !pmod_small.
-            split; 1: by smt(). move=> _. rewrite(ltr_trans _ASIZE); 1:smt(). rewrite aux.
-            split; 1: by smt(). move=> _. rewrite(ltr_trans _ASIZE); 1:smt(). rewrite aux.
-            split; 1: by smt(). move=> _. rewrite(ltr_trans _ASIZE); 1:smt(). rewrite aux.
-            smt().
-          rewrite -(compose7u8_trail _ _ (_at - _cur)) /#.
-        move =>  ??. rewrite /subread_pre !andaE oraE. move => [#]*.
-        do split; 1..6: smt(); 2..4: smt().
-        + rewrite !of_uintK !pmod_small.
-            split; 1: by smt(). move=> _. rewrite(ltr_trans _ASIZE); 1:smt(). rewrite aux.
-            split; 1: by smt(). move=> _. rewrite(ltr_trans _ASIZE); 1:smt(). rewrite aux.
-            split; 1: by smt(). move=> _. rewrite(ltr_trans _ASIZE); 1:smt(). rewrite aux.
-            smt().
-          rewrite -(compose7u8_trail _ _ (_at - _cur)) /#.
-        move =>*.
-    + rcondf 12. wp; ecall (SHLQ_h t16 aT8); wp; ecall (SHLQ_h w aT8); auto => /#.
-      case(tRAIL %% 256 <> 0).
-      + rcondt 12. wp; ecall (SHLQ_h t16 aT8); wp; ecall (SHLQ_h w aT8); auto => /#.
-        wp; ecall (SHLQ_h t8 aT8); wp; ecall (SHLQ_h t16 aT8); wp; ecall (SHLQ_h w aT8).
-        auto => />.
-        rewrite !negb_or negb_and -!lezNgt andb_orr.
-        move => [#] H H1 H2 H3 H4 H5 H6 H7. have->: _len = 6 by smt().
-        split; first smt(). move => [#] H8 H9.
-        split; first smt().
-        rewrite !ifF ..4:/# /subread_spec /subread_pre !andaE oraE => H10 H11.
-        split;first smt(). move=> H12 H13 H14 [#] H15 H16 H17 H18 H19 H20 H21.
-        do split; 1..3: smt(); 2..4: smt().
-        + (* Need info regarding _off and _dlt bounds *)
-          have aux: _ASIZE < W64.modulus. admit.
-          have min_pos: 0 <= _off + _dlt. admit.
-          have max_pos: _off + _dlt + 8 < _ASIZE. admit.
-          rewrite !of_uintK !pmod_small.
-            split; first smt(). move=> _. rewrite(ltr_trans _ASIZE); 1:smt(). rewrite aux.
-            split; first smt(). move=> _. rewrite(ltr_trans _ASIZE); 1:smt(). rewrite aux.
-            smt().
-          rewrite !addrA /= -(compose6u8_trail _ _ (_at - _cur)) /#.
-      + rcondf 12. wp; ecall (SHLQ_h t16 aT8); wp; ecall (SHLQ_h w aT8); auto => /#.
-        wp; ecall (SHLQ_h t16 aT8); wp; ecall (SHLQ_h w aT8). auto => />.
-        rewrite !negb_or negb_and -!lezNgt andb_orr.
-        move => [#] H H1 H2 H3 H4 H5 H6 H7. have->: _len = 6 by smt().
-        split; first smt(). move => [#] H8 H9.
-        split; first smt().
-        rewrite !ifF ..4:/# /subread_spec /subread_pre !andaE oraE.
-        move => H10 H11 H12 [#] H13 H14 H15 H16 H17 H18 H19.
-        do split; 1..6: smt(); 2..4: smt().
-        + (* Need info regarding _off and _dlt bounds *)
-          have aux: _ASIZE < W64.modulus. admit.
-          have min_pos: 0 <= _off + _dlt. admit.
-          have max_pos: _off + _dlt + 8 < _ASIZE. admit.
-          rewrite !of_uintK !pmod_small.
-            split; first smt(). move=> _. rewrite(ltr_trans _ASIZE); 1:smt(). rewrite aux.
-            split; first smt(). move=> _. rewrite(ltr_trans _ASIZE); 1:smt(). rewrite aux.
-          rewrite -of_int_mod H7.
-          rewrite !addrA /= -(compose6u8_trail0 _ _ (_at - _cur)) /#.
-  + rcondf 6. wp; ecall (SHLQ_h w aT8); auto => /#.
-    rcondt 6. wp; ecall (SHLQ_h w aT8); auto => /#.
-    case(lEN = 5).
-    + rcondt 6. wp; ecall (SHLQ_h w aT8); auto => /#.
-      wp; ecall (SHLQ_h t8 aT8); wp; ecall (SHLQ_h w aT8); auto => />.
-      rewrite !negb_or negb_and -!lezNgt.
-      move => *. split; first smt().
-      move => *. split; first smt().
-      rewrite !ifF ..2:/# /subread_spec /subread_pre !andaE oraE => *.
-      (* Need info regarding _off and _dlt bounds *)
-      have aux: _ASIZE < W64.modulus. admit.
-      have min_pos: 0 <= _off + _dlt. admit.
-      have max_pos: _off + _dlt + 8 < _ASIZE. admit.
-      split. move => ??? [#] H10 H11 H12 H13 H14 H15 H16.
-      do split; 1..3:smt(); 2..4:smt().
-        rewrite !of_uintK !pmod_small.
-          split; first smt(). move=> _. rewrite(ltr_trans _ASIZE); 1:smt(). rewrite aux.
-          split; first smt(). move=> _. rewrite(ltr_trans _ASIZE); 1:smt(). rewrite aux.
-          smt().
-        rewrite -shlw_or trail_simplify ..2:/# addrA -(compose5u8_trail _ _ (_at-_cur)) /#.
-      move => ?? [#] H10 H11 H12 H13 H14 H15 H16.
-      do split; 1..6:smt(); 2..4:smt().
-        rewrite !of_uintK !pmod_small.
-          split; first smt(). move=> _. rewrite(ltr_trans _ASIZE); 1:smt(). rewrite aux.
-          split; first smt(). move=> _. rewrite(ltr_trans _ASIZE); 1:smt(). rewrite aux.
-          smt().
-        rewrite -shlw_or trail_simplify ..2:/# addrA -(compose5u8_trail _ _ (_at-_cur)) /#.
-  + rcondf 6. wp; ecall (SHLQ_h w aT8); auto => /#.
-    case(tRAIL %% 256 <> 0).
-    + rcondt 6. wp; ecall (SHLQ_h w aT8); auto => /#.
-      wp; ecall (SHLQ_h t8 aT8); wp; ecall (SHLQ_h w aT8); auto => />.
-      rewrite !negb_or negb_and -!lezNgt andb_orr.
-      move => H H0 H1 H2 H3 H4 H5. have->: _len = 4 by smt().
-      split; first smt(). move => H6 H7.
-      rewrite !ifF ..2:/# /subread_spec /subread_pre !andaE oraE.
-      + (* Need info regarding _off and _dlt bounds *)
-        have aux: _ASIZE < W64.modulus. admit.
-        have min_pos: 0 <= _off + _dlt. admit.
-        have max_pos: _off + _dlt + 8 < _ASIZE. admit.
-      split; first smt(). move => ??? [#] *.
-      do split; 1..3:smt(); 2..4:smt().
-        rewrite of_uintK !pmod_small. 
-          split; first smt(). move=> _. rewrite(ltr_trans _ASIZE); 1:smt(). rewrite aux.
-          smt().
-        rewrite -(compose4u8_trail _ _ (_at - _cur)) /#.
-   + rcondf 6. wp; ecall (SHLQ_h w aT8); auto => /#.
-      wp; ecall (SHLQ_h w aT8); auto => />.
-      rewrite !negb_or negb_and -!lezNgt andb_orr.
-      move => ?????? H5. have->: _len = 4 by smt().
-      split; first smt(). move => *.
-      rewrite !ifF ..2:/# /subread_spec /subread_pre !andaE oraE. move => *.
-      do split; 1..6:smt(); 2..4:smt().
-      + (* Need info regarding _off and _dlt bounds *)
-        have aux: _ASIZE < W64.modulus. admit.
-        have min_pos: 0 <= _off + _dlt. admit.
-        have max_pos: _off + _dlt + 8 < _ASIZE. admit.
-        rewrite of_uintK !pmod_small. 
-          split; first smt(). move=> _. rewrite(ltr_trans _ASIZE); 1:smt(). rewrite aux.
-        rewrite -of_int_mod H5.
-        rewrite -(compose4u8_trail0 _ _ (_at - _cur)) /#.
-(* lEN < 4 *)
-case(2 <= lEN).
-+ rcondt 2. auto => /#.
-  case(aT8 < 5).
-  + rcondt 8. wp; ecall (SHLQ_h t16 aT8); auto => /#.
-    case(lEN = 3).
-    + rcondt 8. wp; ecall (SHLQ_h t16 aT8); auto => /#.
-      case(tRAIL %% 256 <> 0).
-      + rcondt 15. wp; ecall (SHLQ_h t8 aT8); wp; ecall (SHLQ_h t16 aT8); auto => /#.
-        wp; ecall (SHLQ_h t8 aT8); wp; ecall (SHLQ_h t16 aT8); auto => />.
-        rewrite negb_or lezNgt -lezNgt /= => H0 H1 H2.
-        split; first by smt(). move => H3 H4.
-        rewrite !ifF ..2:/#. split; first by smt().
-        rewrite /subread_spec /subread_pre !andaE oraE => *.
-        do split; 1..3: smt(); 2..4: smt().
-      + (* Need info regarding _off and _dlt bounds *)
-        have aux: _ASIZE < W64.modulus. admit.
-        have min_pos: 0 <= _off + _dlt. admit.
-        have max_pos: _off + _dlt + 8 < _ASIZE. admit.
-        rewrite !of_uintK !pmod_small. 
-          split; first smt(). move=> _. rewrite(ltr_trans _ASIZE); 1:smt(). rewrite aux.
-          split; first smt(). move=> _. rewrite(ltr_trans _ASIZE); 1:smt(). rewrite aux.
-        smt().
-        rewrite -(compose3u8_trail _ _ (_at - _cur)) /#.
-    + rcondf 15. wp; ecall (SHLQ_h t8 aT8); wp; ecall (SHLQ_h t16 aT8); auto => /#.
-        wp; ecall (SHLQ_h t8 aT8); wp; ecall (SHLQ_h t16 aT8); auto => />.
-        rewrite negb_or lezNgt -lezNgt /= => *.
-        split; first by smt(). move => *.
-        rewrite !ifF ..2:/#. split; first by smt().
-        rewrite /subread_spec /subread_pre !andaE oraE => *.
-        do split; 1..6: smt(); 2..4: smt().
-      + (* Need info regarding _off and _dlt bounds *)
-        have aux: _ASIZE < W64.modulus. admit.
-        have min_pos: 0 <= _off + _dlt. admit.
-        have max_pos: _off + _dlt + 8 < _ASIZE. admit.
-        rewrite !of_uintK !pmod_small. 
-          split; first smt(). move=> _. rewrite(ltr_trans _ASIZE); 1:smt(). rewrite aux.
-          split; first smt(). move=> _. rewrite(ltr_trans _ASIZE); 1:smt(). rewrite aux.
-        smt().
-        rewrite -(compose3u8_trail _ _ (_at - _cur)) /#.
-    + rcondf 8. wp; ecall (SHLQ_h t16 aT8); auto => /#.
-      case(tRAIL %% 256 <> 0).
-      + rcondt 8. wp; ecall (SHLQ_h t16 aT8); auto => /#.
-        wp; ecall (SHLQ_h t8 aT8); wp; ecall (SHLQ_h t16 aT8); auto => />.
-        rewrite !negb_or lezNgt -lezNgt /= => *.
-        split; first by smt(). move => H7 H8.
-        rewrite !ifF ..2:/#. split; first by smt().
-        rewrite /subread_spec /subread_pre !andaE oraE => *. have->: _len = 2 by smt().
-        do split; 1..3: smt(); 2..4: smt().
-      + (* Need info regarding _off and _dlt bounds *)
-        have aux: _ASIZE < W64.modulus. admit.
-        have min_pos: 0 <= _off + _dlt. admit.
-        have max_pos: _off + _dlt + 8 < _ASIZE. admit.
-        rewrite !of_uintK !pmod_small. 
-          split; first smt(). move=> _. rewrite(ltr_trans _ASIZE); 1:smt(). rewrite aux.
-        smt().
-        rewrite -(compose2u8_trail _ _ (_at - _cur)) /#.
-    + rcondf 8. wp; ecall (SHLQ_h t16 aT8); auto => /#.
-        wp; ecall (SHLQ_h t16 aT8); auto => />.
-        rewrite !negb_or lezNgt -lezNgt /= => ??????H6.
-        split; first by smt(). move => *. have->: _len = 2 by smt().
-        rewrite !ifF ..2:/# /subread_spec /subread_pre !andaE oraE =>*.
-        do split; 1..6: smt(); 2..4: smt().
-        + (* Need info regarding _off and _dlt bounds *)
-          have aux: _ASIZE < W64.modulus. admit.
-          have min_pos: 0 <= _off + _dlt. admit.
-          have max_pos: _off + _dlt + 8 < _ASIZE. admit.
-          rewrite !of_uintK !pmod_small. 
-            split; first smt(). move=> _. rewrite(ltr_trans _ASIZE); 1:smt(). rewrite aux.
-          rewrite -of_int_mod H6.
-          rewrite -(compose2u8_trail0 _ _ (_at - _cur)) /#.
-  case(aT8 = 5).
-  + rcondt 8. wp; ecall (SHLQ_h t16 aT8); auto => /#.
-    case(lEN = 3).
-    + rcondt 8. wp; ecall (SHLQ_h t16 aT8); auto => /#.
-      rcondf 15. wp; ecall (SHLQ_h t8 aT8); wp; ecall (SHLQ_h t16 aT8); auto => /#.
-        wp; ecall (SHLQ_h t8 aT8); wp; ecall (SHLQ_h t16 aT8); auto => />.
-        rewrite negb_or lezNgt -lezNgt /= => *.
-        split; first by smt(). move => *.
-        rewrite !ifF ..2:/#. split; first by smt().
-        rewrite /subread_spec /subread_pre !andaE oraE =>*.
-        do split; 1..6: smt(); 2..4: smt().
-        + (* Need info regarding _off and _dlt bounds *)
-          have aux: _ASIZE < W64.modulus. admit.
-          have min_pos: 0 <= _off + _dlt. admit.
-          have max_pos: _off + _dlt + 8 < _ASIZE. admit.
-          rewrite !of_uintK !pmod_small. 
-            split; first smt(). move=> _. rewrite(ltr_trans _ASIZE); 1:smt(). rewrite aux.
-            split; first smt(). move=> _. rewrite(ltr_trans _ASIZE); 1:smt(). rewrite aux.
-          smt().
-          rewrite !addrA /= -(compose3u8_trail _ _ (_at - _cur)) /#.
-    + rcondf 8. wp; ecall (SHLQ_h t16 aT8); auto => /#.
-      case(tRAIL %% 256 <> 0).
-      + rcondt 8. wp; ecall (SHLQ_h t16 aT8); auto => /#.
-        wp; ecall (SHLQ_h t8 aT8); wp; ecall (SHLQ_h t16 aT8); auto => />.
-        rewrite !negb_or lezNgt -lezNgt /= => *.
-        split; first by smt(). move => *.
-        rewrite !ifF ..2:/#. split; first by smt().
-        rewrite /subread_spec /subread_pre !andaE oraE => *. have->: _len = 2 by smt().
-        do split; 1..3: smt(); 2..4: smt().
-      + (* Need info regarding _off and _dlt bounds *)
-        have aux: _ASIZE < W64.modulus. admit.
-        have min_pos: 0 <= _off + _dlt. admit.
-        have max_pos: _off + _dlt + 8 < _ASIZE. admit.
-        rewrite !of_uintK !pmod_small. 
-          split; first smt(). move=> _. rewrite(ltr_trans _ASIZE); 1:smt(). rewrite aux.
-        smt().
-        rewrite -(compose2u8_trail _ _ (_at - _cur)) /#.
-    + rcondf 8. wp; ecall (SHLQ_h t16 aT8); auto => /#.
-        wp; ecall (SHLQ_h t16 aT8); auto => />.
-        rewrite !negb_or lezNgt -lezNgt /= => ???????H.
-        split; first by smt(). move => *. have->: _len = 2 by smt().
-        rewrite !ifF ..2:/# /subread_spec /subread_pre !andaE oraE => *.
-        do split; 1..6: smt(); 2..4: smt().
-        + (* Need info regarding _off and _dlt bounds *)
-          have aux: _ASIZE < W64.modulus. admit.
-          have min_pos: 0 <= _off + _dlt. admit.
-          have max_pos: _off + _dlt + 8 < _ASIZE. admit.
-          rewrite !of_uintK !pmod_small. 
-           split; first smt(). move=> _. rewrite(ltr_trans _ASIZE); 1:smt(). rewrite aux.
-          rewrite -of_int_mod H.
-          rewrite -(compose2u8_trail0 _ _ (_at - _cur)) /#.
-  + rcondf 8. wp; ecall (SHLQ_h t16 aT8); auto => /#. 
-    wp; ecall (SHLQ_h t16 aT8); auto => />.
-    rewrite !negb_or !negb_and lezNgt -lezNgt /= => *.
-    split; first by smt(). move => H7 H8.
-    rewrite !ifT ..2:/# /subread_spec /subread_pre !andaE oraE => *.
-    do split; 1..6: smt(); 2..5: smt().
-    + (* Need info regarding _off and _dlt bounds *)
-      have aux: _ASIZE < W64.modulus. admit.
-      have min_pos: 0 <= _off + _dlt. admit.
-      have max_pos: _off + _dlt + 8 < _ASIZE. admit.
-      rewrite !of_uintK !pmod_small. 
-        split; first smt(). move=> _. rewrite(ltr_trans _ASIZE); 1: smt(). rewrite aux.
-        rewrite -(compose2u8 _ _ (_at - _cur)) /#.
-(* 0 <= lEN < 2 *)
-rcondf 2. auto => /#.
-case(aT8 < 7).
-+ rcondt 2. auto => /#.
-  case(lEN = 1). 
-  + rcondt 2. auto => /#.
-    case(tRAIL %% 256 <> 0).
-    + rcondt 9. wp; ecall (SHLQ_h t8 aT8); auto => /#.
-       wp; ecall (SHLQ_h t8 aT8); auto => />.
-      rewrite !negb_or lezNgt -lezNgt /= => *.
-      split; first by smt(). move => *.
-      rewrite /subread_spec /subread_pre !andaE oraE => *.
-      do split; 1..3: smt(); 2..4: smt().
-      + (* Need info regarding _off and _dlt bounds *)
-        have aux: _ASIZE < W64.modulus. admit.
-        have min_pos: 0 <= _off + _dlt. admit.
-        have max_pos: _off + _dlt + 8 < _ASIZE. admit.
-        rewrite !of_uintK !pmod_small. 
-          split; first smt(). move=> _. rewrite(ltr_trans _ASIZE); 1:smt(). rewrite aux.
-        smt().
-        rewrite -(compose1u8_trail _ _ (_at - _cur)) /#.
-    + rcondf 9. wp; ecall (SHLQ_h t8 aT8); auto => /#.
-       wp; ecall (SHLQ_h t8 aT8); auto => />.
-      rewrite !negb_or lezNgt -lezNgt /= => *.
-      split; first by smt(). move => H7 H8.
-      rewrite /subread_spec /subread_pre !andaE oraE => *.
-      do split; 1..6: smt(); 2..4: smt().
-      + (* Need info regarding _off and _dlt bounds *)
-        have aux: _ASIZE < W64.modulus. admit.
-        have min_pos: 0 <= _off + _dlt. admit.
-        have max_pos: _off + _dlt + 8 < _ASIZE. admit.
-        rewrite !of_uintK !pmod_small. 
-          split; first smt(). move=> _. rewrite(ltr_trans _ASIZE); 1:smt(). rewrite aux.
-        smt().
-        rewrite -(compose1u8_trail _ _ (_at - _cur)) /#.
-  + rcondf 2. auto => /#.
-    case(tRAIL %% 256 <> 0).
-    + rcondt 2. auto => /#.
-      wp; ecall (SHLQ_h t8 aT8); auto => />.
-      rewrite !negb_or lezNgt -lezNgt /= => *.
-      split; first by smt(). move => *.
-      rewrite /subread_spec /subread_pre !andaE oraE => *.
-      do split; 1..5: smt(); 2..5: smt(). have->: _len = 0 by smt().
-      + (* Need info regarding _off and _dlt bounds *)
-        have aux: _ASIZE < W64.modulus. admit.
-        have min_pos: 0 <= _off + _dlt. admit.
-        have max_pos: _off + _dlt + 8 < _ASIZE. admit.
-        rewrite !pmod_small 1:/# -compose_trail /#.
-    + rcondf 2. auto => /#.
-      by auto => /#.
-case(aT8 = 7).
-  rcondt 2. auto => /#.
-  case(lEN = 1). 
-  + rcondt 2. auto => /#.
-    rcondf 9. wp; ecall (SHLQ_h t8 aT8); auto => /#.
-    wp; ecall (SHLQ_h t8 aT8); auto => />.
-    rewrite !negb_or lezNgt -lezNgt /= => *.
-    split; first by smt(). move => *.
-    rewrite /subread_spec /subread_pre !andaE oraE => *.
-    do split; 1..6: smt(); 2..4: smt().
-    + (* Need info regarding _off and _dlt bounds *)
-      have aux: _ASIZE < W64.modulus. admit.
-      have min_pos: 0 <= _off + _dlt. admit.
-      have max_pos: _off + _dlt + 8 < _ASIZE. admit.
-        rewrite !of_uintK !pmod_small. 
-          split; first smt(). move=> _. rewrite(ltr_trans _ASIZE); 1:smt(). rewrite aux.
-      smt().
-      rewrite -(compose1u8_trail _ _ (_at - _cur)) /#.
-  + rcondf 2. auto => /#.
-    case(tRAIL %% 256 <> 0).
-    + rcondt 2. auto => /#.
-      wp; ecall (SHLQ_h t8 aT8); auto => />.
-      rewrite !negb_or lezNgt -lezNgt /= => *.
-      split; first by smt(). move => *.
-      rewrite /subread_spec /subread_pre !andaE oraE => *.
-      do split; 1..5: smt(); 2..5: smt(). have->: _len = 0 by smt().
-      + (* Need info regarding _off and _dlt bounds *)
-        have aux: _ASIZE < W64.modulus. admit.
-        have min_pos: 0 <= _off + _dlt. admit.
-        have max_pos: _off + _dlt + 8 < _ASIZE. admit.
-        rewrite !pmod_small 1:/# -compose_trail /#.
-    + rcondf 2. auto => /#.
-      by auto => /#.
-+ rcondf 2. auto => /#.
-  auto => /#.
+ auto => /> &m ????H??.
+ by apply subread_w8_trail => /#.
+auto => /> &m ????H; rewrite negb_and => [[C|C]].
+ by apply subread_w8_trail_ahead => /#.
+smt().
 qed.
 
-phoare a_ilen_read_upto8_at_ph _buf _off _dlt _len _trail _cur _at:
- [ MM.__a_ilen_read_upto8_at
- : buf=_buf /\ offset=_off /\ dELTA=_dlt /\ lEN=_len /\ tRAIL=_trail /\ cUR=_cur /\ aT=_at
- ==> subread_spec 8 _buf _off _dlt _len _trail _cur _at res.`1 res.`2 res.`3 res.`4 (u64bytes res.`5)
- ] = 1%r.
-proof.
-by conseq a_ilen_read_upto8_at_ll
-          (a_ilen_read_upto8_at_h _buf _off _dlt _len _trail _cur _at).
-qed.
-
-lemma nseq_ext (x: W8.t) y:
-  0 <= y =>
-  nseq y x ++ [x] = nseq (y+1) x.
-proof. move => H. rewrite -nseq1 (cat_nseq y 1 x) /#. qed.
-
-lemma u8init0:
-W8.init (fun (_ : int) => false) = W8.zero.
-proof.
-  rewrite (W8.ext_eq _ W8.zero). move => x x_bnd.
-  by rewrite initE ifT /#.
-  smt().
-qed.
-
-lemma u64init0:
-W64.init (fun (_ : int) => false) = W64.zero.
-proof.
-  rewrite (W64.ext_eq _ W64.zero). move => x x_bnd.
-  by rewrite initE ifT /#.
-  smt().
-qed.
-
-lemma u128init0:
-W128.init (fun (_ : int) => false) = W128.zero.
-proof.
-  rewrite (W128.ext_eq _ W128.zero). move => x x_bnd.
-  by rewrite initE ifT /#.
-  smt().
-qed.
-
-lemma u128_0s_v0 (_buf: W8.t A.t) _off _dlt _len _trail _cur _at:
-   0 <= _cur =>
-   0 <= _at =>
-   _at < _cur =>
-   0 <= _len =>
-   _len = 0 /\ _trail = 0 =>
-  u128bytes W128.zero = bytes_at 16 _cur _at (sub _buf (_off + _dlt) _len ++ [W8.of_int _trail]).
-proof.
-  move => ? ? ? ? H.
-  pose l1:= u128bytes W128.zero.
-  pose l2:=  bytes_at 16 _cur _at (sub _buf (_off + _dlt) _len ++ [W8.of_int _trail]). 
-  rewrite (eq_from_nth W8.zero l1 l2).
-  + rewrite size_to_list size_take 1:/# !size_cat size_drop 1:/# !size_cat !size_mkseq.
-    rewrite !size_nseq ifF /#.
-  + rewrite size_to_list => i i_bnd.
-    rewrite nth_to_list /(\bits8) nth_take ..2:/# !nth_cat size_drop 1:/# !size_cat.
-    rewrite !H size_mkseq size_nseq /= ifF 1:/#.  rewrite u8init0 nth_nseq /#.
-    smt().
-qed.
-
-lemma u128_0s_v1 (_buf: W8.t A.t) _off _dlt _len _trail _cur _at:
-   0 <= _cur =>
-   0 <= _at =>
-   _cur <= _at =>
-   0 <= _len =>
-   _len = 0 /\ _trail = 0 =>
-  u128bytes W128.zero = bytes_at 16 _cur _at (sub _buf (_off + _dlt) _len ++ [W8.of_int _trail]).
-proof.
-  move => ???? H.
-  pose l1:= u128bytes W128.zero.
-  pose l2:=  bytes_at 16 _cur _at (sub _buf (_off + _dlt) _len ++ [W8.of_int _trail]). 
-  rewrite (eq_from_nth W8.zero l1 l2).
-  + rewrite size_to_list size_take 1:/# !size_cat size_drop 1:/# !size_cat !size_mkseq.
-    rewrite !size_nseq ifT /#.
-  + rewrite size_to_list => i i_bnd.
-    rewrite nth_to_list /(\bits8) nth_take ..2:/# !nth_cat size_drop 1:/# !size_cat.
-    rewrite size_mkseq size_nseq !lez_maxr ..5:/# !H /sub mkseq0 cat0s nseq_ext 1:/#/=.
-    case(i < _at + 1 - _cur) =>*.
-    + rewrite nth_drop ..2:/# nth_nseq 1:/# u8init0 /#.
-    + rewrite nth_nseq 1:/# u8init0 /#.
-    smt().
-qed.
-
-lemma u128_0s_v2 (_buf: W8.t A.t) _off _dlt _len _trail _cur _at:
-   0 <= _cur =>
-   0 <= _at =>
-   0 <= _len =>
-   _cur + 16 <= _at =>
-  u128bytes W128.zero = bytes_at 16 _cur _at (sub _buf (_off + _dlt) _len ++ [W8.of_int _trail]).
-proof.
-  move => ??? H.
-  pose l1:= u128bytes W128.zero.
-  pose l2:=  bytes_at 16 _cur _at (sub _buf (_off + _dlt) _len ++ [W8.of_int _trail]). 
-  rewrite (eq_from_nth W8.zero l1 l2).
-  + rewrite size_to_list size_take 1:/# !size_cat size_drop 1:/# !size_cat !size_mkseq.
-    rewrite !size_nseq ifT /#.
-  + rewrite size_to_list => i i_bnd.
-    rewrite nth_to_list /(\bits8) nth_take ..2:/# !nth_cat size_drop 1:/# !size_cat.
-    rewrite size_mkseq size_nseq !lez_maxr ..5:/# /sub ifT 1:/# drop_cat size_nseq.
-    rewrite ifT 1:/# nth_cat size_drop 1:/# size_nseq ifT 1:/# nth_drop ..2:/#.
-    rewrite nth_nseq 1:/# u8init0 /#.
-    smt().
-qed.
-
-lemma full_u128_0s (_buf: W8.t A.t) _off _dlt _len _trail _cur _at:
-  0 <= _cur =>
-  0 <= _at =>
-  0 <= _len =>
-  ((_len = 0 /\ _trail = 0 /\ (_at < _cur \/ _cur <= _at)) \/ _cur + 16 <= _at) =>
-  u128bytes W128.zero = bytes_at 16 _cur _at (sub _buf (_off + _dlt) _len ++ [W8.of_int _trail]).
-proof.
-  move => H0 H1 H2 [[? [? [H | H]]] | H].
-    rewrite (u128_0s_v0 _buf _off _dlt _len _trail _cur _at) /#.
-    rewrite (u128_0s_v1 _buf _off _dlt _len _trail _cur _at) /#.
-    rewrite (u128_0s_v2 _buf _off _dlt _len _trail _cur _at) /#.
-qed.
-
-lemma compose16u8 (buf: W8.t A.t) pos at cur len trail:
-  16 <= len =>
-  0 <= cur =>
-  0 <= at =>
-  0 <= pos =>
-  pos + 16 <= _ASIZE =>
-  cur <= at =>
-  u128bytes (get128_direct (WA.init8 ("_.[_]" buf)) pos `<<<` 8 * (at - cur)) =
-  bytes_at 16 cur at (sub buf pos len ++ [W8.of_int trail]).
-proof.
-  move => H0 H1 H2 H3 H4 H5.
-  pose l1:= u128bytes (get128_direct (WA.init8 ("_.[_]" buf)) pos `<<<` 8 * (at - cur)).
-  pose l2:= bytes_at 16 cur at (sub buf pos len ++ [W8.of_int trail]).
-  rewrite (eq_from_nth W8.zero l1 l2).
-  + rewrite size_to_list size_take 1:/# size_cat size_drop 1:/# !size_cat size_mkseq.
-    rewrite !size_nseq ifT /#.
-  + rewrite size_to_list. move => i i_bnd.
-    rewrite nth_to_list /(\bits8) nth_take ..2:/# nth_cat nth_drop ..2:/# size_drop 1:/#.
-    rewrite !size_cat size_mkseq size_nseq !lez_maxr ..5:/# ifT 1:/# /=.
-    rewrite nth_cat size_nseq lez_maxr 1:/#.
-    case(i < at - cur) => cT.
-    + rewrite ifT 1:/# nth_nseq 1:/# (W8.ext_eq _ W8.zero). move => x x_bnd.
-      + rewrite initE ifT 1:/# /=. have->: 0 <= i * 8 + x < 128 by smt().
-        rewrite andaE andTb get_out /#.
-      smt().
-    + rewrite ifF 1:/# nth_cat size_mkseq ifT 1:/#.
-      rewrite (W8.ext_eq _ ((sub buf pos len).[cur + i - at])). move => x x_bnd.
-      + rewrite initE ifT 1:/# /=. have->: 0 <= i * 8 + x < 128 by smt().
-        rewrite andaE andTb /get128_direct /pack16_t initE ifT 1:/# /=.
-        rewrite initiE 1:/# /= initE ifT 1:/# /sub nth_mkseq /#.
-      smt().
-    smt().
-qed.
-
-lemma u128_to_1u64 x:
-    u128bytes (VPINSR_2u64 W128.zero x W8.one) =
-    u64bytes (W64.zero) ++ (u64bytes x).
-proof.
-  pose l1:= u128bytes (VPINSR_2u64 W128.zero x W8.one).
-  pose l2:= u64bytes W64.zero ++ u64bytes x.
-  rewrite (eq_from_nth W8.zero l1 l2).
-  + rewrite size_cat !size_to_list /#. 
-  + rewrite size_to_list => i i_bnd.
-    case(i < 8) => i_small.
-    + rewrite nth_cat !nth_to_list /VPINSR_2u64 /(\bits8) !size_to_list.
-      rewrite to_uint1 pmod_small 1:/# ifT 1:/# u8init0 (W8.ext_eq _ W8.zero).
-      + move => x0 x0_bnd. rewrite initE ifT 1:/# /pack2_t /= initE ifT 1:/# /= initE.
-        rewrite ifT 1:/# /= ifF 1:/# /(\bits64) u64init0 /#.
-        smt().
-    + rewrite nth_cat !nth_to_list /VPINSR_2u64 /(\bits8) !size_to_list.
-      rewrite to_uint1 pmod_small 1:/# ifF 1:/#.
-      rewrite (W8.ext_eq _ (W8.init (fun j => x.[(i - 8) * 8 + j]))).
-      +  move => x0 x0_bnd. rewrite initE ifT 1:/# /pack2_t /= initE ifT 1:/# /= initE.
-        rewrite ifT 1:/# /= ifT 1:/# /(\bits64) initE ifT /#.
-      smt().
-    smt().
-qed.
-
-lemma u128_to_2u64 x y:
-  u128bytes (VPINSR_2u64 (zeroextu128 x) y W8.one) =
-  u64bytes x ++ u64bytes y.
-proof.
-  pose l1:= u128bytes (VPINSR_2u64 (zeroextu128 x) y W8.one).
-  pose l2:= u64bytes x ++ u64bytes y.
-  rewrite (eq_from_nth W8.zero l1 l2). 
-  + rewrite size_cat !size_to_list /#.
-  + rewrite size_to_list => i i_bnd.
-    rewrite !nth_to_list /(\bits8) (W8.ext_eq _ l2.[i]). move => x0 x0_bnd.
-    + rewrite initE ifT 1:/# /VPINSR_2u64 /pack2_t /= initE nth_cat size_to_list.
-      case(i < 8) => i_small.
-      + have->: 0 <= i * 8 + x0 < 128 by smt().
-        rewrite andaE andTb initE ifT 1:/# /= ifF 1:/# /(\bits64) initE ifT 1:/#.
-        rewrite /= /zeroextu128 /W128.of_int pmod_small.
-        (*****************************************************************************
-         * This needs to be fixed:                                                   *
-         * 1) smt() can't solve have using W64.to_uint_cmp                           *
-         * 2) smt() can't solve ltr_trans/ltr_le_trans despite having b in context   *
-         *****************************************************************************)
-           have [a b]:0 <= W64.to_uint x < W64.modulus 
-             by rewrite W64.to_uint_cmp.
-           split. smt(). rewrite (ltr_trans W64.modulus) 1:b /#.
-         rewrite get_bits2w 1:/# (int2bs_cat 64) 1:/# pdiv_small.
-           have [a b]:0 <= W64.to_uint x < W64.modulus 
-            by rewrite W64.to_uint_cmp.
-           split. smt(). rewrite (ltr_le_trans W64.modulus) 1:b /#.
-         rewrite nth_cat size_int2bs ifT 1:/# /to_uint.
-         have{1}->: 64 = size (w2bits x) by rewrite size_w2bits.
-         rewrite bs2intK /u64bytes nth_to_list /(\bits8) get_w2bits initE /#.
-      + have->: 0 <= i * 8 + x0 < 128 by smt().
-        rewrite andaE andTb initE ifT 1:/# /= ifT 1:/# /u64bytes nth_to_list /(\bits8).
-        rewrite initE ifT /#.
-      smt().
-    smt().
-qed.
-
-
-lemma u128_compose8u8_trail (_buf: W8.t A.t) x _off _dlt _len _trail _cur _at:
-  0 <= _len =>
-  _len < 16 =>
-  0 <= _cur =>
-  0 <= _at =>
-  8 <= _at - _cur =>
-  u64bytes x =
-    bytes_at 8 8 (_at - _cur) (sub _buf (_off + _dlt) _len ++ [W8.of_int _trail]) =>
-  u64bytes W64.zero ++ u64bytes x =
-  bytes_at 16 _cur _at (sub _buf (_off + _dlt) _len ++ [W8.of_int _trail]).
-proof.
-  move => H0 H1 H2 H3 H4 H5.
-  pose l1:= u64bytes W64.zero ++ u64bytes x.
-  pose l2:= bytes_at 16 _cur _at (sub _buf (_off + _dlt) _len ++ [W8.of_int _trail]).
-  rewrite (eq_from_nth W8.zero l1 l2).
-  + rewrite !size_cat !size_to_list !size_take ..1:/# !size_cat !size_drop ..1:/#.
-    rewrite !size_cat !size_mkseq !size_nseq !lez_maxr ..6:/# ifT /#.
-  + rewrite size_cat !size_to_list /= => i i_bnd.
-    rewrite /l1 H5 /l2.
-    rewrite !nth_cat size_to_list !nth_take ..4:/# !nth_cat !size_drop ..2:/# !size_cat.
-    rewrite !size_mkseq !size_nseq !lez_maxr..8:/# /=.
-    case(i < 8) => i_small.
-    + rewrite nth_to_list /(\bits8) u8init0 nth_drop ..2:/# !nth_cat size_mkseq !size_nseq.
-      rewrite ifT 1:/# nth_nseq /#.
-    + case(i < _at - _cur + _len) => i_mid0.
-      + rewrite ifT 1:/# !nth_drop ..4:/# !nth_cat !size_nseq !lez_maxr ..2:/# !size_mkseq.
-        case(i < _at - _cur) => i_pre.
-        + rewrite !ifT ..3:/# !nth_nseq /#.
-        + rewrite ifF 1:/# ifT 1:/# ifT 1:/# ifF 1:/# ifT /#.
-      + case(i < _at - _cur + _len + 1) => i_mid1.
-        + rewrite ifT 1:/# !nth_drop..4:/# !nth_cat !size_nseq !lez_maxr..2:/# !size_mkseq.
-          rewrite ifF 1:/# ifF 1:/# ifT 1:/# ifF 1:/# ifF /#.
-    + rewrite !ifF ..2:/# !nth_nseq /#.
-    smt().
-qed.
-
-lemma u128_compose16u8_trail (_buf: W8.t A.t) x0 x1 y1 y2 y3 y4 _off _dlt _len _trail _cur _at:
-  0 <= _len =>
-  0 <= _cur =>
-  0 <= _at =>
-  _cur <= _at =>
-  _at - _cur < 8 =>
-  y1 =  _dlt + _len - y2 =>
-  y2 = max 0 (_len - max 0 (8 - (_at - _cur))) =>
-  y4 = max (_at - _cur) (min 8 (_at - _cur + _len + b2i (_trail <> 0))) =>
-  (8 <= _len + (_at - _cur) /\ y3 = _trail \/ _len + (_at - _cur) < 8 /\ y3 = 0) =>
-  u64bytes x0 =
-    bytes_at 8 0 (_at - _cur) (sub _buf (_off + _dlt) _len ++ [W8.of_int _trail]) =>
-  u64bytes x1 =
-    bytes_at 8 8 y4 (sub _buf (_off + y1) y2 ++ [W8.of_int y3]) =>
-  u64bytes x0 ++ u64bytes x1 = bytes_at 16 _cur _at (sub _buf (_off + _dlt) _len ++ [W8.of_int _trail]).
-proof.
-  move => ?????h0 h1 h2 ? H0 H1.
-  pose l1:= u64bytes x0 ++ u64bytes x1.
-  pose l2:= bytes_at 16 _cur _at (sub _buf (_off + _dlt) _len ++ [W8.of_int _trail]).
-  rewrite (eq_from_nth W8.zero l1 l2).
-  + rewrite size_take /l2 /bytes_at 1:/# !size_cat size_drop 1:/# !size_to_list.
-    rewrite !size_cat size_mkseq !size_nseq /#.
-  + rewrite size_cat !size_to_list /= => i i_bnd.
-    rewrite nth_take ..2:/# !nth_cat H0 H1 !size_take 1:/# !nth_drop 1..2:/# !size_cat.
-    rewrite !size_drop ..2:/# !size_cat !size_mkseq !size_nseq !lez_maxr ..9:/# /=.
-    have->: 8 < _at-_cur+(_len+1)+8 by smt().
-    rewrite /=. case(i < 8) => i_small.
-    + case(i < _at - _cur) => pre_0s.
-      + rewrite nth_take ..2:/# drop0 !nth_cat !size_cat !size_mkseq !size_nseq !ifT..4:/#.
-        rewrite !nth_nseq /#.
-      + rewrite nth_take ..2:/# drop0 !nth_cat !size_cat !size_mkseq !size_nseq.
-        case(i < _at - _cur + _len) => *.
-        + rewrite ifT 1:/# ifF 1:/# ifT 1:/# ifT 1:/# ifF 1:/# ifT /#. 
-        + case(i < _at - _cur + _len + 1) => *.
-          + rewrite ifT 1:/# ifF 1:/# ifF 1:/# ifT 1:/# ifT 1:/# ifF /#.
-          + rewrite ifF 1:/# ifF 1:/# !nth_nseq /#.
-    + case(i < _at - _cur) => pre_0s.
-      + rewrite nth_take ..2:/# !nth_cat nth_drop ..2:/# !size_drop 1:/# !size_mkseq.
-        rewrite !size_nseq !ifT..4:/# nth_nseq /#.
-      + rewrite nth_take ..2:/# !nth_cat nth_drop ..2:/# !size_drop 1:/# !size_mkseq.
-        rewrite !size_cat !size_nseq !size_mkseq !nth_cat !size_mkseq !size_nseq.
-        case(i < _at - _cur + _len) => *.
-        + rewrite ifT 1:/# ifF 1:/# ifT 1:/# ifT 1:/# ifF 1:/# ifT 1:/# !nth_mkseq /#.
-        + case(i < _at - _cur + _len + 1) => *.
-          + rewrite ifT 1:/# ifF 1:/# ifF 1:/# ifT 1:/# ifT 1:/# ifF 1:/# ifF 1:/# ifT /#.
-          + rewrite h0 h1 h2. case(_trail <> 0) => *.
-            + case(8 < _at - _cur + _len + b2i true) => *.
-              + rewrite lez_minl 1:/# !ifF ..2:/# !nth_nseq /#.
-              + rewrite lez_minr 1:/#. case(0 <= _len + (_at - _cur) - 8) => *.
-                + rewrite !ifF ..2:/# !nth_nseq /#.
-                + case(i < _at - _cur + _len + 2) =>*.
-                  + rewrite ifT 1:/# ifF 1:/# ifF 1:/# ifT 1:/# ifF 1:/# !nth_nseq /#.
-                  + rewrite !ifF ..2:/# !nth_nseq /#.
-            + rewrite !ifF ..2:/# !nth_nseq /#.
-    smt().
-qed.
 
 hoare a_ilen_read_upto16_at_h _buf _off _dlt _len _trail _cur _at:
  MM.__a_ilen_read_upto16_at
  : buf=_buf /\ offset=_off /\ dELTA=_dlt /\ lEN=_len /\ tRAIL=_trail /\ cUR=_cur /\ aT=_at
  ==> subread_spec 16 _buf _off _dlt _len _trail _cur _at res.`1 res.`2 res.`3 res.`4 (u128bytes res.`5).
-proc.
-(* ((aT < cUR \/ cUR + 16 <= aT) \/ lEN = 0 /\ tRAIL = 0) *)
+proof.
+proc; simplify.
+
 if => //.
-+ auto => /> H. rewrite /subread_spec /subread_pre !andaE !oraE. 
-  move => H0 [#]H1 H2 H3 H4 H5 H6 H7.
-  do split; 1..7: smt(); 2..3: smt().
-  rewrite (full_u128_0s _buf _off _dlt _len _trail _cur _at) /#.
+ auto => |> [[H|H]|H]. 
+ + move=> _; rewrite /subread_pre => /> ?????????.
+   rewrite (:!_cur<=_at) 1:/# /= => [[Elen Etb]].
+   rewrite !Elen !Etb; split; first smt().
+   split.
+    rewrite sub0 bytes_at_zeros 1:/# /u128bytes /= !get_zero.
+    by rewrite -mkseq_nseq /mkseq -iotaredE.
+   smt().
+  + by apply subread_spec_ahead16; smt().
+  by apply subread_spec_empty16; smt().
+
 (* 16 <= lEN *)
-sp. wp. if => //.
-+ wp; ecall (SHLDQ_h w aT16); auto => />.
-  rewrite !negb_or negb_and. move => [#] H0 H1 H2 H3 H4.
-  split; first by smt(). move => H5 H6 H7.
-  rewrite /subread_pre !andaE oraE. move => [#] H8 H9 H10 H11 H12 H13 H14.
-  do split; ..6: smt(); 2..: smt().
-  + have aux: _ASIZE < W64.modulus. admit.
-    have min_pos: 0 <= _off + _dlt. admit.
-    have max_pos: _off + _dlt + 16 < _ASIZE. admit.
-    rewrite of_uintK pmod_small.
-      split; first smt(). move=> _. rewrite(ltr_trans _ASIZE); 1:smt(). rewrite aux.
-    apply compose16u8; smt().
+if => //.
+ wp; ecall (SHLDQ_h w (aT-cUR)); auto => |> *.
+ split; first smt().
+ move=> ??.
+ by apply (subread_u128 _buf _off _dlt _len _trail _cur _at _).
+
 (* lEN < 16 *)
 if => //.
-+ wp; ecall(a_ilen_read_upto8_at_h buf offset dELTA lEN tRAIL 8 aT16); auto => />.
-  rewrite !negb_or negb_and /subread_spec /subread_pre => [#] H0 H1 H2 H3 H4 H5.
-  rewrite !andaE !oraE. move => result H6 H7 [#]H8 H9 H10 H11 H12 H13 H14.
-  move: H6. rewrite H10 H11 H12 !andaE !oraE /=.
-  have->: 0 <= _at - _cur by smt().
-  have->: _at - _cur + _len + b2i (_trail <> 0) <= 200 by smt().
-  have->: (8 <= _at - _cur \/ _len = 0 /\ _trail = 0) by smt().
-  rewrite implyTb. move =>  [#] h1 h2 h3 h4 h5 h6 h7 h8 h9 h10 h11 h12.
-  do split; 1..7:smt(); 2..:smt().
-  + rewrite u128_to_1u64.
-    rewrite (u128_compose8u8_trail _buf result.`5 _off _dlt _len _trail _cur _at) /#.
-+ wp; ecall(a_ilen_read_upto8_at_h buf offset dELTA lEN tRAIL 8 aT16).
-  wp; ecall(a_ilen_read_upto8_at_h buf offset dELTA lEN tRAIL 0 aT16). auto => />.
-  rewrite !negb_or negb_and /subread_spec /subread_pre => [#] H0 H1 H2 H3 H4 H5.
-  rewrite !andaE !oraE. move => result ? result0 ?*.
-  do split; ..2: smt(); 2..: smt().
-  rewrite u128_to_2u64 (u128_compose16u8_trail _buf result.`5 result0.`5 result.`1
-                         result.`2 result.`3 result.`4 _off _dlt _len _trail _cur _at) /#.
+ (* CUR+8 <= AT *)
+ wp; ecall(a_ilen_read_upto8_at_h buf offset dELTA lEN tRAIL (cUR+8) aT); auto => |>.
+ rewrite !negb_or negb_and => |> ??????? [dlt0 len0 tb0 at0 w0] /= H.
+ have H0:= subread_spec_ahead8 _buf _off _dlt _len _trail _cur _at _;first  smt().
+ rewrite -zeroextu128_zero -u64bytes_cat.
+ by apply (subread_spec_cat 8 8 _ _ _ _ _ _ _ _ _ _ _ _ _ _ _ _ _ _ _ H0).
+
+wp; ecall(a_ilen_read_upto8_at_h buf offset dELTA lEN tRAIL (cUR+8) aT).
+wp; ecall(a_ilen_read_upto8_at_h buf offset dELTA lEN tRAIL cUR aT).
+auto => |>.
+rewrite !negb_or negb_and. 
+move => ???[]dlt0 len0 tb0 at0 w0 |> H0 []dlt1 len1 tb1 at1 w1 /= H1.
+rewrite -u64bytes_cat.
+by apply (subread_spec_cat 8 8 _ _ _ _ _ _ _ _ _ _ _ _ _ _ _ _ _ _ _ H0).
 qed.
 
 phoare a_ilen_read_upto16_at_ph _buf _off _dlt _len _trail _cur _at:
@@ -2969,295 +1634,64 @@ by conseq a_ilen_read_upto16_at_ll
           (a_ilen_read_upto16_at_h _buf _off _dlt _len _trail _cur _at).
 qed.
 
-
-lemma u256_to_1u128 x:
-    u256bytes (VINSERTI128 W256.zero x W8.one) =
-    u128bytes (W128.zero) ++ (u128bytes x).
-proof.
-  pose l1:= u256bytes (VINSERTI128 W256.zero x W8.one).
-  pose l2:= u128bytes W128.zero ++ u128bytes x.
-  rewrite (eq_from_nth W8.zero l1 l2).
-  + rewrite size_cat !size_to_list /#. 
-  + rewrite size_to_list => i i_bnd.
-    case(i < 16) => i_small.
-    + rewrite nth_cat !nth_to_list /VINSERTI128 /(\bits8) !size_to_list.
-      rewrite to_uint1 pmod_small 1:/# ifT 1:/# u8init0 (W8.ext_eq _ W8.zero).
-      + move => x0 x0_bnd. rewrite initE ifT 1:/# /pack2_t /= initE ifT 1:/# /of_list /=.
-        rewrite initE ifT 1:/# /= ifT 1:/# /(\bits128) /= u128init0 /#.
-        smt().
-    + rewrite nth_cat !nth_to_list /VINSERTI128 /(\bits8) !size_to_list.
-      rewrite to_uint1 pmod_small 1:/# ifF 1:/#.
-      rewrite (W8.ext_eq _ (W8.init (fun j => x.[(i - 16) * 8 + j]))).
-      +  move => x0 x0_bnd. rewrite initE ifT 1:/# /pack2_t /= initE ifT 1:/# /= initE.
-        rewrite ifT 1:/# /= /of_list initE ifT 1:/# /(\bits64) /= ifF 1:/# ifT /#.
-      smt().
-    smt().
-qed.
-
-lemma u256_to_2u128 x y:
-u256bytes (W256.of_int (to_uint x %% W128.modulus + W128.modulus * to_uint y)) =
-u128bytes x ++ u128bytes y.
-proof.
-  have [a b]: 0 <= W128.to_uint x < W128.modulus by rewrite W128.to_uint_cmp.
-  have [c d]: 0 <= W128.to_uint y < W128.modulus by rewrite W128.to_uint_cmp.
-  rewrite pmod_small. rewrite b /#.
-  rewrite /of_int (int2bs_cat 128) 1:/# !pmod_small.
-  + split. smt(). move =>*.
-    have->: W256.modulus = 2^128 + 2^128 * (2^128-1) by smt().
-    rewrite ltr_le_add.
-    + rewrite 1:b /#.
-    + rewrite ler_pmul2l 1:/# -ltzS d /#.
-  rewrite mulrC divzMDr 1:/# pdiv_small 1:b 1:/# addr0 -int2bs_mod dvdz_modzDr 1:/#.
-  rewrite pmod_small 1:b 1:/#.
-  have->: u256bytes (W256.bits2w (int2bs 128 (to_uint x) ++ int2bs (256-128) (to_uint y)))
-        = u128bytes (x) ++ u128bytes (y).
-    rewrite (eq_from_nth W8.zero _ (u128bytes x ++ u128bytes y)).
-    + rewrite size_cat !size_to_list /#.
-    + rewrite size_to_list => i i_bnd.
-      rewrite nth_cat size_to_list nth_to_list /(\bits8). case(i < 16) => i_small.
-      + rewrite (W8.ext_eq _ (u128bytes x).[i]). move => x0 x0_bnd.
-        + rewrite initE ifT 1:/# /= get_bits2w 1:/# nth_cat size_int2bs ifT 1:/#.
-          rewrite /to_uint. have->: 128 = size (w2bits x) by rewrite size_w2bits /#.
-          rewrite bs2intK get_w2bits nth_to_list /(\bits8) initE ifT /#. smt().
-      + rewrite (W8.ext_eq _ (u128bytes y).[i-16]). move => x0 x0_bnd.
-        + rewrite initE ifT 1:/# /= get_bits2w 1:/# nth_cat size_int2bs ifF 1:/#.
-          rewrite /to_uint. have->: 128 = size (w2bits y) by rewrite size_w2bits /#.
-          rewrite bs2intK get_w2bits nth_to_list /(\bits8) initE ifT /#. smt().
-     smt().
-   smt().
-qed.
-
-lemma u256_full_0s (_buf : W8.t A.t) _off _dlt _len _trail _cur _at:
- 0 <= _cur =>
- 0 <= _at =>
- 0 <= _len =>
- _cur + 32 <= _at \/ _len = 0 /\ _trail = 0 =>
- u256bytes W256.zero =
- bytes_at 32 _cur _at (sub _buf (_off + _dlt) _len ++ [W8.of_int _trail]).
-proof.
-  move => H0 H1 H2 H3.
-  pose l2:= bytes_at 32 _cur _at (sub _buf (_off + _dlt) _len ++ [W8.of_int _trail]).
-  rewrite (eq_from_nth W8.zero (u256bytes W256.zero) l2).
-  + rewrite size_to_list size_take 1:/# size_cat size_drop 1:/# !size_cat size_mkseq.
-    rewrite !size_nseq /#.
-  + rewrite size_to_list => i i_bnd.
-    rewrite nth_to_list /(\bits8) nth_take ..2:/# nth_cat size_drop 1:/# !size_cat.
-    rewrite size_mkseq size_nseq u8init0.
-    move: H3. move => [H3 | H3].
-    + case(i < _len + _at - _cur) => *.
-      + rewrite ifT 1:/# nth_drop ..2:/# !nth_cat size_nseq ifT 1:/# nth_nseq /#.
-      + rewrite ifF 1:/# nth_nseq /#.
-    + rewrite !H3 /=.
-      case(i < _at - _cur + 1) => *.
-      + rewrite ifT 1:/# nth_drop ..2:/# nth_cat size_nseq.
-        case(i<_at-_cur)=>*.
-        + rewrite ifT 1:/# nth_nseq /#.
-        + rewrite ifF 1:/# nth_cat size_mkseq ifF /#.
-      + rewrite ifF 1:/# !nth_nseq /#.
-    smt().
-qed.
-
-lemma u256compose32u8 (_buf : W8.t A.t) _off _dlt _len _trail _cur _at:
- 0 <= _cur =>
- 0 <= _at =>
+lemma subread_u256 _buf _off _dlt _len _trail _cur _at:
  32 <= _len =>
- 0 = _at - _cur =>
- 0 <= _off + _dlt =>
- _off + _dlt + 32 < _ASIZE =>
- u256bytes (get256_direct (WA.init8 ("_.[_]" _buf)) (_off + _dlt)) =
- bytes_at 32 _cur _at (sub _buf (_off + _dlt) _len ++ [W8.of_int _trail]).
+ _at-_cur = 0 =>
+ subread_spec 32 _buf _off _dlt _len _trail _cur _at
+  (_dlt + 32) (_len - 32) _trail (_at + 32)
+  (u256bytes
+     (get256_direct (WA.init8 ("_.[_]" _buf)) (_off + _dlt))).
 proof.
-  move => H0 H1 H2 H3 H4 H5.
-  pose l1:= u256bytes (get256_direct (WA.init8 ("_.[_]" _buf)) (_off + _dlt)).
-  pose l2:= bytes_at 32 _cur _at (sub _buf (_off + _dlt) _len ++ [W8.of_int _trail]).
-  rewrite (eq_from_nth W8.zero l1 l2).
-  + rewrite size_to_list size_take 1:/# size_cat size_drop 1:/# !size_cat size_mkseq.
-    rewrite !size_nseq /#.
-  + rewrite size_to_list => i i_bnd.
-    rewrite nth_to_list /(\bits8) nth_take ..2:/# nth_cat nth_drop ..2:/# size_drop 1:/#.
-    rewrite !size_cat size_mkseq !size_nseq ifT 1:/# !nth_cat size_nseq.
-    rewrite ifF 1:/# size_mkseq ifT 1:/#.
-    rewrite (W8.ext_eq _ (sub _buf (_off + _dlt) _len).[_cur + i - max 0 _at]).
-    + move => x x_bnd.
-      rewrite initE ifT 1:/# /= /get256_direct /pack32_t initE ifT 1:/# /= initE ifT 1:/#.
-      rewrite /= initE ifT 1:/# nth_mkseq /#.
-      smt().
-    smt().
+move=> Hen Hcur _ Hpre; split; first smt().
+split; last smt().
+apply (eq_from_nth W8.zero).
+ rewrite size_to_list size_take // size_cat size_nseq ler_maxr //=.
+ by rewrite size_drop 1:/# !size_cat size_sub 1:/# size_nseq /= /#.
+move=> i; rewrite size_to_list => Hi.
+rewrite nth_bytes_at 1..2:/#.
+rewrite get_u256bytes get256E pack32bE // initiE //= initiE 1:/#.
+by rewrite ifT 1:/# nth_cat size_sub 1:/# ifT 1:/# nth_sub /#.
 qed.
 
-
-lemma u256compose16u8 (_buf : W8.t A.t) x _off _dlt _len _trail _cur _at:
- 0 <= _cur =>
- 0 <= _at =>
- 0 <= _len =>
- 16 <= _at - _cur =>
- 0 <= _off + _dlt =>
- _off + _dlt + 32 < _ASIZE =>
- _cur <= _at \/ _len = 0 /\ _trail = 0 =>
- u128bytes x =
- bytes_at 16 16 (_at - _cur) (sub _buf (_off + _dlt) _len ++ [W8.of_int _trail]) =>
-u256bytes (VINSERTI128 W256.zero x W8.one) =
-bytes_at 32 _cur _at (sub _buf (_off + _dlt) _len ++ [W8.of_int _trail]).
-proof.
-  move =>??????? H0.
-  pose l1:= u256bytes (VINSERTI128 W256.zero x W8.one).
-  pose l2:= bytes_at 32 _cur _at (sub _buf (_off + _dlt) _len ++ [W8.of_int _trail]).
-  rewrite (eq_from_nth W8.zero l1 l2).
-  + rewrite size_to_list size_take 1:/# size_cat size_drop 1:/# !size_cat size_mkseq.
-    rewrite !size_nseq /#.
-  + rewrite size_to_list => i i_bnd.
-    rewrite /l1 u256_to_1u128 nth_cat size_to_list nth_take ..2:/# nth_cat nth_drop ..2:/#.
-    rewrite size_drop 1:/# !size_cat size_mkseq !size_nseq.
-    case(i < 16) => i_small.
-    + rewrite ifT 1:/# nth_to_list /(\bits8) /= u8init0 nth_cat size_nseq.
-      case(i < _at - _cur) => *.
-      + rewrite ifT 1:/# nth_nseq /#.
-        rewrite ifF 1:/# nth_cat size_mkseq /#.
-    + case(i < _at - _cur) => *.
-      + rewrite ifT 1:/# nth_cat size_nseq ifT 1:/# H0 nth_take ..2:/# nth_cat.
-        rewrite size_drop 1:/# !size_cat size_mkseq !size_nseq ifT 1:/# nth_drop ..2:/#.
-        rewrite !nth_cat size_nseq ifT 1:/# !nth_nseq /#.
-      + case(i < _at - _cur + _len) => *.
-        + rewrite H0 nth_take ..2:/# !nth_cat size_drop 1:/# !size_cat size_mkseq.
-          rewrite !size_nseq ifT 1:/# ifT 1:/# ifF 1:/# ifT 1:/# nth_drop ..2:/# !nth_cat.
-          rewrite size_mkseq size_nseq ifF 1:/# ifT /#.
-        + case(i < _at - _cur + _len + 1) => *.
-          + rewrite H0 nth_take ..2:/# !nth_cat size_drop 1:/# !size_cat size_mkseq.
-            rewrite size_nseq ifT 1:/# ifT 1:/# size_nseq ifF 1:/# ifF 1:/# nth_drop..2:/#.
-            rewrite !nth_cat size_nseq ifF 1:/# size_mkseq ifF /#.
-          + rewrite H0 nth_take ..2:/# !nth_cat size_drop 1:/# !size_cat size_mkseq.
-            rewrite size_nseq !ifF ..2:/# !nth_nseq /#.
-        smt().
-qed.
-
-lemma u256_compose32u8 (_buf: W8.t A.t) x0 x1 y1 y2 y3 y4 _off _dlt _len _trail _cur _at:
-  0 <= _len =>
-  0 <= _cur =>
-  0 <= _at =>
-  _cur <= _at =>
-  _at - _cur < 32 =>
-  y1 =  _dlt + _len - y2 =>
-  y2 = max 0 (_len - max 0 (16 - (_at - _cur))) =>
-  y4 = max (_at - _cur) (min 16 (_at - _cur + _len + b2i (_trail <> 0))) =>
-  (16 <= _len + (_at - _cur) /\ y3 = _trail \/ _len + (_at - _cur) < 16 /\ y3 = 0) =>
-  u128bytes x0 =
-    bytes_at 16 0 (_at - _cur) (sub _buf (_off + _dlt) _len ++ [W8.of_int _trail]) =>
-  u128bytes x1 =
-    bytes_at 16 16 y4 (sub _buf (_off + y1) y2 ++ [W8.of_int y3]) =>
-  u128bytes x0 ++ u128bytes x1 =
-  bytes_at 32 _cur _at (sub _buf (_off + _dlt) _len ++ [W8.of_int _trail]).
-proof.
-  move => ??????y_2 y_4? H0 H1.
-  pose l2:= bytes_at 32 _cur _at (sub _buf (_off + _dlt) _len ++ [W8.of_int _trail]).
-  rewrite (eq_from_nth W8.zero (u128bytes x0 ++ u128bytes x1) l2).
-  + rewrite size_cat !size_to_list size_take 1:/# size_cat size_drop 1:/# !size_cat.
-    rewrite size_mkseq !size_nseq /#.
-  + rewrite size_cat !size_to_list => i i_bnd.
-    case(i < 16) => i_small.
-    + rewrite H0 H1 nth_cat size_take 1:/# drop0 !size_cat !size_mkseq !size_nseq.
-      + rewrite ifT 1:/# (W8.ext_eq _ l2.[i]). move => _x _X_bnd.
-        rewrite !nth_take ..4:/# drop0 !nth_cat !size_cat !size_mkseq !size_nseq.
-        rewrite size_drop 1:/# !size_cat !size_mkseq !size_nseq nth_drop ..2:/# !nth_cat.
-        case(i < _at - _cur) => *.
-        + rewrite size_nseq !ifT ..4:/# !nth_nseq /#.
-        + case(i < _at - _cur + _len) => *.
-          + rewrite size_mkseq size_nseq ifT 1:/# ifF 1:/# ifT 1:/# ifT 1:/# ifF 1:/#.
-            rewrite !ifT /#.
-          + case(i < _at - _cur + _len + 1) => *.
-            + rewrite size_mkseq size_nseq ifT 1:/# ifF 1:/# ifF 1:/# ifT 1:/# ifT 1:/#.
-              rewrite ifF 1:/# ifF 1:/# ifT /#.
-            + rewrite !ifF ..2:/# !nth_nseq /#. 
-      smt().
-    + rewrite nth_cat size_to_list ifF 1:/# H1 !nth_take ..4:/# !nth_cat !size_drop ..2:/#.
-      rewrite !size_cat !size_mkseq !size_nseq.
-      case(i < _at - _cur) => *.
-      + rewrite ifT 1:/# nth_drop ..2:/# !nth_cat !size_mkseq !size_nseq !ifT ..2:/#.
-        rewrite nth_drop ..2:/# nth_cat size_nseq ifT 1:/# !nth_nseq /#.
-      + case(i < _at - _cur + _len) => *.
-        + rewrite !ifT ..2:/# !nth_drop ..4:/# !nth_cat !size_mkseq !size_nseq ifF 1:/#.
-          rewrite ifT 1:/# ifF 1:/# ifT 1:/# !nth_mkseq /#.
-        + case(_trail = 0) =>*.
-          + case(_len + _at - _cur < 16) =>*.
-            + case(_at - _cur < 16) => *.
-              + rewrite !ifF ..2:/# !nth_nseq /#.
-              + rewrite !ifT ..2:/# !nth_drop ..4:/# !nth_cat !size_mkseq !size_nseq.
-                rewrite !ifF /#.
-            + case(_at - _cur < 16) => *.
-              + case(i < _len + (_at - _cur) + 1) => *.
-                + rewrite !ifT ..2:/# !nth_drop ..4:/# !nth_cat !size_mkseq !size_nseq.
-                  rewrite !ifF /#.
-                + rewrite !ifF ..2:/# !nth_nseq /#.
-              + case(i < _len + (_at - _cur) + 1) => *.
-                + rewrite !ifT ..2:/# !nth_drop ..4:/# !nth_cat !size_mkseq !size_nseq.
-                  rewrite !ifF /#.
-                + rewrite !ifF ..2:/# !nth_nseq /#.
-          + case(_len + _at - _cur + 1 < 16) =>*.
-            + case(_at - _cur < 16) => *.
-              + rewrite !ifF ..2:/# !nth_nseq /#.
-              + rewrite !ifT ..2:/# !nth_drop ..4:/# !nth_cat !size_mkseq !size_nseq.
-                rewrite !ifF /#.
-            + case(_at - _cur < 16) => *.
-              + case(i < _len + (_at - _cur) + 1) => *.
-                + rewrite !ifT ..2:/# !nth_drop ..4:/# !nth_cat !size_mkseq !size_nseq.
-                  rewrite !ifF /#.
-                + case(_len + _at - _cur < 16) => *.
-                  + case(i < 17) => *.
-                    + rewrite ifT 1:/# ifF 1:/# nth_drop ..2:/# nth_cat size_nseq ifF 1:/#.
-                      rewrite nth_cat size_mkseq ifF 1:/# nth_nseq /#.
-                    + rewrite !ifF ..2:/# !nth_nseq /#.
-                  + rewrite !ifF ..2:/# !nth_nseq /#.
-              + case(i < _len + _at - _cur + 1) => *.
-                + rewrite !ifT ..2:/# !nth_drop ..4:/# !nth_cat !size_mkseq !size_nseq.
-                  rewrite !ifF /#.
-                + rewrite !ifF ..2:/# !nth_nseq /#.
-          smt().
-qed.
-    
 hoare a_ilen_read_upto32_at_h _buf _off _dlt _len _trail _cur _at:
  MM.__a_ilen_read_upto32_at
  : buf=_buf /\ offset=_off /\ dELTA=_dlt /\ lEN=_len /\ tRAIL=_trail /\ cUR=_cur /\ aT=_at
  ==> subread_spec 32 _buf _off _dlt _len _trail _cur _at res.`1 res.`2 res.`3 res.`4 (u256bytes res.`5).
 proof.
-proc. if => //. auto => /> H. rewrite /subread_spec /subread_pre !andaE !oraE.
-  move => H0 [#]H1 H2 H3 H4 H5 H6 H7.
-  do split; 1..7: smt(); 2..3: smt().
-  rewrite (u256_full_0s _buf _off _dlt _len _trail _cur _at) /#.
-(* aT32 = 0 /\ 32 <= lEN *)
-sp. wp. if => //. auto => />. rewrite !negb_or -!lezNgt negb_and => H0 H1 H2 H3 H4.
-  rewrite /subread_spec /subread_pre !andaE !oraE.
-  do split; ..7: smt(); 2..: smt().
-    have min_pos: 0 <= _off + _dlt. admit.
-    have max_pos: _off + _dlt + 32 < _ASIZE. admit.
-  rewrite (u256compose32u8 _buf _off _dlt _len _trail _cur _at) /#.
-if => //. 
-  wp; ecall(a_ilen_read_upto16_at_h buf offset dELTA lEN tRAIL 16 aT32); auto => />.
-  rewrite !negb_or -!lezNgt negb_and => H0 H1 H2 H3.
-  rewrite /subread_spec /subread_pre !andaE !oraE.
-  move => H4 H5 [#] H6 H7 H8 H9 H10 H11 H12. move: H4.
-  rewrite H8 H9 H10 /=.
-  have->: 0 <= _at - _cur by smt().
-  have->: _at - _cur + _len + b2i (_trail <> 0) <= 200 by smt().
-  have->: 16 <= _at - _cur \/ _len = 0 /\ _trail = 0 by smt().
-  rewrite implyTb. move => [#] H13 H14 H15 H16 H17 H18 H19 H20 H21 H22 H23 H24.
-  do split; ..7: smt(); 2..: smt().
-    have min_pos: 0 <= _off + _dlt. admit.
-    have max_pos: _off + _dlt + 32 < _ASIZE. admit.
-  rewrite (u256compose16u8 _buf H3.`5 _off _dlt _len _trail _cur _at) /#.
-wp. ecall(a_ilen_read_upto16_at_h buf offset dELTA lEN tRAIL 16 aT32).
-wp. ecall(a_ilen_read_upto16_at_h buf offset dELTA lEN tRAIL 0 aT32); auto => />.
-  rewrite !negb_or -!lezNgt !negb_and /= => H0. rewrite lezNgt /= => H1 H2 H3.
-  rewrite /subread_spec /subread_pre !andaE !oraE.
-  move => H4 H5 H6 H7 [#]H8 H9 H10 H11 H12 H13 H14. rewrite !andaE oraE. move: H4.
-  rewrite H10 H11 H12 /=.
-  have->: 0 <= _at - _cur by smt().
-  have->: _at - _cur + _len + b2i (_trail <> 0) <= 200 by smt().
-  rewrite implyTb. move => [#] H15 H16 H17 H18 H19 H20 H21 H22 H23 H24 H25 H26.
-  move: H6. rewrite H15 H16 H17 H18 H19 H20 !andaE !oraE /=.
-  move => [#]  h1 h2 h3 h4 h5 h6 h7 h8*.
-  do split; ..7: smt(); 2..: smt().
-  have->: 340282366920938463463374607431768211456 = W128.modulus by smt().
-  rewrite u256_to_2u128 (u256_compose32u8 _buf H3.`5 H5.`5 H3.`1 H3.`2 H3.`3 H3.`4
-                                          _off _dlt _len _trail _cur _at) /#.
+proc; simplify.
+
+if => //.
+ auto => |> [[H|H]|H]. 
+ + move=> _; rewrite /subread_pre => /> ?????????.
+   rewrite (:!_cur<=_at) 1:/# /= => [[Elen Etb]].
+   rewrite !Elen !Etb; split; first smt().
+   split.
+    rewrite sub0 bytes_at_zeros /u256bytes 1:/# /= !get_zero.
+    by rewrite -mkseq_nseq /mkseq -iotaredE.
+   smt().
+  + by apply subread_spec_ahead32; smt().
+  by apply subread_spec_empty32; smt().
+
+(* 32 <= lEN *)
+sp; if => //.
+ auto => |> ??.
+ by apply subread_u256.
+
+(* lEN < 16 *)
+if => //.
+ (* CUR+16 <= AT *)
+ wp; ecall(a_ilen_read_upto16_at_h buf offset dELTA lEN tRAIL (cUR+16) aT); auto => |>.
+ rewrite !negb_or negb_and => |> ?????? [dlt0 len0 tb0 at0 w0] /= H.
+ have H0:= subread_spec_ahead16 _buf _off _dlt _len _trail _cur _at _;first  smt().
+ rewrite -zeroextu256_zero -u128bytes_cat.
+ by apply (subread_spec_cat 16 16 _ _ _ _ _ _ _ _ _ _ _ _ _ _ _ _ _ _ _ H0) => //.
+wp; ecall(a_ilen_read_upto16_at_h buf offset dELTA lEN tRAIL (cUR+16) aT).
+wp; ecall(a_ilen_read_upto16_at_h buf offset dELTA lEN tRAIL cUR aT).
+auto => |>.
+rewrite !negb_or negb_and. 
+move => ???[]dlt0 len0 tb0 at0 w0 |> H0 []dlt1 len1 tb1 at1 w1 /= H1.
+rewrite -u128bytes_cat.
+by apply (subread_spec_cat 16 16 _ _ _ _ _ _ _ _ _ _ _ _ _ _ _ _ _ _ _ H0 _).
 qed.
 
 
@@ -3271,33 +1705,6 @@ by conseq a_ilen_read_upto32_at_ll
           (a_ilen_read_upto32_at_h _buf _off _dlt _len _trail _cur _at).
 qed.
 
-require import Keccak_bindings.
 
-lemma trunc_zext_u64_u128 w:
- truncateu64 (W2u64.zeroextu128 w) = w.
-proof.
-rewrite zeroextu128E /truncateu64.
-admitted.
-
-equiv a_ilen_read_bcast_upto8_at_eq:
- MM.__a_ilen_read_bcast_upto8_at
- ~ MM.__a_ilen_read_upto8_at
- : ={arg}
- ==> (res.`1,res.`2,res.`3,res.`4,res.`5){1}
-     = (res.`1,res.`2,res.`3,res.`4,VPBROADCAST_4u64 (truncateu64 (zeroextu128 res.`5))){2}.
-proof.
-proc; simplify.
-if => //=.
- auto => />.
- by move=> *; clear; circuit.
-sp; if => //=.
- inline*; auto => /> &m *; split => *.
- + rewrite /VPSLL_4u64 /VPBROADCAST_4u64 /= -iotaredE /=; congr; congr=> />.
-   by (do split); rewrite /W64.(`<<`) trunc_zext_u64_u128 of_uintK modz_small 1:/# of_uintK modz_small /#.
- + by rewrite /W64.(`<<`) trunc_zext_u64_u128; congr; congr.
-inline *.
-rcondf {1} 9; first by auto.
-rcondf {1} 10; first by auto.
-admitted.
 
 end ReadWriteArray.
